lib/monads: refactor trace monad theories
This splits material out of Trace_Monad and Trace_VCG and into more
specific theories, following the same approach and structure as the
nondet theories. This commit is mainly focused on definitions and lemmas
that also appear in the nondet monad; trace monad concepts are left
where they are for now.

Signed-off-by: Corey Lewis <corey.lewis@proofcraft.systems>

lib/Monads/trace/Trace_Monad.thy
@@ -202,7 +202,7 @@ lemma bind_def2:
 lemma elem_bindE:
   "\<lbrakk>(tr, res) \<in> bind f g s;
     \<lbrakk>res = Incomplete \<or> res = Failed; (tr, map_tmres undefined undefined res) \<in> f s\<rbrakk> \<Longrightarrow> P;
-    \<And>tr' tr'' x s'. \<lbrakk>(tr', Result (x, s')) \<in> f s \<Longrightarrow> (tr'', res) \<in> g x s'; tr = tr'' @ tr'\<rbrakk> \<Longrightarrow> P\<rbrakk>
+    \<And>tr' tr'' x s'. \<lbrakk>(tr', Result (x, s')) \<in> f s; (tr'', res) \<in> g x s'; tr = tr'' @ tr'\<rbrakk> \<Longrightarrow> P\<rbrakk>
    \<Longrightarrow> P"
   by (auto simp: bind_def2)
 
@@ -687,166 +687,6 @@ definition Await :: "('s \<Rightarrow> bool) \<Rightarrow> ('s,unit) tmonad" whe
   od"
 
 
-section "Hoare Logic"
-
-subsection "Validity"
-
-text \<open>
-  This section defines a Hoare logic for partial correctness for
-  the interference trace monad as well as the exception monad.
-  The logic talks only about the behaviour part of the monad and ignores
-  the failure flag.
-
-  The logic is defined semantically. Rules work directly on the
-  validity predicate.
-
-  In the interference trace monad, validity is a triple of precondition,
-  monad, and postcondition. The precondition is a function from state to
-  bool (a state predicate), the postcondition is a function from return value
-  to state to bool. A triple is valid if for all states that satisfy the
-  precondition, all result values and result states that are returned by
-  the monad satisfy the postcondition. Note that if the computation returns
-  the empty set, the triple is trivially valid. This means @{term "assert P"}
-  does not require us to prove that @{term P} holds, but rather allows us
-  to assume @{term P}! Proving non-failure is done via separate predicate and
-  calculus (see below).\<close>
-
-definition valid :: "('s \<Rightarrow> bool) \<Rightarrow> ('s,'a) tmonad \<Rightarrow> ('a \<Rightarrow> 's \<Rightarrow> bool) \<Rightarrow> bool"
-  ("\<lbrace>_\<rbrace>/ _ /\<lbrace>_\<rbrace>") where
-  "\<lbrace>P\<rbrace> f \<lbrace>Q\<rbrace> \<equiv> \<forall>s. P s \<longrightarrow> (\<forall>(r,s') \<in> mres (f s). Q r s')"
-
-text \<open>
-  We often reason about invariant predicates. The following provides shorthand syntax
-  that avoids repeating potentially long predicates.\<close>
-abbreviation (input) invariant ::
-  "('s,'a) tmonad \<Rightarrow> ('s \<Rightarrow> bool) \<Rightarrow> bool" ("_ \<lbrace>_\<rbrace>" [59,0] 60) where
-  "invariant f P \<equiv> \<lbrace>P\<rbrace> f \<lbrace>\<lambda>_. P\<rbrace>"
-
-text \<open>
-  Validity for the exception monad is similar and build on the standard
-  validity above. Instead of one postcondition, we have two: one for
-  normal and one for exceptional results.\<close>
-definition validE ::
-  "('s \<Rightarrow> bool) \<Rightarrow> ('s, 'a + 'b) tmonad \<Rightarrow> ('b \<Rightarrow> 's \<Rightarrow> bool) \<Rightarrow> ('a \<Rightarrow> 's \<Rightarrow> bool) \<Rightarrow> bool"
-  ("\<lbrace>_\<rbrace>/ _ /(\<lbrace>_\<rbrace>,/ \<lbrace>_\<rbrace>)" ) where
-  "\<lbrace>P\<rbrace> f \<lbrace>Q\<rbrace>,\<lbrace>E\<rbrace> \<equiv> \<lbrace>P\<rbrace> f \<lbrace> \<lambda>v s. case v of Inr r \<Rightarrow> Q r s | Inl e \<Rightarrow> E e s \<rbrace>"
-
-lemma validE_def2:
-  "\<lbrace>P\<rbrace> f \<lbrace>Q\<rbrace>,\<lbrace>E\<rbrace> \<equiv> \<forall>s. P s \<longrightarrow> (\<forall>(r,s') \<in> mres (f s). case r of Inr b \<Rightarrow> Q b s' | Inl a \<Rightarrow> E a s')"
-  by (unfold valid_def validE_def)
-(*
-text \<open>Validity for exception monad with interferences. Not as easy to phrase
- as we need to \<close>
-definition validIE :: "('s, 'a + 'b) tmonad \<Rightarrow>
-             's rg_pred \<Rightarrow>
-             's rg_pred \<Rightarrow> 's rg_pred \<Rightarrow>
-             ('b \<Rightarrow> 's rg_pred) \<Rightarrow>
-             ('a \<Rightarrow> 's rg_pred) \<Rightarrow> bool"
- ("_ //PRE _//RELY _//GUAR _//POST _//EXC _" [59,0,0,0,0,0] 60) where
-  "validIE f P R G Q E \<equiv> f SAT [P,R,G,\<lambda>v. case v of Inr r \<Rightarrow> Q r | Inl e \<Rightarrow> E e]"
-
-abbreviation (input)
-  validIEsat :: "('s, 'a + 'b) tmonad \<Rightarrow>
-             's rg_pred \<Rightarrow>
-             's rg_pred \<Rightarrow> 's rg_pred \<Rightarrow>
-             ('b \<Rightarrow> 's rg_pred) \<Rightarrow>
-             ('a \<Rightarrow> 's rg_pred) \<Rightarrow> bool"
-  ("_ //SAT [_, _, _, _, _]" [59,0,0,0,0,0] 60)
-  where
-  "validIEsat f P R G Q E \<equiv> validIE f P R G Q E"
- *)
-text \<open>
-  The following two instantiations are convenient to separate reasoning for exceptional and
-  normal case.\<close>
-(* Narrator: they are in fact not convenient, and are now considered a mistake that should have
-             been an abbreviation instead. *)
-definition validE_R :: (* FIXME lib: this should be an abbreviation *)
-  "('s \<Rightarrow> bool) \<Rightarrow> ('s, 'e + 'a) tmonad \<Rightarrow> ('a \<Rightarrow> 's \<Rightarrow> bool) \<Rightarrow> bool" ("\<lbrace>_\<rbrace>/ _ /\<lbrace>_\<rbrace>, -") where
-  "\<lbrace>P\<rbrace> f \<lbrace>Q\<rbrace>,- \<equiv> validE P f Q (\<lambda>x y. True)"
-
-definition validE_E :: (* FIXME lib: this should be an abbreviation *)
-  "('s \<Rightarrow> bool) \<Rightarrow>  ('s, 'e + 'a) tmonad \<Rightarrow> ('e \<Rightarrow> 's \<Rightarrow> bool) \<Rightarrow> bool" ("\<lbrace>_\<rbrace>/ _ /-, \<lbrace>_\<rbrace>") where
-  "\<lbrace>P\<rbrace> f -,\<lbrace>Q\<rbrace> \<equiv> validE P f (\<lambda>x y. True) Q"
-
-
-text \<open>rg_pred type: Rely-Guaranty predicates (state before => state after => bool)\<close>
-type_synonym 's rg_pred = "'s \<Rightarrow> 's \<Rightarrow> bool"
-
-text \<open>Abbreviations for trivial postconditions (taking three arguments):\<close>
-abbreviation(input)
-  toptoptop :: "'a \<Rightarrow> 'b \<Rightarrow> 'b \<Rightarrow> bool" ("\<top>\<top>\<top>") where
-  "\<top>\<top>\<top> \<equiv> \<lambda>_ _ _. True"
-
-abbreviation(input)
-  botbotbot :: "'a \<Rightarrow> 'b \<Rightarrow> 'b \<Rightarrow> bool" ("\<bottom>\<bottom>\<bottom>") where
-  "\<bottom>\<bottom>\<bottom> \<equiv> \<lambda>_ _ _. False"
-
-
-subsection "Determinism"
-
-text \<open>
-  A monad of type @{text tmonad} is deterministic iff it
-  returns an empty trace, exactly one state and result and does not fail\<close>
-definition det :: "('a,'s) tmonad \<Rightarrow> bool" where
-  "det f \<equiv> \<forall>s. \<exists>r. f s = {([], Result r)}"
-
-text \<open>A deterministic @{text tmonad} can be turned into a normal state monad:\<close>
-definition the_run_state :: "('s,'a) tmonad \<Rightarrow> 's \<Rightarrow> 'a \<times> 's" where
-  "the_run_state M \<equiv> \<lambda>s. THE s'. mres (M s) = {s'}"
-
-
-subsection "Non-Failure"
-
-text \<open>
-  With the failure flag, we can formulate non-failure separately from validity.
-  A monad @{text m} does not fail under precondition @{text P}, if for no start
-  state that satisfies the precondition it sets the failure flag.
-\<close>
-definition no_fail :: "('s \<Rightarrow> bool) \<Rightarrow> ('s,'a) tmonad \<Rightarrow> bool" where
-  "no_fail P m \<equiv> \<forall>s. P s \<longrightarrow> Failed \<notin> snd ` (m s)"
-
-text \<open>
-  It is often desired to prove non-failure and a Hoare triple simultaneously, as the reasoning
-  is often similar. The following definitions allow such reasoning to take place.\<close>
-
-definition validNF ::
-  "('s \<Rightarrow> bool) \<Rightarrow> ('s,'a) tmonad \<Rightarrow> ('a \<Rightarrow> 's \<Rightarrow> bool) \<Rightarrow> bool" ("\<lbrace>_\<rbrace>/ _ /\<lbrace>_\<rbrace>!") where
-  "validNF P f Q \<equiv> valid P f Q \<and> no_fail P f"
-
-definition validE_NF ::
-  "('s \<Rightarrow> bool) \<Rightarrow> ('s, 'a + 'b) tmonad \<Rightarrow> ('b \<Rightarrow> 's \<Rightarrow> bool) \<Rightarrow> ('a \<Rightarrow> 's \<Rightarrow> bool) \<Rightarrow> bool"
-  ("\<lbrace>_\<rbrace>/ _ /(\<lbrace>_\<rbrace>,/ \<lbrace>_\<rbrace>!)") where
-  "validE_NF P f Q E \<equiv> validE P f Q E \<and> no_fail P f"
-
-lemma validE_NF_alt_def:
-  "\<lbrace> P \<rbrace> B \<lbrace> Q \<rbrace>,\<lbrace> E \<rbrace>! = \<lbrace> P \<rbrace> B \<lbrace> \<lambda>v s. case v of Inl e \<Rightarrow> E e s | Inr r \<Rightarrow> Q r s \<rbrace>!"
-  by (clarsimp simp: validE_NF_def validE_def validNF_def)
-
-(* text \<open>
-  Usually, well-formed monads constructed from the primitives
-  above will have the following property: if they return an
-  empty set of results, they will have the failure flag set.\<close>
-definition empty_fail :: "('s,'a) tmonad \<Rightarrow> bool" where
-  "empty_fail m \<equiv> \<forall>s. fst (m s) = {} \<longrightarrow> snd (m s)"
-
-text \<open>
-  Useful in forcing otherwise unknown executions to have
-  the @{const empty_fail} property.\<close>
-definition mk_ef :: "'a set \<times> bool \<Rightarrow> 'a set \<times> bool" where
-  "mk_ef S \<equiv> (fst S, fst S = {} \<or> snd S)"
- *)
-section "Basic exception reasoning"
-
-text \<open>
-  The predicates @{text no_throw} and @{text no_return} allow us to reason about functions in
-  the exception monad that never throw an exception or never return normally.\<close>
-
-definition no_throw :: "('s \<Rightarrow> bool) \<Rightarrow> ('s, 'e + 'a) tmonad \<Rightarrow> bool" where
-  "no_throw P A \<equiv> \<lbrace> P \<rbrace> A \<lbrace> \<lambda>_ _. True \<rbrace>,\<lbrace> \<lambda>_ _. False \<rbrace>"
-
-definition no_return :: "('a \<Rightarrow> bool) \<Rightarrow> ('a, 'b + 'c) tmonad \<Rightarrow> bool" where
-  "no_return P A \<equiv> \<lbrace> P \<rbrace> A \<lbrace>\<lambda>_ _. False\<rbrace>,\<lbrace>\<lambda>_ _. True \<rbrace>"
-
 section "Trace monad Parallel"
 
 definition parallel :: "('s,'a) tmonad \<Rightarrow> ('s,'a) tmonad \<Rightarrow> ('s,'a) tmonad" where
@@ -899,6 +739,18 @@ next
     apply simp
     done
 qed
+
+text \<open>rg_pred type: Rely-Guaranty predicates (state before => state after => bool)\<close>
+type_synonym 's rg_pred = "'s \<Rightarrow> 's \<Rightarrow> bool"
+
+text \<open>Abbreviations for trivial postconditions (taking three arguments):\<close>
+abbreviation(input)
+  toptoptop :: "'a \<Rightarrow> 'b \<Rightarrow> 'b \<Rightarrow> bool" ("\<top>\<top>\<top>") where
+  "\<top>\<top>\<top> \<equiv> \<lambda>_ _ _. True"
+
+abbreviation(input)
+  botbotbot :: "'a \<Rightarrow> 'b \<Rightarrow> 'b \<Rightarrow> bool" ("\<bottom>\<bottom>\<bottom>") where
+  "\<bottom>\<bottom>\<bottom> \<equiv> \<lambda>_ _ _. False"
 
 definition rely_cond :: "'s rg_pred \<Rightarrow> 's \<Rightarrow> (tmid \<times> 's) list \<Rightarrow> bool" where
   "rely_cond R s0s tr = (\<forall>(ident, s0, s) \<in> trace_steps (rev tr) s0s. ident = Env \<longrightarrow> R s0 s)"
