lib/Monads/trace/Trace_VCG.thy
@@ -1,14 +1,1108 @@
 (*
+ * Copyright 2023, Proofcraft Pty Ltd
  * Copyright 2020, Data61, CSIRO (ABN 41 687 119 230)
  *
  * SPDX-License-Identifier: BSD-2-Clause
  *)
+
 theory Trace_VCG
-imports
-  Trace_Monad
-  Fun_Pred_Syntax
-  WPSimp
+  imports
+    Trace_Lemmas
+    WPSimp
 begin
+
+section \<open>Hoare Logic\<close>
+
+subsection \<open>Validity\<close>
+
+text \<open>
+  This section defines a Hoare logic for partial correctness for
+  the interference trace monad as well as the exception monad.
+  The logic talks only about the behaviour part of the monad and ignores
+  the failure flag.
+
+  The logic is defined semantically. Rules work directly on the
+  validity predicate.
+
+  In the interference trace monad, validity is a triple of precondition,
+  monad, and postcondition. The precondition is a function from state to
+  bool (a state predicate), the postcondition is a function from return value
+  to state to bool. A triple is valid if for all states that satisfy the
+  precondition, all result values and result states that are returned by
+  the monad satisfy the postcondition. Note that if the computation returns
+  the empty set, the triple is trivially valid. This means @{term "assert P"}
+  does not require us to prove that @{term P} holds, but rather allows us
+  to assume @{term P}! Proving non-failure is done via separate predicate and
+  calculus (see below).\<close>
+
+definition valid :: "('s \<Rightarrow> bool) \<Rightarrow> ('s,'a) tmonad \<Rightarrow> ('a \<Rightarrow> 's \<Rightarrow> bool) \<Rightarrow> bool"
+  ("\<lbrace>_\<rbrace>/ _ /\<lbrace>_\<rbrace>") where
+  "\<lbrace>P\<rbrace> f \<lbrace>Q\<rbrace> \<equiv> \<forall>s. P s \<longrightarrow> (\<forall>(r,s') \<in> mres (f s). Q r s')"
+
+text \<open>
+  We often reason about invariant predicates. The following provides shorthand syntax
+  that avoids repeating potentially long predicates.\<close>
+abbreviation (input) invariant ::
+  "('s,'a) tmonad \<Rightarrow> ('s \<Rightarrow> bool) \<Rightarrow> bool" ("_ \<lbrace>_\<rbrace>" [59,0] 60) where
+  "invariant f P \<equiv> \<lbrace>P\<rbrace> f \<lbrace>\<lambda>_. P\<rbrace>"
+
+text \<open>
+  Validity for the exception monad is similar and build on the standard
+  validity above. Instead of one postcondition, we have two: one for
+  normal and one for exceptional results.\<close>
+definition validE ::
+  "('s \<Rightarrow> bool) \<Rightarrow> ('s, 'a + 'b) tmonad \<Rightarrow> ('b \<Rightarrow> 's \<Rightarrow> bool) \<Rightarrow> ('a \<Rightarrow> 's \<Rightarrow> bool) \<Rightarrow> bool"
+  ("\<lbrace>_\<rbrace>/ _ /(\<lbrace>_\<rbrace>,/ \<lbrace>_\<rbrace>)" ) where
+  "\<lbrace>P\<rbrace> f \<lbrace>Q\<rbrace>,\<lbrace>E\<rbrace> \<equiv> \<lbrace>P\<rbrace> f \<lbrace> \<lambda>v s. case v of Inr r \<Rightarrow> Q r s | Inl e \<Rightarrow> E e s \<rbrace>"
+
+lemma validE_def2:
+  "\<lbrace>P\<rbrace> f \<lbrace>Q\<rbrace>,\<lbrace>E\<rbrace> \<equiv> \<forall>s. P s \<longrightarrow> (\<forall>(r,s') \<in> mres (f s). case r of Inr b \<Rightarrow> Q b s' | Inl a \<Rightarrow> E a s')"
+  by (unfold valid_def validE_def)
+(*
+text \<open>Validity for exception monad with interferences. Not as easy to phrase
+ as we need to \<close>
+definition validIE :: "('s, 'a + 'b) tmonad \<Rightarrow>
+             's rg_pred \<Rightarrow>
+             's rg_pred \<Rightarrow> 's rg_pred \<Rightarrow>
+             ('b \<Rightarrow> 's rg_pred) \<Rightarrow>
+             ('a \<Rightarrow> 's rg_pred) \<Rightarrow> bool"
+ ("_ //PRE _//RELY _//GUAR _//POST _//EXC _" [59,0,0,0,0,0] 60) where
+  "validIE f P R G Q E \<equiv> f SAT [P,R,G,\<lambda>v. case v of Inr r \<Rightarrow> Q r | Inl e \<Rightarrow> E e]"
+
+abbreviation (input)
+  validIEsat :: "('s, 'a + 'b) tmonad \<Rightarrow>
+             's rg_pred \<Rightarrow>
+             's rg_pred \<Rightarrow> 's rg_pred \<Rightarrow>
+             ('b \<Rightarrow> 's rg_pred) \<Rightarrow>
+             ('a \<Rightarrow> 's rg_pred) \<Rightarrow> bool"
+  ("_ //SAT [_, _, _, _, _]" [59,0,0,0,0,0] 60)
+  where
+  "validIEsat f P R G Q E \<equiv> validIE f P R G Q E"
+ *)
+text \<open>
+  The following two instantiations are convenient to separate reasoning for exceptional and
+  normal case.\<close>
+(* Narrator: they are in fact not convenient, and are now considered a mistake that should have
+             been an abbreviation instead. *)
+definition validE_R :: (* FIXME lib: this should be an abbreviation *)
+  "('s \<Rightarrow> bool) \<Rightarrow> ('s, 'e + 'a) tmonad \<Rightarrow> ('a \<Rightarrow> 's \<Rightarrow> bool) \<Rightarrow> bool" ("\<lbrace>_\<rbrace>/ _ /\<lbrace>_\<rbrace>, -") where
+  "\<lbrace>P\<rbrace> f \<lbrace>Q\<rbrace>,- \<equiv> validE P f Q (\<lambda>x y. True)"
+
+definition validE_E :: (* FIXME lib: this should be an abbreviation *)
+  "('s \<Rightarrow> bool) \<Rightarrow>  ('s, 'e + 'a) tmonad \<Rightarrow> ('e \<Rightarrow> 's \<Rightarrow> bool) \<Rightarrow> bool" ("\<lbrace>_\<rbrace>/ _ /-, \<lbrace>_\<rbrace>") where
+  "\<lbrace>P\<rbrace> f -,\<lbrace>Q\<rbrace> \<equiv> validE P f (\<lambda>x y. True) Q"
+
+
+section \<open>Lemmas\<close>
+
+lemma hoare_pre_imp:
+  "\<lbrakk> \<And>s. P s \<Longrightarrow> Q s; \<lbrace>Q\<rbrace> a \<lbrace>R\<rbrace> \<rbrakk> \<Longrightarrow> \<lbrace>P\<rbrace> a \<lbrace>R\<rbrace>"
+  by (fastforce simp: valid_def)
+
+lemmas hoare_weaken_pre = hoare_pre_imp[rotated]
+
+lemma hoare_vcg_precond_impE: (* FIXME lib: eliminate in favour of hoare_weaken_preE *)
+  "\<lbrakk> \<lbrace>Q\<rbrace> f \<lbrace>R\<rbrace>,\<lbrace>E\<rbrace>; \<And>s. P s \<Longrightarrow> Q s \<rbrakk> \<Longrightarrow> \<lbrace>P\<rbrace> f \<lbrace>R\<rbrace>,\<lbrace>E\<rbrace>"
+  by (fastforce simp add:validE_def2)
+
+lemmas hoare_weaken_preE = hoare_vcg_precond_impE
+
+lemma hoare_vcg_precond_impE_R: (* FIXME lib: rename to hoare_weaken_preE_R *)
+  "\<lbrakk> \<lbrace>P'\<rbrace> f \<lbrace>Q\<rbrace>,-; \<And>s. P s \<Longrightarrow> P' s \<rbrakk> \<Longrightarrow> \<lbrace>P\<rbrace> f \<lbrace>Q\<rbrace>,-"
+  unfolding validE_R_def
+  by (rule hoare_vcg_precond_impE)
+
+lemma hoare_weaken_preE_E:
+  "\<lbrakk> \<lbrace>P'\<rbrace> f -,\<lbrace>Q\<rbrace>; \<And>s. P s \<Longrightarrow> P' s \<rbrakk> \<Longrightarrow> \<lbrace>P\<rbrace> f -,\<lbrace>Q\<rbrace>"
+  by (fastforce simp add: validE_E_def validE_def valid_def)
+
+lemmas hoare_pre [wp_pre] =
+  hoare_weaken_pre
+  hoare_weaken_preE
+  hoare_vcg_precond_impE_R
+  hoare_weaken_preE_E
+
+
+subsection \<open>Setting up the precondition case splitter.\<close>
+
+lemma wpc_helper_valid:
+  "\<lbrace>Q\<rbrace> g \<lbrace>S\<rbrace> \<Longrightarrow> wpc_helper (P, P', P'') (Q, Q', Q'') \<lbrace>P\<rbrace> g \<lbrace>S\<rbrace>"
+  by (clarsimp simp: wpc_helper_def elim!: hoare_pre)
+
+lemma wpc_helper_validE:
+  "\<lbrace>Q\<rbrace> f \<lbrace>R\<rbrace>,\<lbrace>E\<rbrace> \<Longrightarrow> wpc_helper (P, P', P'') (Q, Q', Q'') \<lbrace>P\<rbrace> f \<lbrace>R\<rbrace>,\<lbrace>E\<rbrace>"
+  by (clarsimp simp: wpc_helper_def elim!: hoare_pre)
+
+lemma wpc_helper_validE_R:
+  "\<lbrace>Q\<rbrace> f \<lbrace>R\<rbrace>,- \<Longrightarrow> wpc_helper (P, P', P'') (Q, Q', Q'') \<lbrace>P\<rbrace> f \<lbrace>R\<rbrace>,-"
+  by (clarsimp simp: wpc_helper_def elim!: hoare_pre)
+
+lemma wpc_helper_validR_R:
+  "\<lbrace>Q\<rbrace> f -,\<lbrace>E\<rbrace> \<Longrightarrow> wpc_helper (P, P', P'') (Q, Q', Q'') \<lbrace>P\<rbrace> f -,\<lbrace>E\<rbrace>"
+  by (clarsimp simp: wpc_helper_def elim!: hoare_pre)
+
+
+wpc_setup "\<lambda>m. \<lbrace>P\<rbrace> m \<lbrace>Q\<rbrace>" wpc_helper_valid
+wpc_setup "\<lambda>m. \<lbrace>P\<rbrace> m \<lbrace>Q\<rbrace>,\<lbrace>E\<rbrace>" wpc_helper_validE
+wpc_setup "\<lambda>m. \<lbrace>P\<rbrace> m \<lbrace>Q\<rbrace>,-" wpc_helper_validE_R
+wpc_setup "\<lambda>m. \<lbrace>P\<rbrace> m -,\<lbrace>E\<rbrace>" wpc_helper_validR_R
+
+
+subsection "Simplification Rules for Lifted And/Or"
+
+lemma bipred_disj_op_eq[simp]:
+  "reflp R \<Longrightarrow> ((=) or R) = R"
+  apply (rule ext, rule ext)
+  apply (auto simp: reflp_def)
+  done
+
+lemma bipred_le_true[simp]: "R \<le> \<top>\<top>"
+  by clarsimp
+
+subsection "Hoare Logic Rules"
+
+lemma bind_wp[wp_split]:
+  "\<lbrakk> \<And>r. \<lbrace>Q' r\<rbrace> g r \<lbrace>Q\<rbrace>; \<lbrace>P\<rbrace>f \<lbrace>Q'\<rbrace> \<rbrakk> \<Longrightarrow> \<lbrace>P\<rbrace> f >>= (\<lambda>rv. g rv) \<lbrace>Q\<rbrace>"
+  by (fastforce simp: valid_def bind_def2 mres_def intro: image_eqI[rotated])
+
+lemma seq':
+  "\<lbrakk> \<lbrace>A\<rbrace> f \<lbrace>B\<rbrace>; \<forall>x. P x \<longrightarrow> \<lbrace>C\<rbrace> g x \<lbrace>D\<rbrace>; \<forall>x s. B x s \<longrightarrow> P x \<and> C s \<rbrakk> \<Longrightarrow>
+   \<lbrace>A\<rbrace> do x \<leftarrow> f; g x od \<lbrace>D\<rbrace>"
+  apply (erule bind_wp[rotated])
+  apply (clarsimp simp: valid_def)
+  apply (fastforce elim: rev_bexI image_eqI[rotated])
+  done
+
+lemma seq:
+  assumes f_valid: "\<lbrace>A\<rbrace> f \<lbrace>B\<rbrace>"
+  assumes g_valid: "\<And>x. P x \<Longrightarrow> \<lbrace>C\<rbrace> g x \<lbrace>D\<rbrace>"
+  assumes bind:  "\<And>x s. B x s \<Longrightarrow> P x \<and> C s"
+  shows "\<lbrace>A\<rbrace> do x \<leftarrow> f; g x od \<lbrace>D\<rbrace>"
+  apply (insert f_valid g_valid bind)
+  apply (blast intro: seq')
+  done
+
+lemma seq_ext':
+  "\<lbrakk> \<lbrace>A\<rbrace> f \<lbrace>B\<rbrace>; \<forall>x. \<lbrace>B x\<rbrace> g x \<lbrace>C\<rbrace> \<rbrakk> \<Longrightarrow>
+   \<lbrace>A\<rbrace> do x \<leftarrow> f; g x od \<lbrace>C\<rbrace>"
+  by (metis bind_wp)
+
+lemmas seq_ext = bind_wp[rotated]
+
+lemma seqE':
+  "\<lbrakk> \<lbrace>A\<rbrace> f \<lbrace>B\<rbrace>,\<lbrace>E\<rbrace>; \<forall>x. \<lbrace>B x\<rbrace> g x \<lbrace>C\<rbrace>,\<lbrace>E\<rbrace> \<rbrakk> \<Longrightarrow>
+   \<lbrace>A\<rbrace> doE x \<leftarrow> f; g x odE \<lbrace>C\<rbrace>,\<lbrace>E\<rbrace>"
+  apply (simp add: bindE_def validE_def)
+  apply (erule seq_ext')
+  apply (auto simp: lift_def valid_def throwError_def return_def mres_def
+             split: sum.splits)
+  done
+
+lemma seqE:
+  assumes f_valid: "\<lbrace>A\<rbrace> f \<lbrace>B\<rbrace>,\<lbrace>E\<rbrace>"
+  assumes g_valid: "\<And>x. \<lbrace>B x\<rbrace> g x \<lbrace>C\<rbrace>,\<lbrace>E\<rbrace>"
+  shows "\<lbrace>A\<rbrace> doE x \<leftarrow> f; g x odE \<lbrace>C\<rbrace>,\<lbrace>E\<rbrace>"
+  apply (insert f_valid g_valid)
+  apply (blast intro: seqE')
+  done
+
+lemma hoare_TrueI:
+  "\<lbrace>P\<rbrace> f \<lbrace>\<lambda>_. \<top>\<rbrace>"
+  by (simp add: valid_def)
+
+lemma hoareE_TrueI:
+  "\<lbrace>P\<rbrace> f \<lbrace>\<lambda>_. \<top>\<rbrace>, \<lbrace>\<lambda>r. \<top>\<rbrace>"
+  by (simp add: validE_def valid_def)
+
+lemma hoare_True_E_R[simp]:
+  "\<lbrace>P\<rbrace> f \<lbrace>\<lambda>_ s. True\<rbrace>, -"
+  by (auto simp: validE_R_def validE_def valid_def split: sum.splits)
+
+lemma hoare_post_conj[intro]:
+  "\<lbrakk> \<lbrace>P\<rbrace> f \<lbrace>Q\<rbrace>; \<lbrace>P\<rbrace> f \<lbrace>R\<rbrace> \<rbrakk> \<Longrightarrow> \<lbrace>P\<rbrace> f \<lbrace>Q and R\<rbrace>"
+  by (fastforce simp: valid_def)
+
+lemma hoare_pre_disj[intro]:
+  "\<lbrakk> \<lbrace>P\<rbrace> f \<lbrace>R\<rbrace>; \<lbrace>Q\<rbrace> f \<lbrace>R\<rbrace> \<rbrakk> \<Longrightarrow> \<lbrace>P or Q\<rbrace> f \<lbrace>R\<rbrace>"
+  by (simp add:valid_def pred_disj_def)
+
+lemma hoare_conj:
+  "\<lbrakk> \<lbrace>P\<rbrace> f \<lbrace>Q\<rbrace>; \<lbrace>P'\<rbrace> f \<lbrace>Q'\<rbrace> \<rbrakk> \<Longrightarrow> \<lbrace>P and P'\<rbrace> f \<lbrace>Q and Q'\<rbrace>"
+  unfolding valid_def by auto
+
+lemmas hoare_post_taut = hoare_TrueI (* FIXME lib: eliminate *)
+
+lemmas wp_post_taut = hoare_TrueI[where P=\<top>]
+lemmas wp_post_tautE = hoareE_TrueI[where P=\<top>]
+
+lemma hoare_pre_cont[simp]:
+  "\<lbrace>\<bottom>\<rbrace> f \<lbrace>P\<rbrace>"
+  by (simp add:valid_def)
+
+lemma hoare_return_drop_var[iff]:
+  "\<lbrace>Q\<rbrace> return x \<lbrace>\<lambda>r. Q\<rbrace>"
+  by (simp add: valid_def return_def mres_def)
+
+lemma hoare_gets[intro]:
+  "\<lbrakk> \<And>s. P s \<Longrightarrow> Q (f s) s \<rbrakk> \<Longrightarrow> \<lbrace>P\<rbrace> gets f \<lbrace>Q\<rbrace>"
+  by (simp add:valid_def gets_def get_def bind_def return_def mres_def)
+
+lemma hoare_modifyE_var:
+  "\<lbrakk> \<And>s. P s \<Longrightarrow> Q (f s) \<rbrakk> \<Longrightarrow> \<lbrace>P\<rbrace> modify f \<lbrace>\<lambda>_ s. Q s\<rbrace>"
+  by(simp add: valid_def modify_def put_def get_def bind_def mres_def)
+
+lemma hoare_if:
+  "\<lbrakk> P \<Longrightarrow> \<lbrace>Q\<rbrace> a \<lbrace>R\<rbrace>; \<not> P \<Longrightarrow> \<lbrace>Q\<rbrace> b \<lbrace>R\<rbrace> \<rbrakk> \<Longrightarrow> \<lbrace>Q\<rbrace> if P then a else b \<lbrace>R\<rbrace>"
+  by (simp add: valid_def)
+
+lemma hoare_pre_subst:
+  "\<lbrakk> A = B; \<lbrace>A\<rbrace> a \<lbrace>C\<rbrace> \<rbrakk> \<Longrightarrow> \<lbrace>B\<rbrace> a \<lbrace>C\<rbrace>"
+  by (erule subst)
+
+lemma hoare_post_subst:
+  "\<lbrakk> B = C; \<lbrace>A\<rbrace> a \<lbrace>B\<rbrace> \<rbrakk> \<Longrightarrow> \<lbrace>A\<rbrace> a \<lbrace>C\<rbrace>"
+  by (erule subst)
+
+lemma hoare_post_imp:
+  "\<lbrakk> \<And>rv s. Q rv s \<Longrightarrow> R rv s; \<lbrace>P\<rbrace> a \<lbrace>Q\<rbrace> \<rbrakk> \<Longrightarrow> \<lbrace>P\<rbrace> a \<lbrace>R\<rbrace>"
+  by(fastforce simp:valid_def split_def)
+
+lemma hoare_post_impErr': (* FIXME lib: eliminate *)
+  "\<lbrakk> \<lbrace>P\<rbrace> a \<lbrace>Q\<rbrace>,\<lbrace>E\<rbrace>; \<forall>rv s. Q rv s \<longrightarrow> R rv s; \<forall>e s. E e s \<longrightarrow> F e s \<rbrakk> \<Longrightarrow> \<lbrace>P\<rbrace> a \<lbrace>R\<rbrace>,\<lbrace>F\<rbrace>"
+  unfolding validE_def valid_def
+  by (fastforce split: sum.splits)
+
+lemma hoare_post_impErr:
+  "\<lbrakk> \<lbrace>P\<rbrace> a \<lbrace>Q\<rbrace>,\<lbrace>E\<rbrace>; \<And>rv s. Q rv s \<Longrightarrow> R rv s; \<And>e s. E e s \<Longrightarrow> F e s \<rbrakk> \<Longrightarrow> \<lbrace>P\<rbrace> a \<lbrace>R\<rbrace>,\<lbrace>F\<rbrace>"
+  by (blast intro: hoare_post_impErr')
+
+lemma hoare_validE_cases:
+  "\<lbrakk> \<lbrace>P\<rbrace> f \<lbrace>Q\<rbrace>, \<lbrace>\<lambda>_ _. True\<rbrace>; \<lbrace>P\<rbrace> f \<lbrace>\<lambda>_ _. True\<rbrace>, \<lbrace>R\<rbrace> \<rbrakk> \<Longrightarrow> \<lbrace>P\<rbrace> f \<lbrace>Q\<rbrace>, \<lbrace>R\<rbrace>"
+  by (fastforce simp: validE_def valid_def split: sum.splits)
+
+lemma hoare_post_imp_dc:
+  "\<lbrakk>\<lbrace>P\<rbrace> a \<lbrace>\<lambda>_. Q\<rbrace>; \<And>s. Q s \<Longrightarrow> R s\<rbrakk> \<Longrightarrow> \<lbrace>P\<rbrace> a \<lbrace>\<lambda>_. R\<rbrace>, \<lbrace>\<lambda>_. R\<rbrace>"
+  by (fastforce simp: validE_def valid_def split: sum.splits)
+
+lemma hoare_post_imp_dc2:
+  "\<lbrakk>\<lbrace>P\<rbrace> a \<lbrace>\<lambda>_. Q\<rbrace>; \<And>s. Q s \<Longrightarrow> R s\<rbrakk> \<Longrightarrow> \<lbrace>P\<rbrace> a \<lbrace>\<lambda>_. R\<rbrace>, \<lbrace>\<lambda>_. \<top>\<rbrace>"
+  by (fastforce simp: validE_def valid_def split: sum.splits)
+
+lemma hoare_post_imp_dc2E:
+  "\<lbrakk>\<lbrace>P\<rbrace> a \<lbrace>\<lambda>_. Q\<rbrace>; \<And>s. Q s \<Longrightarrow> R s\<rbrakk> \<Longrightarrow> \<lbrace>P\<rbrace> a \<lbrace>\<lambda>_. \<top>\<rbrace>, \<lbrace>\<lambda>_. R\<rbrace>"
+  by (fastforce simp: validE_def valid_def split: sum.splits)
+
+lemma hoare_post_imp_dc2_actual:
+  "\<lbrace>P\<rbrace> a \<lbrace>\<lambda>_. R\<rbrace> \<Longrightarrow> \<lbrace>P\<rbrace> a \<lbrace>\<lambda>_. R\<rbrace>, \<lbrace>\<lambda>_. \<top>\<rbrace>"
+  by (rule hoare_post_imp_dc2)
+
+lemma hoare_post_imp_dc2E_actual:
+  "\<lbrace>P\<rbrace> a \<lbrace>\<lambda>_. R\<rbrace> \<Longrightarrow> \<lbrace>P\<rbrace> a \<lbrace>\<lambda>_. \<top>\<rbrace>, \<lbrace>\<lambda>_. R\<rbrace>"
+  by (rule hoare_post_imp_dc2E)
+
+lemmas hoare_post_impE = hoare_post_imp (* FIXME lib: eliminate; probably should be on validE *)
+
+lemma hoare_conjD1:
+  "\<lbrace>P\<rbrace> f \<lbrace>\<lambda>rv. Q rv and R rv\<rbrace> \<Longrightarrow> \<lbrace>P\<rbrace> f \<lbrace>\<lambda>rv. Q rv\<rbrace>"
+  unfolding valid_def by auto
+
+lemma hoare_conjD2:
+  "\<lbrace>P\<rbrace> f \<lbrace>\<lambda>rv. Q rv and R rv\<rbrace> \<Longrightarrow> \<lbrace>P\<rbrace> f \<lbrace>\<lambda>rv. R rv\<rbrace>"
+  unfolding valid_def by auto
+
+lemma hoare_post_disjI1:
+  "\<lbrace>P\<rbrace> f \<lbrace>\<lambda>rv. Q rv\<rbrace> \<Longrightarrow> \<lbrace>P\<rbrace> f \<lbrace>\<lambda>rv. Q rv or R rv\<rbrace>"
+  unfolding valid_def by auto
+
+lemma hoare_post_disjI2:
+  "\<lbrace>P\<rbrace> f \<lbrace>\<lambda>rv. R rv\<rbrace> \<Longrightarrow> \<lbrace>P\<rbrace> f \<lbrace>\<lambda>rv. Q rv or R rv\<rbrace>"
+  unfolding valid_def by auto
+
+lemmas hoare_strengthen_post = hoare_post_imp[rotated]
+
+lemma use_valid:
+  "\<lbrakk>(r, s') \<in> mres (f s); \<lbrace>P\<rbrace> f \<lbrace>Q\<rbrace>; P s \<rbrakk> \<Longrightarrow> Q r s'"
+  unfolding valid_def by blast
+
+lemmas post_by_hoare = use_valid[rotated]
+
+lemma use_validE_norm:
+  "\<lbrakk> (Inr r', s') \<in> mres (B s); \<lbrace>P\<rbrace> B \<lbrace>Q\<rbrace>,\<lbrace> E \<rbrace>; P s \<rbrakk> \<Longrightarrow> Q r' s'"
+  unfolding validE_def valid_def by force
+
+lemma use_validE_except:
+  "\<lbrakk> (Inl r', s') \<in> mres (B s); \<lbrace>P\<rbrace> B \<lbrace>Q\<rbrace>,\<lbrace> E \<rbrace>; P s \<rbrakk> \<Longrightarrow> E r' s'"
+  unfolding validE_def valid_def by force
+
+lemma in_inv_by_hoareD:
+  "\<lbrakk> \<And>P. f \<lbrace>P\<rbrace>; (x,s') \<in> mres (f s) \<rbrakk> \<Longrightarrow> s' = s"
+  by (auto simp add: valid_def) blast
+
+
+subsection \<open>Misc\<close>
+
+lemma hoare_return_simp:
+  "\<lbrace>P\<rbrace> return x \<lbrace>Q\<rbrace> = (\<forall>s. P s \<longrightarrow> Q x s)"
+  by (simp add: valid_def return_def mres_def)
+
+lemma hoare_gen_asm:
+  "(P \<Longrightarrow> \<lbrace>P'\<rbrace> f \<lbrace>Q\<rbrace>) \<Longrightarrow> \<lbrace>P' and K P\<rbrace> f \<lbrace>Q\<rbrace>"
+  by (fastforce simp add: valid_def)
+
+lemma hoare_conjI:
+  "\<lbrakk> \<lbrace>P\<rbrace> f \<lbrace>Q\<rbrace>; \<lbrace>P\<rbrace> f \<lbrace>R\<rbrace> \<rbrakk> \<Longrightarrow> \<lbrace>P\<rbrace> f \<lbrace>\<lambda>r s. Q r s \<and> R r s\<rbrace>"
+  unfolding valid_def by blast
+
+lemma hoare_disjI1:
+  "\<lbrakk> \<lbrace>P\<rbrace> f \<lbrace>Q\<rbrace> \<rbrakk> \<Longrightarrow> \<lbrace>P\<rbrace> f \<lbrace>\<lambda>rv s. Q rv s \<or>  R rv s \<rbrace>"
+  unfolding valid_def by blast
+
+lemma hoare_disjI2:
+  "\<lbrakk> \<lbrace>P\<rbrace> f \<lbrace>R\<rbrace> \<rbrakk> \<Longrightarrow> \<lbrace>P\<rbrace> f \<lbrace>\<lambda>rv s. Q rv s \<or>  R rv s \<rbrace>"
+  unfolding valid_def by blast
+
+lemma hoare_assume_pre:
+  "(\<And>s. P s \<Longrightarrow> \<lbrace>P\<rbrace> f \<lbrace>Q\<rbrace>) \<Longrightarrow> \<lbrace>P\<rbrace> f \<lbrace>Q\<rbrace>"
+  by (auto simp: valid_def)
+
+lemma hoare_assume_preE:
+  "(\<And>s. P s \<Longrightarrow> \<lbrace>P\<rbrace> f \<lbrace>Q\<rbrace>,\<lbrace>R\<rbrace>) \<Longrightarrow> \<lbrace>P\<rbrace> f \<lbrace>Q\<rbrace>,\<lbrace>R\<rbrace>"
+  by (auto simp: valid_def validE_def)
+
+lemma hoare_allI:
+  "(\<And>x. \<lbrace>P\<rbrace>f\<lbrace>Q x\<rbrace>) \<Longrightarrow> \<lbrace>P\<rbrace>f\<lbrace>\<lambda>rv s. \<forall>x. Q x rv s\<rbrace>"
+  by (simp add: valid_def) blast
+
+lemma validE_allI:
+  "(\<And>x. \<lbrace>P\<rbrace> f \<lbrace>\<lambda>r s. Q x r s\<rbrace>,\<lbrace>E\<rbrace>) \<Longrightarrow> \<lbrace>P\<rbrace> f \<lbrace>\<lambda>rv s. \<forall>x. Q x rv s\<rbrace>,\<lbrace>E\<rbrace>"
+  by (fastforce simp: valid_def validE_def split: sum.splits)
+
+lemma hoare_exI:
+  "\<lbrace>P\<rbrace> f \<lbrace>Q x\<rbrace> \<Longrightarrow> \<lbrace>P\<rbrace> f \<lbrace>\<lambda>rv s. \<exists>x. Q x rv s\<rbrace>"
+  by (simp add: valid_def) blast
+
+lemma hoare_impI:
+  "(R \<Longrightarrow> \<lbrace>P\<rbrace> f \<lbrace>Q\<rbrace>) \<Longrightarrow> \<lbrace>P\<rbrace> f \<lbrace>\<lambda>rv s. R \<longrightarrow> Q rv s\<rbrace>"
+  by (simp add: valid_def) blast
+
+lemma validE_impI:
+  "\<lbrakk>\<And>E. \<lbrace>P\<rbrace> f \<lbrace>\<lambda>_ _. True\<rbrace>,\<lbrace>E\<rbrace>; (P' \<Longrightarrow> \<lbrace>P\<rbrace> f \<lbrace>Q\<rbrace>,\<lbrace>E\<rbrace>)\<rbrakk> \<Longrightarrow>
+   \<lbrace>P\<rbrace> f \<lbrace>\<lambda>rv s. P' \<longrightarrow> Q rv s\<rbrace>, \<lbrace>E\<rbrace>"
+  by (fastforce simp: validE_def valid_def split: sum.splits)
+
+lemma hoare_case_option_wp:
+  "\<lbrakk> \<lbrace>P\<rbrace> f None \<lbrace>Q\<rbrace>; \<And>x.  \<lbrace>P' x\<rbrace> f (Some x) \<lbrace>Q' x\<rbrace> \<rbrakk>
+  \<Longrightarrow> \<lbrace>case_option P P' v\<rbrace> f v \<lbrace>\<lambda>rv. case v of None \<Rightarrow> Q rv | Some x \<Rightarrow> Q' x rv\<rbrace>"
+  by (cases v) auto
+
+lemma hoare_vcg_prop:
+  "\<lbrace>\<lambda>s. P\<rbrace> f \<lbrace>\<lambda>rv s. P\<rbrace>"
+  by (simp add: valid_def)
+
+
+subsection \<open>@{const valid} and @{const validE}, @{const validE_R}, @{const validE_E}\<close>
+
+lemma valid_validE:
+  "\<lbrace>P\<rbrace> f \<lbrace>\<lambda>_. Q\<rbrace> \<Longrightarrow> \<lbrace>P\<rbrace> f \<lbrace>\<lambda>_. Q\<rbrace>, \<lbrace>\<lambda>_. Q\<rbrace>"
+  by (rule hoare_post_imp_dc)
+
+lemma valid_validE2:
+  "\<lbrakk> \<lbrace>P\<rbrace> f \<lbrace>\<lambda>_. Q'\<rbrace>; \<And>s. Q' s \<Longrightarrow> Q s; \<And>s. Q' s \<Longrightarrow> E s \<rbrakk> \<Longrightarrow> \<lbrace>P\<rbrace> f \<lbrace>\<lambda>_. Q\<rbrace>, \<lbrace>\<lambda>_. E\<rbrace>"
+  unfolding valid_def validE_def
+  by (clarsimp split: sum.splits) blast
+
+lemma validE_valid:
+  "\<lbrace>P\<rbrace> f \<lbrace>\<lambda>_. Q\<rbrace>, \<lbrace>\<lambda>_. Q\<rbrace> \<Longrightarrow> \<lbrace>P\<rbrace> f \<lbrace>\<lambda>_. Q\<rbrace>"
+  unfolding validE_def valid_def
+  by fastforce
+
+lemma valid_validE_R:
+  "\<lbrace>P\<rbrace> f \<lbrace>\<lambda>_. Q\<rbrace> \<Longrightarrow> \<lbrace>P\<rbrace> f \<lbrace>\<lambda>_. Q\<rbrace>,-"
+  by (simp add: validE_R_def hoare_post_impErr [OF valid_validE])
+
+lemma valid_validE_E:
+  "\<lbrace>P\<rbrace> f \<lbrace>\<lambda>_. Q\<rbrace> \<Longrightarrow> \<lbrace>P\<rbrace> f -,\<lbrace>\<lambda>_. Q\<rbrace>"
+  by (simp add: validE_E_def hoare_post_impErr [OF valid_validE])
+
+lemma validE_validE_R:
+  "\<lbrace>P\<rbrace> f \<lbrace>Q\<rbrace>,\<lbrace>\<top>\<top>\<rbrace> \<Longrightarrow> \<lbrace>P\<rbrace> f \<lbrace>Q\<rbrace>,-"
+  by (simp add: validE_R_def)
+
+lemma validE_R_validE:
+  "\<lbrace>P\<rbrace> f \<lbrace>Q\<rbrace>,- \<Longrightarrow> \<lbrace>P\<rbrace> f \<lbrace>Q\<rbrace>,\<lbrace>\<top>\<top>\<rbrace>"
+  by (simp add: validE_R_def)
+
+lemma validE_validE_E:
+  "\<lbrace>P\<rbrace> f \<lbrace>\<top>\<top>\<rbrace>, \<lbrace>E\<rbrace> \<Longrightarrow> \<lbrace>P\<rbrace> f -, \<lbrace>E\<rbrace>"
+  by (simp add: validE_E_def)
+
+lemma validE_E_validE:
+  "\<lbrace>P\<rbrace> f -, \<lbrace>E\<rbrace> \<Longrightarrow> \<lbrace>P\<rbrace> f \<lbrace>\<top>\<top>\<rbrace>, \<lbrace>E\<rbrace>"
+  by (simp add: validE_E_def)
+
+
+subsection \<open>@{const liftM}\<close>
+
+lemma in_image_constant:
+  "(x \<in> (\<lambda>_. v) ` S) = (x = v \<and> S \<noteq> {})"
+  by (simp add: image_constant_conv)
+
+lemma hoare_liftM_subst:
+  "\<lbrace>P\<rbrace> liftM f m \<lbrace>Q\<rbrace> = \<lbrace>P\<rbrace> m \<lbrace>Q \<circ> f\<rbrace>"
+  apply (simp add: liftM_def bind_def2 return_def split_def)
+  apply (simp add: valid_def Ball_def mres_def image_Un)
+  apply (simp add: image_image in_image_constant)
+  apply force
+  done
+
+lemma hoare_liftME_subst:
+  "\<lbrace>P\<rbrace> liftME f m \<lbrace>Q\<rbrace>, \<lbrace>E\<rbrace> = \<lbrace>P\<rbrace> m \<lbrace>Q \<circ> f\<rbrace>, \<lbrace>E\<rbrace>"
+  unfolding validE_def liftME_liftM hoare_liftM_subst o_def
+  by (fastforce intro!: arg_cong[where f="valid P m"] split: sum.splits)
+
+lemma liftE_validE[simp]:
+  "\<lbrace>P\<rbrace> liftE f \<lbrace>Q\<rbrace>, \<lbrace>E\<rbrace> = \<lbrace>P\<rbrace> f \<lbrace>Q\<rbrace>"
+  by (simp add: liftE_liftM validE_def hoare_liftM_subst o_def)
+
+
+subsection \<open>Operator lifting/splitting\<close>
+
+lemma hoare_vcg_if_split:
+  "\<lbrakk> P \<Longrightarrow> \<lbrace>Q\<rbrace> f \<lbrace>S\<rbrace>; \<not>P \<Longrightarrow> \<lbrace>R\<rbrace> g \<lbrace>S\<rbrace> \<rbrakk> \<Longrightarrow> \<lbrace>\<lambda>s. (P \<longrightarrow> Q s) \<and> (\<not>P \<longrightarrow> R s)\<rbrace> if P then f else g \<lbrace>S\<rbrace>"
+  by simp
+
+lemma hoare_vcg_if_splitE:
+  "\<lbrakk> P \<Longrightarrow> \<lbrace>Q\<rbrace> f \<lbrace>S\<rbrace>,\<lbrace>E\<rbrace>; \<not>P \<Longrightarrow> \<lbrace>R\<rbrace> g \<lbrace>S\<rbrace>,\<lbrace>E\<rbrace> \<rbrakk> \<Longrightarrow>
+   \<lbrace>\<lambda>s. (P \<longrightarrow> Q s) \<and> (\<not>P \<longrightarrow> R s)\<rbrace> if P then f else g \<lbrace>S\<rbrace>,\<lbrace>E\<rbrace>"
+  by simp
+
+lemma hoare_vcg_split_case_option:
+ "\<lbrakk> \<And>x. x = None \<Longrightarrow> \<lbrace>P x\<rbrace> f x \<lbrace>R x\<rbrace>; \<And>x y. x = Some y \<Longrightarrow> \<lbrace>Q x y\<rbrace> g x y \<lbrace>R x\<rbrace> \<rbrakk> \<Longrightarrow>
+  \<lbrace>\<lambda>s. (x = None \<longrightarrow> P x s) \<and> (\<forall>y. x = Some y \<longrightarrow> Q x y s)\<rbrace>
+  case x of None \<Rightarrow> f x | Some y \<Rightarrow> g x y
+  \<lbrace>R x\<rbrace>"
+  by (cases x; simp)
+
+lemma hoare_vcg_split_case_optionE:
+  "\<lbrakk> \<And>x. x = None \<Longrightarrow> \<lbrace>P x\<rbrace> f x \<lbrace>R x\<rbrace>,\<lbrace>E x\<rbrace>; \<And>x y. x = Some y \<Longrightarrow> \<lbrace>Q x y\<rbrace> g x y \<lbrace>R x\<rbrace>,\<lbrace>E x\<rbrace> \<rbrakk> \<Longrightarrow>
+   \<lbrace>\<lambda>s. (x = None \<longrightarrow> P x s) \<and> (\<forall>y. x = Some y \<longrightarrow> Q x y s)\<rbrace>
+   case x of None \<Rightarrow> f x | Some y \<Rightarrow> g x y
+   \<lbrace>R x\<rbrace>, \<lbrace>E x\<rbrace>"
+  by (cases x; simp)
+
+lemma hoare_vcg_split_case_sum:
+ "\<lbrakk> \<And>x a. x = Inl a \<Longrightarrow> \<lbrace>P x a\<rbrace> f x a \<lbrace>R x\<rbrace>; \<And>x b. x = Inr b \<Longrightarrow> \<lbrace>Q x b\<rbrace> g x b \<lbrace>R x\<rbrace> \<rbrakk> \<Longrightarrow>
+  \<lbrace>\<lambda>s. (\<forall>a. x = Inl a \<longrightarrow> P x a s) \<and> (\<forall>b. x = Inr b \<longrightarrow> Q x b s) \<rbrace>
+  case x of Inl a \<Rightarrow> f x a | Inr b \<Rightarrow> g x b
+  \<lbrace>R x\<rbrace>"
+  by (cases x; simp)
+
+lemmas hoare_vcg_precond_imp = hoare_weaken_pre (* FIXME lib: eliminate *)
+
+lemmas hoare_seq_ext = seq_ext[rotated]
+lemmas hoare_vcg_seqE = seqE[rotated]
+
+lemma hoare_seq_ext_nobind:
+  "\<lbrakk> \<lbrace>B\<rbrace> g \<lbrace>C\<rbrace>; \<lbrace>A\<rbrace> f \<lbrace>\<lambda>_. B\<rbrace> \<rbrakk> \<Longrightarrow> \<lbrace>A\<rbrace> do f; g od \<lbrace>C\<rbrace>"
+  by (erule seq_ext) (clarsimp simp: valid_def)
+
+lemma hoare_seq_ext_nobindE:
+  "\<lbrakk> \<lbrace>B\<rbrace> g \<lbrace>C\<rbrace>, \<lbrace>E\<rbrace>; \<lbrace>A\<rbrace> f \<lbrace>\<lambda>_. B\<rbrace>, \<lbrace>E\<rbrace> \<rbrakk> \<Longrightarrow> \<lbrace>A\<rbrace> doE f; g odE \<lbrace>C\<rbrace>, \<lbrace>E\<rbrace>"
+  by (erule seqE) (clarsimp simp: validE_def)
+
+lemmas hoare_seq_ext_skip' = hoare_seq_ext[where Q'=Q and Q=Q for Q]
+
+lemma hoare_chain:
+  "\<lbrakk> \<lbrace>P\<rbrace> f \<lbrace>Q\<rbrace>; \<And>s. R s \<Longrightarrow> P s; \<And>rv s. Q rv s \<Longrightarrow> S rv s \<rbrakk> \<Longrightarrow> \<lbrace>R\<rbrace> f \<lbrace>S\<rbrace>"
+  by (wp_pre, rule hoare_post_imp)
+
+lemma validE_weaken: (* FIXME lib: eliminate in favour of hoare_chainE *)
+  "\<lbrakk> \<lbrace>P'\<rbrace> A \<lbrace>Q'\<rbrace>,\<lbrace>E'\<rbrace>; \<And>s. P s \<Longrightarrow> P' s; \<And>rv s. Q' rv s \<Longrightarrow> Q rv s; \<And>rv s. E' rv s \<Longrightarrow> E rv s \<rbrakk>
+   \<Longrightarrow> \<lbrace>P\<rbrace> A \<lbrace>Q\<rbrace>,\<lbrace>E\<rbrace>"
+  by wp_pre (rule hoare_post_impErr)
+
+lemmas hoare_chainE = validE_weaken
+
+lemma hoare_vcg_conj_lift:
+  "\<lbrakk> \<lbrace>P\<rbrace> f \<lbrace>Q\<rbrace>; \<lbrace>P'\<rbrace> f \<lbrace>Q'\<rbrace> \<rbrakk> \<Longrightarrow> \<lbrace>\<lambda>s. P s \<and> P' s\<rbrace> f \<lbrace>\<lambda>rv s. Q rv s \<and> Q' rv s\<rbrace>"
+  unfolding valid_def
+  by fastforce
+
+lemma hoare_vcg_conj_liftE1:
+  "\<lbrakk> \<lbrace>P\<rbrace> f \<lbrace>Q\<rbrace>,-; \<lbrace>P'\<rbrace> f \<lbrace>Q'\<rbrace>,\<lbrace>E\<rbrace> \<rbrakk> \<Longrightarrow> \<lbrace>P and P'\<rbrace> f \<lbrace>\<lambda>rv s. Q rv s \<and> Q' rv s\<rbrace>,\<lbrace>E\<rbrace>"
+  unfolding valid_def validE_R_def validE_def
+  by (fastforce simp: split_def split: sum.splits)
+
+lemma hoare_vcg_disj_lift:
+  "\<lbrakk> \<lbrace>P\<rbrace> f \<lbrace>Q\<rbrace>; \<lbrace>P'\<rbrace> f \<lbrace>Q'\<rbrace> \<rbrakk> \<Longrightarrow> \<lbrace>\<lambda>s. P s \<or> P' s\<rbrace> f \<lbrace>\<lambda>rv s. Q rv s \<or> Q' rv s\<rbrace>"
+  unfolding valid_def
+  by fastforce
+
+lemma hoare_vcg_const_Ball_lift:
+  "\<lbrakk> \<And>x. x \<in> S \<Longrightarrow> \<lbrace>P x\<rbrace> f \<lbrace>Q x\<rbrace> \<rbrakk> \<Longrightarrow> \<lbrace>\<lambda>s. \<forall>x\<in>S. P x s\<rbrace> f \<lbrace>\<lambda>rv s. \<forall>x\<in>S. Q x rv s\<rbrace>"
+  by (fastforce simp: valid_def)
+
+lemma hoare_vcg_const_Ball_lift_R:
+ "\<lbrakk> \<And>x. x \<in> S \<Longrightarrow> \<lbrace>P x\<rbrace> f \<lbrace>Q x\<rbrace>,- \<rbrakk> \<Longrightarrow> \<lbrace>\<lambda>s. \<forall>x \<in> S. P x s\<rbrace> f \<lbrace>\<lambda>rv s. \<forall>x \<in> S. Q x rv s\<rbrace>,-"
+  unfolding validE_R_def validE_def
+  by (rule hoare_strengthen_post)
+     (fastforce intro!: hoare_vcg_const_Ball_lift split: sum.splits)+
+
+lemma hoare_vcg_all_lift:
+  "\<lbrakk> \<And>x. \<lbrace>P x\<rbrace> f \<lbrace>Q x\<rbrace> \<rbrakk> \<Longrightarrow> \<lbrace>\<lambda>s. \<forall>x. P x s\<rbrace> f \<lbrace>\<lambda>rv s. \<forall>x. Q x rv s\<rbrace>"
+  by (fastforce simp: valid_def)
+
+lemma hoare_vcg_all_lift_R:
+  "(\<And>x. \<lbrace>P x\<rbrace> f \<lbrace>Q x\<rbrace>, -) \<Longrightarrow> \<lbrace>\<lambda>s. \<forall>x. P x s\<rbrace> f \<lbrace>\<lambda>rv s. \<forall>x. Q x rv s\<rbrace>, -"
+  by (rule hoare_vcg_const_Ball_lift_R[where S=UNIV, simplified])
+
+lemma hoare_vcg_const_imp_lift:
+  "\<lbrakk> P \<Longrightarrow> \<lbrace>Q\<rbrace> m \<lbrace>R\<rbrace> \<rbrakk> \<Longrightarrow> \<lbrace>\<lambda>s. P \<longrightarrow> Q s\<rbrace> m \<lbrace>\<lambda>rv s. P \<longrightarrow> R rv s\<rbrace>"
+  by (cases P, simp_all add: hoare_vcg_prop)
+
+lemma hoare_vcg_const_imp_lift_R:
+  "(P \<Longrightarrow> \<lbrace>Q\<rbrace> m \<lbrace>R\<rbrace>,-) \<Longrightarrow> \<lbrace>\<lambda>s. P \<longrightarrow> Q s\<rbrace> m \<lbrace>\<lambda>rv s. P \<longrightarrow> R rv s\<rbrace>,-"
+  by (fastforce simp: validE_R_def validE_def valid_def split_def split: sum.splits)
+
+lemma hoare_weak_lift_imp:
+  "\<lbrace>P'\<rbrace> f \<lbrace>Q\<rbrace> \<Longrightarrow> \<lbrace>\<lambda>s. P \<longrightarrow> P' s\<rbrace> f \<lbrace>\<lambda>rv s. P \<longrightarrow> Q rv s\<rbrace>"
+  by (auto simp add: valid_def split_def)
+
+lemma hoare_vcg_ex_lift:
+  "\<lbrakk> \<And>x. \<lbrace>P x\<rbrace> f \<lbrace>Q x\<rbrace> \<rbrakk> \<Longrightarrow> \<lbrace>\<lambda>s. \<exists>x. P x s\<rbrace> f \<lbrace>\<lambda>rv s. \<exists>x. Q x rv s\<rbrace>"
+  by (clarsimp simp: valid_def, blast)
+
+lemma hoare_vcg_ex_lift_R1:
+  "(\<And>x. \<lbrace>P x\<rbrace> f \<lbrace>Q\<rbrace>, -) \<Longrightarrow> \<lbrace>\<lambda>s. \<exists>x. P x s\<rbrace> f \<lbrace>Q\<rbrace>, -"
+  by (fastforce simp: valid_def validE_R_def validE_def split: sum.splits)
+
+(* for instantiations *)
+lemma hoare_triv:    "\<lbrace>P\<rbrace>f\<lbrace>Q\<rbrace> \<Longrightarrow> \<lbrace>P\<rbrace>f\<lbrace>Q\<rbrace>" .
+lemma hoare_trivE:   "\<lbrace>P\<rbrace> f \<lbrace>Q\<rbrace>,\<lbrace>E\<rbrace> \<Longrightarrow> \<lbrace>P\<rbrace> f \<lbrace>Q\<rbrace>,\<lbrace>E\<rbrace>" .
+lemma hoare_trivE_R: "\<lbrace>P\<rbrace> f \<lbrace>Q\<rbrace>,- \<Longrightarrow> \<lbrace>P\<rbrace> f \<lbrace>Q\<rbrace>,-" .
+lemma hoare_trivR_R: "\<lbrace>P\<rbrace> f -,\<lbrace>E\<rbrace> \<Longrightarrow> \<lbrace>P\<rbrace> f -,\<lbrace>E\<rbrace>" .
+
+lemma hoare_vcg_E_conj:
+  "\<lbrakk> \<lbrace>P\<rbrace> f -,\<lbrace>E\<rbrace>; \<lbrace>P'\<rbrace> f \<lbrace>Q'\<rbrace>,\<lbrace>E'\<rbrace> \<rbrakk> \<Longrightarrow> \<lbrace>\<lambda>s. P s \<and> P' s\<rbrace> f \<lbrace>Q'\<rbrace>, \<lbrace>\<lambda>rv s. E rv s \<and> E' rv s\<rbrace>"
+  unfolding validE_def validE_E_def
+  by (rule hoare_post_imp[OF _ hoare_vcg_conj_lift]; simp split: sum.splits)
+
+lemma hoare_vcg_E_elim:
+  "\<lbrakk> \<lbrace>P\<rbrace> f -,\<lbrace>E\<rbrace>; \<lbrace>P'\<rbrace> f \<lbrace>Q\<rbrace>,- \<rbrakk> \<Longrightarrow> \<lbrace>\<lambda>s. P s \<and> P' s\<rbrace> f \<lbrace>Q\<rbrace>,\<lbrace>E\<rbrace>"
+  by (rule hoare_post_impErr[OF hoare_vcg_E_conj]) (simp add: validE_R_def)+
+
+lemma hoare_vcg_R_conj:
+  "\<lbrakk> \<lbrace>P\<rbrace> f \<lbrace>Q\<rbrace>,-; \<lbrace>P'\<rbrace> f \<lbrace>Q'\<rbrace>,- \<rbrakk> \<Longrightarrow> \<lbrace>\<lambda>s. P s \<and> P' s\<rbrace> f \<lbrace>\<lambda>rv s. Q rv s \<and> Q' rv s\<rbrace>,-"
+  unfolding validE_R_def validE_def
+  by (rule hoare_post_imp[OF _ hoare_vcg_conj_lift]; simp split: sum.splits)
+
+lemma hoare_post_imp_R:
+  "\<lbrakk> \<lbrace>P\<rbrace> f \<lbrace>Q'\<rbrace>,-; \<And>rv s. Q' rv s \<Longrightarrow> Q rv s \<rbrakk> \<Longrightarrow> \<lbrace>P\<rbrace> f \<lbrace>Q\<rbrace>,-"
+  unfolding validE_R_def
+  by (erule hoare_post_impErr)
+
+lemma hoare_post_comb_imp_conj:
+  "\<lbrakk> \<lbrace>P'\<rbrace> f \<lbrace>Q\<rbrace>; \<lbrace>P\<rbrace> f \<lbrace>Q'\<rbrace>; \<And>s. P s \<Longrightarrow> P' s \<rbrakk> \<Longrightarrow> \<lbrace>P\<rbrace> f \<lbrace>\<lambda>rv s. Q rv s \<and> Q' rv s\<rbrace>"
+  by (wpsimp wp: hoare_vcg_conj_lift)
+
+
+subsection \<open>Weakest Precondition Rules\<close>
+
+lemma fail_wp:
+  "\<lbrace>\<top>\<rbrace> fail \<lbrace>Q\<rbrace>"
+  by (simp add: valid_def fail_def mres_def vimage_def)
+
+lemma return_wp:
+  "\<lbrace>P x\<rbrace> return x \<lbrace>P\<rbrace>"
+  by(simp add: valid_def return_def mres_def)
+
+lemma get_wp:
+  "\<lbrace>\<lambda>s. Q s s\<rbrace> get \<lbrace>Q\<rbrace>"
+  by (simp add: get_def valid_def mres_def)
+
+lemma gets_wp:
+  "\<lbrace>\<lambda>s. P (f s) s\<rbrace> gets f \<lbrace>P\<rbrace>"
+  by(simp add: valid_def split_def gets_def return_def get_def bind_def mres_def)
+
+lemma put_wp:
+  "\<lbrace>\<lambda>_. Q () s\<rbrace> put s \<lbrace>Q\<rbrace>"
+  by (simp add: put_def valid_def mres_def)
+
+lemma modify_wp:
+  "\<lbrace>\<lambda>s. Q () (f s)\<rbrace> modify f \<lbrace>Q\<rbrace>"
+  unfolding modify_def
+  by (wp put_wp get_wp)
+
+lemma failE_wp:
+  "\<lbrace>\<top>\<rbrace> fail \<lbrace>Q\<rbrace>, \<lbrace>E\<rbrace>"
+  by (simp add: validE_def fail_wp)
+
+lemma returnOk_wp:
+  "\<lbrace>P x\<rbrace> returnOk x \<lbrace>P\<rbrace>,\<lbrace>E\<rbrace>"
+  by (simp add: validE_def2 returnOk_def return_def mres_def)
+
+lemma throwError_wp:
+  "\<lbrace>E e\<rbrace> throwError e \<lbrace>P\<rbrace>,\<lbrace>E\<rbrace>"
+  by(simp add: validE_def2 throwError_def return_def mres_def)
+
+lemma returnOKE_R_wp:
+  "\<lbrace>P x\<rbrace> returnOk x \<lbrace>P\<rbrace>, -"
+  by (simp add: validE_R_def validE_def valid_def returnOk_def return_def mres_def)
+
+lemma liftE_wp:
+  "\<lbrace>P\<rbrace> f \<lbrace>Q\<rbrace> \<Longrightarrow> \<lbrace>P\<rbrace> liftE f \<lbrace>Q\<rbrace>,\<lbrace>E\<rbrace>"
+  by simp
+
+lemma catch_wp:
+  "\<lbrakk> \<And>x. \<lbrace>E x\<rbrace> handler x \<lbrace>Q\<rbrace>; \<lbrace>P\<rbrace> f \<lbrace>Q\<rbrace>,\<lbrace>E\<rbrace> \<rbrakk> \<Longrightarrow> \<lbrace>P\<rbrace> catch f handler \<lbrace>Q\<rbrace>"
+  apply (unfold catch_def validE_def)
+  apply (erule seq_ext)
+  apply (simp add: return_wp split: sum.splits)
+  done
+
+lemma handleE'_wp:
+  "\<lbrakk> \<And>x. \<lbrace>F x\<rbrace> handler x \<lbrace>Q\<rbrace>,\<lbrace>E\<rbrace>; \<lbrace>P\<rbrace> f \<lbrace>Q\<rbrace>,\<lbrace>F\<rbrace> \<rbrakk> \<Longrightarrow> \<lbrace>P\<rbrace> f <handle2> handler \<lbrace>Q\<rbrace>,\<lbrace>E\<rbrace>"
+  apply (unfold handleE'_def validE_def)
+  apply (erule seq_ext)
+  apply (clarsimp split: sum.splits)
+  apply (simp add: valid_def return_def mres_def)
+  done
+
+lemma handleE_wp:
+  assumes x: "\<And>x. \<lbrace>F x\<rbrace> handler x \<lbrace>Q\<rbrace>,\<lbrace>E\<rbrace>"
+  assumes y: "\<lbrace>P\<rbrace> f \<lbrace>Q\<rbrace>,\<lbrace>F\<rbrace>"
+  shows      "\<lbrace>P\<rbrace> f <handle> handler \<lbrace>Q\<rbrace>,\<lbrace>E\<rbrace>"
+  by (simp add: handleE_def handleE'_wp [OF x y])
+
+lemma liftM_wp:
+  "\<lbrace>P\<rbrace> m \<lbrace>Q \<circ> f\<rbrace> \<Longrightarrow> \<lbrace>P\<rbrace> liftM f m \<lbrace>Q\<rbrace>"
+  by (simp add: hoare_liftM_subst)
+
+lemma liftME_wp:
+  "\<lbrace>P\<rbrace> m \<lbrace>Q \<circ> f\<rbrace>,\<lbrace>E\<rbrace> \<Longrightarrow> \<lbrace>P\<rbrace> liftME f m \<lbrace>Q\<rbrace>,\<lbrace>E\<rbrace>"
+  by (simp add: hoare_liftME_subst)
+
+lemma assert_wp:
+  "\<lbrace>\<lambda>s. P \<longrightarrow> Q () s\<rbrace> assert P \<lbrace>Q\<rbrace>"
+  unfolding assert_def
+  by (wpsimp wp: return_wp fail_wp | rule conjI)+
+
+lemma list_cases_wp:
+  assumes a: "\<lbrace>P_A\<rbrace> a \<lbrace>Q\<rbrace>"
+  assumes b: "\<And>x xs. ts = x#xs \<Longrightarrow> \<lbrace>P_B x xs\<rbrace> b x xs \<lbrace>Q\<rbrace>"
+  shows "\<lbrace>case_list P_A P_B ts\<rbrace> case ts of [] \<Rightarrow> a | x # xs \<Rightarrow> b x xs \<lbrace>Q\<rbrace>"
+  by (cases ts, auto simp: a b)
+
+lemma hoare_vcg_handle_elseE:
+  "\<lbrakk> \<lbrace>P\<rbrace> f \<lbrace>Q\<rbrace>,\<lbrace>E\<rbrace>; \<And>e. \<lbrace>E e\<rbrace> g e \<lbrace>R\<rbrace>,\<lbrace>F\<rbrace>; \<And>x. \<lbrace>Q x\<rbrace> h x \<lbrace>R\<rbrace>,\<lbrace>F\<rbrace> \<rbrakk> \<Longrightarrow>
+   \<lbrace>P\<rbrace> f <handle> g <else> h \<lbrace>R\<rbrace>,\<lbrace>F\<rbrace>"
+  unfolding handle_elseE_def validE_def
+  by (wpsimp wp: seq_ext | assumption | rule conjI)+
+
+lemma alternative_wp:
+  assumes x: "\<lbrace>P\<rbrace> f \<lbrace>Q\<rbrace>"
+  assumes y: "\<lbrace>P'\<rbrace> f' \<lbrace>Q\<rbrace>"
+  shows      "\<lbrace>P and P'\<rbrace> f \<sqinter> f' \<lbrace>Q\<rbrace>"
+  unfolding valid_def alternative_def mres_def
+  using post_by_hoare[OF x _ in_mres] post_by_hoare[OF y _ in_mres]
+  by fastforce
+
+lemma alternativeE_wp:
+  assumes "\<lbrace>P\<rbrace> f \<lbrace>Q\<rbrace>,\<lbrace>E\<rbrace>"
+  assumes "\<lbrace>P'\<rbrace> f' \<lbrace>Q\<rbrace>,\<lbrace>E\<rbrace>"
+  shows   "\<lbrace>P and P'\<rbrace> f \<sqinter> f' \<lbrace>Q\<rbrace>,\<lbrace>E\<rbrace>"
+  unfolding validE_def
+  by (wpsimp wp: assms alternative_wp | fold validE_def)+
+
+lemma alternativeE_R_wp:
+  "\<lbrakk> \<lbrace>P\<rbrace> f \<lbrace>Q\<rbrace>,-; \<lbrace>P'\<rbrace> f' \<lbrace>Q\<rbrace>,- \<rbrakk> \<Longrightarrow> \<lbrace>P and P'\<rbrace> f \<sqinter> f' \<lbrace>Q\<rbrace>,-"
+  unfolding validE_R_def
+  by (rule alternativeE_wp)
+
+lemma alternativeE_E_wp:
+  "\<lbrakk> \<lbrace>P\<rbrace> f -,\<lbrace>Q\<rbrace>; \<lbrace>P'\<rbrace> g -,\<lbrace>Q\<rbrace> \<rbrakk> \<Longrightarrow> \<lbrace>P and P'\<rbrace> f \<sqinter> g -, \<lbrace>Q\<rbrace>"
+  unfolding validE_E_def
+  by (rule alternativeE_wp)
+
+lemma select_wp:
+  "\<lbrace>\<lambda>s. \<forall>x \<in> S. Q x s\<rbrace> select S \<lbrace>Q\<rbrace>"
+  by (simp add: select_def valid_def mres_def image_def)
+
+lemma state_select_wp:
+  "\<lbrace> \<lambda>s. \<forall>t. (s, t) \<in> f \<longrightarrow> P () t \<rbrace> state_select f \<lbrace>P\<rbrace>"
+  apply (clarsimp simp: state_select_def assert_def)
+  apply (rule hoare_weaken_pre)
+   apply (wp put_wp select_wp hoare_vcg_if_split return_wp fail_wp get_wp)
+  apply simp
+  done
+
+lemma condition_wp:
+  "\<lbrakk> \<lbrace>Q\<rbrace> A \<lbrace>P\<rbrace>;  \<lbrace>R\<rbrace> B \<lbrace>P\<rbrace> \<rbrakk> \<Longrightarrow> \<lbrace>\<lambda>s. if C s then Q s else R s\<rbrace> condition C A B \<lbrace>P\<rbrace>"
+  by (clarsimp simp: condition_def valid_def)
+
+lemma conditionE_wp:
+  "\<lbrakk> \<lbrace>P\<rbrace> A \<lbrace>Q\<rbrace>,\<lbrace>R\<rbrace>; \<lbrace>P'\<rbrace> B \<lbrace>Q\<rbrace>,\<lbrace>R\<rbrace> \<rbrakk> \<Longrightarrow> \<lbrace>\<lambda>s. if C s then P s else P' s\<rbrace> condition C A B \<lbrace>Q\<rbrace>,\<lbrace>R\<rbrace>"
+  by (clarsimp simp: condition_def validE_def valid_def)
+
+lemma state_assert_wp:
+  "\<lbrace>\<lambda>s. f s \<longrightarrow> P () s\<rbrace> state_assert f \<lbrace>P\<rbrace>"
+  unfolding state_assert_def
+  by (wp seq_ext get_wp assert_wp)
+
+lemma when_wp[wp_split]:
+  "\<lbrakk> P \<Longrightarrow> \<lbrace>Q\<rbrace> f \<lbrace>R\<rbrace> \<rbrakk> \<Longrightarrow> \<lbrace>if P then Q else R ()\<rbrace> when P f \<lbrace>R\<rbrace>"
+  by (clarsimp simp: when_def valid_def return_def mres_def)
+
+lemma unless_wp[wp_split]:
+  "(\<not>P \<Longrightarrow> \<lbrace>Q\<rbrace> f \<lbrace>R\<rbrace>) \<Longrightarrow> \<lbrace>if P then R () else Q\<rbrace> unless P f \<lbrace>R\<rbrace>"
+  unfolding unless_def by wp auto
+
+lemma whenE_wp:
+  "(P \<Longrightarrow> \<lbrace>Q\<rbrace> f \<lbrace>R\<rbrace>, \<lbrace>E\<rbrace>) \<Longrightarrow> \<lbrace>if P then Q else R ()\<rbrace> whenE P f \<lbrace>R\<rbrace>, \<lbrace>E\<rbrace>"
+  unfolding whenE_def by clarsimp (wp returnOk_wp)
+
+lemma hoare_K_bind[wp_split]:
+  "\<lbrace>P\<rbrace> f \<lbrace>Q\<rbrace> \<Longrightarrow> \<lbrace>P\<rbrace> K_bind f x \<lbrace>Q\<rbrace>"
+  by simp
+
+lemma hoare_fun_app_wp:
+  "\<lbrace>P\<rbrace> f' x \<lbrace>Q'\<rbrace> \<Longrightarrow> \<lbrace>P\<rbrace> f' $ x \<lbrace>Q'\<rbrace>"
+  "\<lbrace>P\<rbrace> f x \<lbrace>Q\<rbrace>,\<lbrace>E\<rbrace> \<Longrightarrow> \<lbrace>P\<rbrace> f $ x \<lbrace>Q\<rbrace>,\<lbrace>E\<rbrace>"
+  "\<lbrace>P\<rbrace> f x \<lbrace>Q\<rbrace>,- \<Longrightarrow> \<lbrace>P\<rbrace> f $ x \<lbrace>Q\<rbrace>,-"
+  "\<lbrace>P\<rbrace> f x -,\<lbrace>E\<rbrace> \<Longrightarrow> \<lbrace>P\<rbrace> f $ x -,\<lbrace>E\<rbrace>"
+  by simp+
+
+lemma liftE_validE_E:
+  "\<lbrace>\<top>\<rbrace> liftE f -, \<lbrace>Q\<rbrace>"
+  by (clarsimp simp: validE_E_def valid_def)
+
+lemma returnOk_E:
+  "\<lbrace>\<top>\<rbrace> returnOk r -, \<lbrace>Q\<rbrace>"
+  by (simp add: validE_E_def) (wp returnOk_wp)
+
+lemma case_option_wp:
+  "\<lbrakk> \<And>x. \<lbrace>P x\<rbrace> m x \<lbrace>Q\<rbrace>; \<lbrace>P'\<rbrace> m' \<lbrace>Q\<rbrace> \<rbrakk> \<Longrightarrow>
+   \<lbrace>\<lambda>s. (x = None \<longrightarrow> P' s) \<and> (x \<noteq> None \<longrightarrow> P (the x) s)\<rbrace> case_option m' m x \<lbrace>Q\<rbrace>"
+  by (cases x; simp)
+
+lemma case_option_wpE:
+  "\<lbrakk> \<And>x. \<lbrace>P x\<rbrace> m x \<lbrace>Q\<rbrace>,\<lbrace>E\<rbrace>; \<lbrace>P'\<rbrace> m' \<lbrace>Q\<rbrace>,\<lbrace>E\<rbrace> \<rbrakk> \<Longrightarrow>
+   \<lbrace>\<lambda>s. (x = None \<longrightarrow> P' s) \<and> (x \<noteq> None \<longrightarrow> P (the x) s)\<rbrace> case_option m' m x \<lbrace>Q\<rbrace>,\<lbrace>E\<rbrace>"
+  by (cases x; simp)
+
+lemmas liftME_E_E_wp[wp_split] = validE_validE_E [OF liftME_wp, simplified, OF validE_E_validE]
+
+(* FIXME: make wp *)
+lemma whenE_throwError_wp:
+  "\<lbrace>\<lambda>s. \<not>Q \<longrightarrow> P s\<rbrace> whenE Q (throwError e) \<lbrace>\<lambda>rv. P\<rbrace>, -"
+  by (simp add: whenE_def returnOk_def throwError_def return_def validE_R_def validE_def valid_def
+                mres_def)
+
+lemma select_throwError_wp:
+  "\<lbrace>\<lambda>s. \<forall>x\<in>S. Q x s\<rbrace> select S >>= throwError -, \<lbrace>Q\<rbrace>"
+  by (clarsimp simp: bind_def throwError_def return_def select_def validE_E_def
+                     validE_def valid_def mres_def)
+
+
+subsection \<open>Setting up the @{method wp} method\<close>
+
+lemma valid_is_triple:
+  "valid P f Q = triple_judgement P f (postcondition Q (\<lambda>s f. mres (f s)))"
+  by (simp add: triple_judgement_def valid_def postcondition_def)
+
+lemma validE_is_triple:
+  "validE P f Q E =
+   triple_judgement P f
+     (postconditions (postcondition Q (\<lambda>s f. {(rv, s'). (Inr rv, s') \<in> mres (f s)}))
+                     (postcondition E (\<lambda>s f. {(rv, s'). (Inl rv, s') \<in> mres (f s)})))"
+  by (fastforce simp: validE_def triple_judgement_def valid_def postcondition_def postconditions_def
+                split: sum.split)
+
+lemma validE_R_is_triple:
+  "validE_R P f Q =
+   triple_judgement P f (postcondition Q (\<lambda>s f. {(rv, s'). (Inr rv, s') \<in> mres (f s)}))"
+  by (simp add: validE_R_def validE_is_triple postconditions_def postcondition_def)
+
+lemma validE_E_is_triple:
+  "validE_E P f E =
+   triple_judgement P f (postcondition E (\<lambda>s f. {(rv, s'). (Inl rv, s') \<in> mres (f s)}))"
+  by (simp add: validE_E_def validE_is_triple postconditions_def postcondition_def)
+
+lemmas hoare_wp_combs = hoare_vcg_conj_lift
+
+lemmas hoare_wp_combsE =
+  validE_validE_R
+  hoare_vcg_R_conj
+  hoare_vcg_E_elim
+  hoare_vcg_E_conj
+
+lemmas hoare_wp_state_combsE =
+  valid_validE_R
+  hoare_vcg_R_conj[OF valid_validE_R]
+  hoare_vcg_E_elim[OF valid_validE_E]
+  hoare_vcg_E_conj[OF valid_validE_E]
+
+lemmas hoare_classic_wp_combs = hoare_post_comb_imp_conj hoare_vcg_precond_imp hoare_wp_combs
+lemmas hoare_classic_wp_combsE = hoare_vcg_precond_impE hoare_vcg_precond_impE_R hoare_wp_combsE
+
+lemmas hoare_classic_wp_state_combsE =
+  hoare_vcg_precond_impE[OF valid_validE]
+  hoare_vcg_precond_impE_R[OF valid_validE_R]
+  hoare_wp_state_combsE
+
+lemmas all_classic_wp_combs =
+  hoare_classic_wp_state_combsE
+  hoare_classic_wp_combsE
+  hoare_classic_wp_combs
+
+lemmas hoare_wp_splits[wp_split] =
+  hoare_seq_ext hoare_vcg_seqE handleE'_wp handleE_wp
+  validE_validE_R [OF hoare_vcg_seqE [OF validE_R_validE]]
+  validE_validE_R [OF handleE'_wp [OF validE_R_validE]]
+  validE_validE_R [OF handleE_wp [OF validE_R_validE]]
+  catch_wp hoare_vcg_if_split hoare_vcg_if_splitE
+  validE_validE_R [OF hoare_vcg_if_splitE [OF validE_R_validE validE_R_validE]]
+  liftM_wp liftME_wp
+  validE_validE_R [OF liftME_wp [OF validE_R_validE]]
+  validE_valid
+
+lemmas [wp_comb] = hoare_wp_state_combsE hoare_wp_combsE  hoare_wp_combs
+
+(* rules towards the bottom will be matched first *)
+lemmas [wp] = hoare_vcg_prop
+              wp_post_taut
+              hoare_fun_app_wp
+              returnOk_E
+              liftE_validE_E
+              put_wp
+              get_wp
+              gets_wp
+              modify_wp
+              return_wp
+              returnOk_wp
+              throwError_wp
+              fail_wp
+              failE_wp
+              assert_wp
+              state_assert_wp
+              liftE_wp
+              alternative_wp
+              alternativeE_R_wp
+              alternativeE_E_wp
+              alternativeE_wp
+              select_wp
+              state_select_wp
+              condition_wp
+              conditionE_wp
+
+lemmas [wp_trip] = valid_is_triple validE_is_triple validE_E_is_triple validE_R_is_triple
+
+lemmas validE_E_combs[wp_comb] =
+    hoare_vcg_E_conj[where Q'="\<top>\<top>", folded validE_E_def]
+    valid_validE_E
+    hoare_vcg_E_conj[where Q'="\<top>\<top>", folded validE_E_def, OF valid_validE_E]
+
+
+text \<open>Simplifications on conjunction\<close>
+
+lemma hoare_post_eq:
+  "\<lbrakk> Q = Q'; \<lbrace>P\<rbrace> f \<lbrace>Q'\<rbrace> \<rbrakk> \<Longrightarrow> \<lbrace>P\<rbrace> f \<lbrace>Q\<rbrace>"
+  by simp
+
+lemma hoare_post_eqE1:
+  "\<lbrakk> Q = Q'; \<lbrace>P\<rbrace> f \<lbrace>Q'\<rbrace>,\<lbrace>E\<rbrace> \<rbrakk> \<Longrightarrow> \<lbrace>P\<rbrace> f \<lbrace>Q\<rbrace>,\<lbrace>E\<rbrace>"
+  by simp
+
+lemma hoare_post_eqE2:
+  "\<lbrakk> E = E'; \<lbrace>P\<rbrace> f \<lbrace>Q\<rbrace>,\<lbrace>E'\<rbrace> \<rbrakk> \<Longrightarrow> \<lbrace>P\<rbrace> f \<lbrace>Q\<rbrace>,\<lbrace>E\<rbrace>"
+  by simp
+
+lemma hoare_post_eqE_R:
+  "\<lbrakk> Q = Q'; \<lbrace>P\<rbrace> f \<lbrace>Q'\<rbrace>,- \<rbrakk> \<Longrightarrow> \<lbrace>P\<rbrace> f \<lbrace>Q\<rbrace>,-"
+  by simp
+
+lemma pred_conj_apply_elim:
+  "(\<lambda>rv. Q rv and Q' rv) = (\<lambda>rv s. Q rv s \<and> Q' rv s)"
+  by (simp add: pred_conj_def)
+
+lemma pred_conj_conj_elim:
+  "(\<lambda>rv s. (Q rv and Q' rv) s \<and> Q'' rv s) = (\<lambda>rv s. Q rv s \<and> Q' rv s \<and> Q'' rv s)"
+  by simp
+
+lemma conj_assoc_apply:
+  "(\<lambda>rv s. (Q rv s \<and> Q' rv s) \<and> Q'' rv s) = (\<lambda>rv s. Q rv s \<and> Q' rv s \<and> Q'' rv s)"
+  by simp
+
+lemma all_elim:
+  "(\<lambda>rv s. \<forall>x. P rv s) = P"
+  by simp
+
+lemma all_conj_elim:
+  "(\<lambda>rv s. (\<forall>x. P rv s) \<and> Q rv s) = (\<lambda>rv s. P rv s \<and> Q rv s)"
+  by simp
+
+lemmas vcg_rhs_simps =
+  pred_conj_apply_elim pred_conj_conj_elim conj_assoc_apply all_elim all_conj_elim
+
+lemma if_apply_reduct:
+  "\<lbrace>P\<rbrace> If P' (f x) (g x) \<lbrace>Q\<rbrace> \<Longrightarrow> \<lbrace>P\<rbrace> If P' f g x \<lbrace>Q\<rbrace>"
+  by (cases P'; simp)
+
+lemma if_apply_reductE:
+  "\<lbrace>P\<rbrace> If P' (f x) (g x) \<lbrace>Q\<rbrace>,\<lbrace>E\<rbrace> \<Longrightarrow> \<lbrace>P\<rbrace> If P' f g x \<lbrace>Q\<rbrace>,\<lbrace>E\<rbrace>"
+  by (cases P'; simp)
+
+lemma if_apply_reductE_R:
+  "\<lbrace>P\<rbrace> If P' (f x) (g x) \<lbrace>Q\<rbrace>,- \<Longrightarrow> \<lbrace>P\<rbrace> If P' f g x \<lbrace>Q\<rbrace>,-"
+  by (cases P'; simp)
+
+lemmas hoare_wp_simps [wp_split] =
+  vcg_rhs_simps [THEN hoare_post_eq] vcg_rhs_simps [THEN hoare_post_eqE1]
+  vcg_rhs_simps [THEN hoare_post_eqE2] vcg_rhs_simps [THEN hoare_post_eqE_R]
+  if_apply_reduct if_apply_reductE if_apply_reductE_R TrueI
+
+schematic_goal if_apply_test:
+  "\<lbrace>?Q\<rbrace> (if A then returnOk else K fail) x \<lbrace>P\<rbrace>,\<lbrace>E\<rbrace>"
+  by wpsimp
+
+lemma hoare_elim_pred_conj:
+  "\<lbrace>P\<rbrace> f \<lbrace>\<lambda>rv s. Q rv s \<and> Q' rv s\<rbrace> \<Longrightarrow> \<lbrace>P\<rbrace> f \<lbrace>\<lambda>rv. Q rv and Q' rv\<rbrace>"
+  by (unfold pred_conj_def)
+
+lemma hoare_elim_pred_conjE1:
+  "\<lbrace>P\<rbrace> f \<lbrace>\<lambda>rv s. Q rv s \<and> Q' rv s\<rbrace>,\<lbrace>E\<rbrace> \<Longrightarrow> \<lbrace>P\<rbrace> f \<lbrace>\<lambda>rv. Q rv and Q' rv\<rbrace>,\<lbrace>E\<rbrace>"
+  by (unfold pred_conj_def)
+
+lemma hoare_elim_pred_conjE2:
+  "\<lbrace>P\<rbrace> f \<lbrace>Q\<rbrace>, \<lbrace>\<lambda>rv s. E rv s \<and> E' rv s\<rbrace> \<Longrightarrow> \<lbrace>P\<rbrace> f \<lbrace>Q\<rbrace>,\<lbrace>\<lambda>rv. E rv and E' rv\<rbrace>"
+  by (unfold pred_conj_def)
+
+lemma hoare_elim_pred_conjE_R:
+  "\<lbrace>P\<rbrace> f \<lbrace>\<lambda>rv s. Q rv s \<and> Q' rv s\<rbrace>,- \<Longrightarrow> \<lbrace>P\<rbrace> f \<lbrace>\<lambda>rv. Q rv and Q' rv\<rbrace>,-"
+  by (unfold pred_conj_def)
+
+lemmas hoare_wp_pred_conj_elims =
+  hoare_elim_pred_conj hoare_elim_pred_conjE1
+  hoare_elim_pred_conjE2 hoare_elim_pred_conjE_R
+
+
+text \<open>Miscellaneous lemmas on hoare triples\<close>
+
+lemma hoare_vcg_mp:
+  "\<lbrakk> \<lbrace>P\<rbrace> f \<lbrace>Q\<rbrace>; \<lbrace>P\<rbrace> f \<lbrace>\<lambda>r s. Q r s \<longrightarrow> Q' r s\<rbrace> \<rbrakk> \<Longrightarrow> \<lbrace>P\<rbrace> f \<lbrace>Q'\<rbrace>"
+  by (auto simp: valid_def split_def)
+
+(* note about this precond stuff: rules get a chance to bind directly
+   before any of their combined forms. As a result, these precondition
+   implication rules are only used when needed. *)
+lemma hoare_add_post:
+  "\<lbrakk> \<lbrace>P'\<rbrace> f \<lbrace>Q'\<rbrace>; \<And>s. P s \<Longrightarrow> P' s; \<lbrace>P\<rbrace> f \<lbrace>\<lambda>rv s. Q' rv s \<longrightarrow> Q rv s\<rbrace> \<rbrakk> \<Longrightarrow> \<lbrace>P\<rbrace> f \<lbrace>Q\<rbrace>"
+  unfolding valid_def
+  by fastforce
+
+lemma hoare_gen_asmE:
+  "(P \<Longrightarrow> \<lbrace>P'\<rbrace> f \<lbrace>Q\<rbrace>,-) \<Longrightarrow> \<lbrace>P' and K P\<rbrace> f \<lbrace>Q\<rbrace>, -"
+  by (simp add: validE_R_def validE_def valid_def) blast
+
+lemma hoare_list_case:
+  "\<lbrakk> \<lbrace>P1\<rbrace> f f1 \<lbrace>Q\<rbrace>; \<And>y ys. xs = y#ys \<Longrightarrow> \<lbrace>P2 y ys\<rbrace> f (f2 y ys) \<lbrace>Q\<rbrace> \<rbrakk> \<Longrightarrow>
+   \<lbrace>case xs of [] \<Rightarrow> P1 | y#ys \<Rightarrow> P2 y ys\<rbrace> f (case xs of [] \<Rightarrow> f1 | y#ys \<Rightarrow> f2 y ys) \<lbrace>Q\<rbrace>"
+  by (cases xs; simp)
+
+lemma hoare_use_eq:
+  assumes "\<And>P. \<lbrace>\<lambda>s. P (f s)\<rbrace> m \<lbrace>\<lambda>_ s. P (f s)\<rbrace>"
+  assumes "\<And>f. \<lbrace>\<lambda>s. P f s\<rbrace> m \<lbrace>\<lambda>_ s. Q f s\<rbrace>"
+  shows "\<lbrace>\<lambda>s. P (f s) s\<rbrace> m \<lbrace>\<lambda>_ s. Q (f s) s \<rbrace>"
+  apply (rule hoare_post_imp[where Q="\<lambda>_ s. \<exists>y. y = f s \<and> Q y s"], simp)
+  apply (wpsimp wp: hoare_vcg_ex_lift assms)
+  done
+
+lemma hoare_fail_any[simp]:
+  "\<lbrace>P\<rbrace> fail \<lbrace>Q\<rbrace>"
+  by wp
+
+lemma hoare_failE[simp]:
+  "\<lbrace>P\<rbrace> fail \<lbrace>Q\<rbrace>, \<lbrace>E\<rbrace>"
+  by wp
+
+lemma hoare_FalseE[simp]:
+  "\<lbrace>\<bottom>\<rbrace> f \<lbrace>Q\<rbrace>, \<lbrace>E\<rbrace>"
+  by (simp add: valid_def validE_def)
+
+lemma hoare_validE_pred_conj:
+  "\<lbrakk> \<lbrace>P\<rbrace> f \<lbrace>Q\<rbrace>, \<lbrace>E\<rbrace>; \<lbrace>P\<rbrace> f \<lbrace>R\<rbrace>, \<lbrace>E\<rbrace> \<rbrakk> \<Longrightarrow> \<lbrace>P\<rbrace> f \<lbrace>Q and R\<rbrace>, \<lbrace>E\<rbrace>"
+  unfolding valid_def validE_def
+  by (simp add: split_def split: sum.splits)
+
+lemma hoare_validE_conj:
+  "\<lbrakk> \<lbrace>P\<rbrace> f \<lbrace>Q\<rbrace>, \<lbrace>E\<rbrace>; \<lbrace>P\<rbrace> f \<lbrace>R\<rbrace>, \<lbrace>E\<rbrace> \<rbrakk> \<Longrightarrow> \<lbrace>P\<rbrace> f \<lbrace>\<lambda>rv s. Q rv s \<and> R rv s\<rbrace>, \<lbrace>E\<rbrace>"
+  unfolding valid_def validE_def
+  by (simp add: split_def split: sum.splits)
+
+lemmas hoare_valid_validE = valid_validE (* FIXME lib: eliminate one *)
+
+declare validE_validE_E[wp_comb]
+
+lemmas if_validE_E[wp_split] =
+  validE_validE_E[OF hoare_vcg_if_splitE[OF validE_E_validE validE_E_validE]]
+
+lemma hoare_drop_imp:
+  "\<lbrace>P\<rbrace> f \<lbrace>Q\<rbrace> \<Longrightarrow> \<lbrace>P\<rbrace> f \<lbrace>\<lambda>rv s. R rv s \<longrightarrow> Q rv s\<rbrace>"
+  by (auto simp: valid_def)
+
+lemma hoare_drop_impE:
+  "\<lbrakk>\<lbrace>P\<rbrace> f \<lbrace>\<lambda>r. Q\<rbrace>, \<lbrace>E\<rbrace>\<rbrakk> \<Longrightarrow> \<lbrace>P\<rbrace> f \<lbrace>\<lambda>rv s. R rv s \<longrightarrow> Q s\<rbrace>, \<lbrace>E\<rbrace>"
+  by (simp add: validE_weaken)
+
+lemma hoare_drop_impE_R:
+  "\<lbrace>P\<rbrace> f \<lbrace>Q\<rbrace>,- \<Longrightarrow> \<lbrace>P\<rbrace> f \<lbrace>\<lambda>rv s. R rv s \<longrightarrow> Q rv s\<rbrace>, -"
+  by (auto simp: validE_R_def validE_def valid_def split_def split: sum.splits)
+
+lemma hoare_drop_impE_E:
+  "\<lbrace>P\<rbrace> f -,\<lbrace>Q\<rbrace> \<Longrightarrow> \<lbrace>P\<rbrace> f -, \<lbrace>\<lambda>rv s. R rv s \<longrightarrow> Q rv s\<rbrace>"
+  by (auto simp: validE_E_def validE_def valid_def split_def split: sum.splits)
+
+lemmas hoare_drop_imps = hoare_drop_imp hoare_drop_impE_R hoare_drop_impE_E
+
+lemmas bindE_E_wp[wp_split] = validE_validE_E[OF hoare_vcg_seqE [OF validE_E_validE]]
+
+lemma True_E_E[wp]:
+  "\<lbrace>\<top>\<rbrace> f -,\<lbrace>\<top>\<top>\<rbrace>"
+  by (auto simp: validE_E_def validE_def valid_def split: sum.splits)
+
+
+subsection \<open>Strongest postcondition rules\<close>
+
+lemma get_sp:
+  "\<lbrace>P\<rbrace> get \<lbrace>\<lambda>rv s. s = rv \<and> P s\<rbrace>"
+  by(simp add:get_def valid_def mres_def)
+
+lemma put_sp:
+  "\<lbrace>\<top>\<rbrace> put a \<lbrace>\<lambda>_ s. s = a\<rbrace>"
+  by(simp add:put_def valid_def mres_def)
+
+lemma return_sp:
+  "\<lbrace>P\<rbrace> return a \<lbrace>\<lambda>rv s. rv = a \<and> P s\<rbrace>"
+  by(simp add:return_def valid_def mres_def)
+
+lemma hoare_return_sp: (* FIXME lib: eliminate *)
+  "\<lbrace>P\<rbrace> return x \<lbrace>\<lambda>rv. P and K (rv = x)\<rbrace>"
+  by (simp add: valid_def return_def mres_def)
+
+lemma assert_sp:
+  "\<lbrace>P\<rbrace> assert Q \<lbrace>\<lambda>_ s. P s \<and> Q \<rbrace>"
+  by (simp add: assert_def fail_def return_def valid_def mres_def)
+
+lemma hoare_gets_sp:
+  "\<lbrace>P\<rbrace> gets f \<lbrace>\<lambda>rv s. rv = f s \<and> P s\<rbrace>"
+  by (simp add: valid_def simpler_gets_def mres_def)
+
+lemma hoare_returnOk_sp:
+  "\<lbrace>P\<rbrace> returnOk x \<lbrace>\<lambda>rv s. rv = x \<and> P s\<rbrace>, \<lbrace>Q\<rbrace>"
+  by (simp add: valid_def validE_def returnOk_def return_def mres_def)
+
+
+
 
 lemma trace_steps_append:
   "trace_steps (xs @ ys) s
@@ -348,9 +1442,6 @@ lemma prefix_closed_select[iff]:
   "prefix_closed (select S)"
   by (simp add: prefix_closed_def select_def image_def)
 
-lemma select_wp[wp]: "\<lbrace>\<lambda>s. \<forall>x \<in> S. Q x s\<rbrace> select S \<lbrace>Q\<rbrace>"
-  by (simp add: select_def valid_def mres_def image_def)
-
 lemma rely_cond_rtranclp:
   "rely_cond R s (map (Pair Env) xs) \<Longrightarrow> rtranclp R s (last_st_tr (map (Pair Env) xs) s)"
   apply (induct xs arbitrary: s rule: rev_induct)
@@ -359,24 +1450,6 @@ lemma rely_cond_rtranclp:
   apply (erule converse_rtranclp_into_rtranclp)
   apply simp
   done
-
-lemma put_wp[wp]:
-  "\<lbrace>\<lambda>_. Q () s\<rbrace> put s \<lbrace>Q\<rbrace>"
-  by (simp add: put_def valid_def mres_def)
-
-lemma get_wp[wp]:
-  "\<lbrace>\<lambda>s. Q s s\<rbrace> get \<lbrace>Q\<rbrace>"
-  by (simp add: get_def valid_def mres_def)
-
-lemma bind_wp[wp_split]:
-  "\<lbrakk>  \<And>r. \<lbrace>Q' r\<rbrace> g r \<lbrace>Q\<rbrace>; \<lbrace>P\<rbrace>f \<lbrace>Q'\<rbrace> \<rbrakk>
-    \<Longrightarrow> \<lbrace>P\<rbrace>  f >>= (\<lambda>r. g r) \<lbrace>Q\<rbrace>"
-  by (fastforce simp: valid_def bind_def2 mres_def intro: image_eqI[rotated])
-
-lemma modify_wp[wp]:
-  "\<lbrace>\<lambda>s. Q () (f s)\<rbrace> modify f \<lbrace>Q\<rbrace>"
-  unfolding modify_def
-  by wp
 
 definition
   no_trace :: "('s,'a) tmonad  \<Rightarrow> bool"
@@ -413,17 +1486,11 @@ lemma validI_is_triple:
   apply (cases "prefix_closed f"; simp)
   done
 
-lemma valid_is_triple:
-  "valid P f Q =
-      triple_judgement P f
-           (\<lambda>s f. (\<forall>(r,s') \<in> (mres (f s)). Q r s'))"
-  by (simp add: triple_judgement_def valid_def mres_def)
-
 lemma no_trace_is_triple:
   "no_trace f = triple_judgement \<top> f (\<lambda>() f. id no_trace f)"
   by (simp add: triple_judgement_def split: unit.split)
 
-lemmas [wp_trip] = valid_is_triple validI_is_triple no_trace_is_triple
+lemmas [wp_trip] = validI_is_triple no_trace_is_triple
 
 lemma valid_validI_wp[wp_comb]:
   "no_trace f \<Longrightarrow> (\<And>s0. \<lbrace>P s0\<rbrace> f \<lbrace>\<lambda>v. Q v s0 \<rbrace>)
@@ -493,1579 +1560,13 @@ lemma Await_sync_twp:
   apply (simp add: o_def)
   done
 
-(* Wrap up the standard usage pattern of wp/wpc/simp into its own command: *)
-method wpsimp uses wp simp split split_del cong =
-  ((determ \<open>wp add: wp|wpc|clarsimp simp: simp split: split split del: split_del cong: cong\<close>)+)[1]
-
-section "Satisfiability"
-
-text \<open>
-  The dual to validity: an existential instead of a universal
-  quantifier for the post condition. In refinement, it is
-  often sufficient to know that there is one state that
-  satisfies a condition.
-\<close>
-definition
-  exs_valid :: "('a \<Rightarrow> bool) \<Rightarrow> ('a, 'b) tmonad \<Rightarrow>
-                ('b \<Rightarrow> 'a \<Rightarrow> bool) \<Rightarrow> bool"
-  ("\<lbrace>_\<rbrace> _ \<exists>\<lbrace>_\<rbrace>")
-where
-  "exs_valid P f Q \<equiv> (\<forall>s. P s \<longrightarrow> (\<exists>(rv, s') \<in> mres (f s). Q rv s'))"
-
-
-text \<open>The above for the exception monad\<close>
-definition
-  ex_exs_validE :: "('a \<Rightarrow> bool) \<Rightarrow> ('a, 'e + 'b) tmonad \<Rightarrow>
-                    ('b \<Rightarrow> 'a \<Rightarrow> bool) \<Rightarrow> ('e \<Rightarrow> 'a \<Rightarrow> bool) \<Rightarrow> bool"
-   ("\<lbrace>_\<rbrace> _ \<exists>\<lbrace>_\<rbrace>, \<lbrace>_\<rbrace>")
-where
-  "ex_exs_validE P f Q E \<equiv>
-     exs_valid P f (\<lambda>rv. case rv of Inl e \<Rightarrow> E e | Inr v \<Rightarrow> Q v)"
-
-
-section "Lemmas"
-
-subsection \<open>Determinism\<close>
-
-lemma det_set_iff:
-  "det f \<Longrightarrow> (r \<in> mres (f s)) = (mres (f s) = {r})"
-  apply (simp add: det_def mres_def)
-  apply (fastforce elim: allE[where x=s])
-  done
-
-lemma return_det [iff]:
-  "det (return x)"
-  by (simp add: det_def return_def)
-
-lemma put_det [iff]:
-  "det (put s)"
-  by (simp add: det_def put_def)
-
-lemma get_det [iff]:
-  "det get"
-  by (simp add: det_def get_def)
-
-lemma det_gets [iff]:
-  "det (gets f)"
-  by (auto simp add: gets_def det_def get_def return_def bind_def)
-
-lemma det_UN:
-  "det f \<Longrightarrow> (\<Union>x \<in> mres (f s). g x) = (g (THE x. x \<in> mres (f s)))"
-  unfolding det_def mres_def
-  apply simp
-  apply (drule spec [of _ s])
-  apply (clarsimp simp: vimage_def)
-  done
-
-lemma bind_detI [simp, intro!]:
-  "\<lbrakk> det f; \<forall>x. det (g x) \<rbrakk> \<Longrightarrow> det (f >>= g)"
-  apply (simp add: bind_def det_def split_def)
-  apply clarsimp
-  apply (erule_tac x=s in allE)
-  apply clarsimp
-  done
-
-lemma det_modify[iff]:
-  "det (modify f)"
-  by (simp add: modify_def)
-
-lemma the_run_stateI:
-  "mres (M s) = {s'} \<Longrightarrow> the_run_state M s = s'"
-  by (simp add: the_run_state_def)
-
-lemma the_run_state_det:
-  "\<lbrakk> s' \<in> mres (M s); det M \<rbrakk> \<Longrightarrow> the_run_state M s = s'"
-  by (simp only: the_run_stateI det_set_iff[where f=M and s=s])
-
-subsection "Lifting and Alternative Basic Definitions"
-
-lemma liftE_liftM: "liftE = liftM Inr"
-  apply (rule ext)
-  apply (simp add: liftE_def liftM_def)
-  done
-
-lemma liftME_liftM: "liftME f = liftM (case_sum Inl (Inr \<circ> f))"
-  apply (rule ext)
-  apply (simp add: liftME_def liftM_def bindE_def returnOk_def lift_def)
-  apply (rule_tac f="bind x" in arg_cong)
-  apply (rule ext)
-  apply (case_tac xa)
-   apply (simp_all add: lift_def throwError_def)
-  done
-
-lemma liftE_bindE:
-  "(liftE a) >>=E b = a >>= b"
-  apply (simp add: liftE_def bindE_def lift_def bind_assoc)
-  done
-
-lemma liftM_id[simp]: "liftM id = id"
-  apply (rule ext)
-  apply (simp add: liftM_def)
-  done
-
-lemma liftM_bind:
-  "(liftM t f >>= g) = (f >>= (\<lambda>x. g (t x)))"
-  by (simp add: liftM_def bind_assoc)
-
-lemma gets_bind_ign: "gets f >>= (\<lambda>x. m) = m"
-  apply (rule ext)
-  apply (simp add: bind_def simpler_gets_def)
-  done
-
-lemma get_bind_apply: "(get >>= f) x = f x x"
-  by (simp add: get_def bind_def)
-
-lemma exec_gets:
-  "(gets f >>= m) s = m (f s) s"
-  by (simp add: simpler_gets_def bind_def)
-
-lemma exec_get:
-  "(get >>= m) s = m s s"
-  by (simp add: get_def bind_def)
-
-lemma bind_eqI:
-  "\<lbrakk> f = f'; \<And>x. g x = g' x \<rbrakk> \<Longrightarrow> f >>= g = f' >>= g'"
-  apply (rule ext)
-  apply (simp add: bind_def)
-  done
-
-subsection "Simplification Rules for Lifted And/Or"
-
-lemma bipred_disj_op_eq[simp]:
-  "reflp R \<Longrightarrow> ((=) or R) = R"
-  apply (rule ext, rule ext)
-  apply (auto simp: reflp_def)
-  done
-
-lemma bipred_le_true[simp]: "R \<le> \<top>\<top>"
-  by clarsimp
-
-subsection "Hoare Logic Rules"
-
-lemma validE_def2:
-   "validE P f Q R \<equiv> \<forall>s. P s \<longrightarrow> (\<forall>(r,s') \<in> mres (f s). case r of Inr b \<Rightarrow> Q b s'
-                                                              | Inl a \<Rightarrow> R a s')"
-   by (unfold valid_def validE_def)
-
-lemma seq':
-  "\<lbrakk> \<lbrace>A\<rbrace> f \<lbrace>B\<rbrace>;
-     \<forall>x. P x \<longrightarrow> \<lbrace>C\<rbrace> g x \<lbrace>D\<rbrace>;
-     \<forall>x s. B x s \<longrightarrow> P x \<and> C s \<rbrakk> \<Longrightarrow>
-   \<lbrace>A\<rbrace> do x \<leftarrow> f; g x od \<lbrace>D\<rbrace>"
-  apply (erule bind_wp[rotated])
-  apply (clarsimp simp: valid_def)
-  apply (fastforce elim: rev_bexI image_eqI[rotated])
-  done
-
-lemma seq:
-  assumes f_valid: "\<lbrace>A\<rbrace> f \<lbrace>B\<rbrace>"
-  assumes g_valid: "\<And>x. P x \<Longrightarrow> \<lbrace>C\<rbrace> g x \<lbrace>D\<rbrace>"
-  assumes bind:  "\<And>x s. B x s \<Longrightarrow> P x \<and> C s"
-  shows "\<lbrace>A\<rbrace> do x \<leftarrow> f; g x od \<lbrace>D\<rbrace>"
-apply (insert f_valid g_valid bind)
-apply (blast intro: seq')
-done
-
-lemma seq_ext':
-  "\<lbrakk> \<lbrace>A\<rbrace> f \<lbrace>B\<rbrace>;
-     \<forall>x. \<lbrace>B x\<rbrace> g x \<lbrace>C\<rbrace> \<rbrakk> \<Longrightarrow>
-   \<lbrace>A\<rbrace> do x \<leftarrow> f; g x od \<lbrace>C\<rbrace>"
-  by (metis bind_wp)
-
-lemmas seq_ext = bind_wp[rotated]
-
-lemma seqE':
-  "\<lbrakk> \<lbrace>A\<rbrace> f \<lbrace>B\<rbrace>,\<lbrace>E\<rbrace> ;
-     \<forall>x. \<lbrace>B x\<rbrace> g x \<lbrace>C\<rbrace>,\<lbrace>E\<rbrace> \<rbrakk> \<Longrightarrow>
-   \<lbrace>A\<rbrace> doE x \<leftarrow> f; g x odE \<lbrace>C\<rbrace>,\<lbrace>E\<rbrace>"
-  apply (simp add: bindE_def validE_def)
-  apply (erule seq_ext')
-  apply (auto simp: lift_def valid_def throwError_def return_def mres_def
-             split: sum.splits)
-  done
-
-lemma seqE:
-  assumes f_valid: "\<lbrace>A\<rbrace> f \<lbrace>B\<rbrace>,\<lbrace>E\<rbrace>"
-  assumes g_valid: "\<And>x. \<lbrace>B x\<rbrace> g x \<lbrace>C\<rbrace>,\<lbrace>E\<rbrace>"
-  shows "\<lbrace>A\<rbrace> doE x \<leftarrow> f; g x odE \<lbrace>C\<rbrace>,\<lbrace>E\<rbrace>"
-  apply(insert f_valid g_valid)
-  apply(blast intro: seqE')
-  done
-
-lemma hoare_TrueI: "\<lbrace>P\<rbrace> f \<lbrace>\<lambda>_. \<top>\<rbrace>"
-  by (simp add: valid_def)
-
-lemma hoareE_TrueI: "\<lbrace>P\<rbrace> f \<lbrace>\<lambda>_. \<top>\<rbrace>, \<lbrace>\<lambda>r. \<top>\<rbrace>"
-  by (simp add: validE_def valid_def)
-
-lemma hoare_True_E_R [simp]:
-  "\<lbrace>P\<rbrace> f \<lbrace>\<lambda>r s. True\<rbrace>, -"
-  by (auto simp add: validE_R_def validE_def valid_def split: sum.splits)
-
-lemma hoare_post_conj [intro!]:
-  "\<lbrakk> \<lbrace> P \<rbrace> a \<lbrace> Q \<rbrace>; \<lbrace> P \<rbrace> a \<lbrace> R \<rbrace> \<rbrakk> \<Longrightarrow> \<lbrace> P \<rbrace> a \<lbrace> Q and R \<rbrace>"
-  by (fastforce simp: valid_def split_def pred_conj_def)
-
-lemma hoare_pre_disj [intro!]:
-  "\<lbrakk> \<lbrace> P \<rbrace> a \<lbrace> R \<rbrace>; \<lbrace> Q \<rbrace> a \<lbrace> R \<rbrace> \<rbrakk> \<Longrightarrow> \<lbrace> P or Q \<rbrace> a \<lbrace> R \<rbrace>"
-  by (simp add:valid_def pred_disj_def)
-
-lemma hoare_conj:
-  "\<lbrakk> \<lbrace>P\<rbrace> f \<lbrace>Q\<rbrace>; \<lbrace>P'\<rbrace> f \<lbrace>Q'\<rbrace> \<rbrakk> \<Longrightarrow> \<lbrace>P and P'\<rbrace> f \<lbrace>Q and Q'\<rbrace>"
-  unfolding valid_def
-  by (auto)
-
-lemma hoare_post_taut: "\<lbrace> P \<rbrace> a \<lbrace> \<top>\<top> \<rbrace>"
-  by (simp add:valid_def)
-
-lemma wp_post_taut: "\<lbrace>\<lambda>r. True\<rbrace> f \<lbrace>\<lambda>r s. True\<rbrace>"
-  by (rule hoare_post_taut)
-
-lemma wp_post_tautE: "\<lbrace>\<lambda>r. True\<rbrace> f \<lbrace>\<lambda>r s. True\<rbrace>,\<lbrace>\<lambda>f s. True\<rbrace>"
-proof -
-  have P: "\<And>r. (case r of Inl a \<Rightarrow> True | _ \<Rightarrow> True) = True"
-    by (case_tac r, simp_all)
-  show ?thesis
-    by (simp add: validE_def P wp_post_taut)
-qed
-
-lemma hoare_pre_cont [simp]: "\<lbrace> \<bottom> \<rbrace> a \<lbrace> P \<rbrace>"
-  by (simp add:valid_def)
-
-
-subsection \<open>Strongest Postcondition Rules\<close>
-
-lemma get_sp:
-  "\<lbrace>P\<rbrace> get \<lbrace>\<lambda>a s. s = a \<and> P s\<rbrace>"
-  by(simp add:get_def valid_def mres_def)
-
-lemma put_sp:
-  "\<lbrace>\<top>\<rbrace> put a \<lbrace>\<lambda>_ s. s = a\<rbrace>"
-  by(simp add:put_def valid_def mres_def)
-
-lemma return_sp:
-  "\<lbrace>P\<rbrace> return a \<lbrace>\<lambda>b s. b = a \<and> P s\<rbrace>"
-  by(simp add:return_def valid_def mres_def)
-
-lemma assert_sp:
-  "\<lbrace> P \<rbrace> assert Q \<lbrace> \<lambda>r s. P s \<and> Q \<rbrace>"
-  by (simp add: assert_def fail_def return_def valid_def mres_def)
-
-lemma hoare_gets_sp:
-  "\<lbrace>P\<rbrace> gets f \<lbrace>\<lambda>rv s. rv = f s \<and> P s\<rbrace>"
-  by (simp add: valid_def simpler_gets_def mres_def)
-
-lemma hoare_return_drop_var [iff]: "\<lbrace> Q \<rbrace> return x \<lbrace> \<lambda>r. Q \<rbrace>"
-  by (simp add:valid_def return_def mres_def)
-
-lemma hoare_gets [intro!]: "\<lbrakk> \<And>s. P s \<Longrightarrow> Q (f s) s \<rbrakk> \<Longrightarrow> \<lbrace> P \<rbrace> gets f \<lbrace> Q \<rbrace>"
-  by (simp add:valid_def gets_def get_def bind_def return_def mres_def)
-
-lemma hoare_modifyE_var [intro!]:
-  "\<lbrakk> \<And>s. P s \<Longrightarrow> Q (f s) \<rbrakk> \<Longrightarrow> \<lbrace> P \<rbrace> modify f \<lbrace> \<lambda>r s. Q s \<rbrace>"
-  by(simp add: valid_def modify_def put_def get_def bind_def mres_def)
-
-lemma hoare_if [intro!]:
-  "\<lbrakk> P \<Longrightarrow> \<lbrace> Q \<rbrace> a \<lbrace> R \<rbrace>; \<not> P \<Longrightarrow> \<lbrace> Q \<rbrace> b \<lbrace> R \<rbrace> \<rbrakk> \<Longrightarrow>
-   \<lbrace> Q \<rbrace> if P then a else b \<lbrace> R \<rbrace>"
-  by (simp add:valid_def)
-
-lemma hoare_pre_subst: "\<lbrakk> A = B; \<lbrace>A\<rbrace> a \<lbrace>C\<rbrace> \<rbrakk> \<Longrightarrow> \<lbrace>B\<rbrace> a \<lbrace>C\<rbrace>"
-  by(clarsimp simp:valid_def split_def)
-
-lemma hoare_post_subst: "\<lbrakk> B = C; \<lbrace>A\<rbrace> a \<lbrace>B\<rbrace> \<rbrakk> \<Longrightarrow> \<lbrace>A\<rbrace> a \<lbrace>C\<rbrace>"
-  by(clarsimp simp:valid_def split_def)
-
-lemma hoare_pre_tautI: "\<lbrakk> \<lbrace>A and P\<rbrace> a \<lbrace>B\<rbrace>; \<lbrace>A and not P\<rbrace> a \<lbrace>B\<rbrace> \<rbrakk> \<Longrightarrow> \<lbrace>A\<rbrace> a \<lbrace>B\<rbrace>"
-  by(fastforce simp:valid_def split_def pred_conj_def pred_neg_def)
-
-lemma hoare_pre_imp: "\<lbrakk> \<And>s. P s \<Longrightarrow> Q s; \<lbrace>Q\<rbrace> a \<lbrace>R\<rbrace> \<rbrakk> \<Longrightarrow> \<lbrace>P\<rbrace> a \<lbrace>R\<rbrace>"
-  by (fastforce simp add:valid_def)
-
-lemma hoare_post_imp: "\<lbrakk> \<And>r s. Q r s \<Longrightarrow> R r s; \<lbrace>P\<rbrace> a \<lbrace>Q\<rbrace> \<rbrakk> \<Longrightarrow> \<lbrace>P\<rbrace> a \<lbrace>R\<rbrace>"
-  by(fastforce simp:valid_def split_def)
-
-lemma hoare_post_impErr': "\<lbrakk> \<lbrace>P\<rbrace> a \<lbrace>Q\<rbrace>,\<lbrace>E\<rbrace>;
-                           \<forall>r s. Q r s \<longrightarrow> R r s;
-                           \<forall>e s. E e s \<longrightarrow> F e s \<rbrakk> \<Longrightarrow>
-                         \<lbrace>P\<rbrace> a \<lbrace>R\<rbrace>,\<lbrace>F\<rbrace>"
- apply (simp add: validE_def)
- apply (rule_tac Q="\<lambda>r s. case r of Inl a \<Rightarrow> E a s | Inr b \<Rightarrow> Q b s" in hoare_post_imp)
-  apply (case_tac r)
-   apply simp_all
- done
-
-lemma hoare_post_impErr: "\<lbrakk> \<lbrace>P\<rbrace> a \<lbrace>Q\<rbrace>,\<lbrace>E\<rbrace>;
-                          \<And>r s. Q r s \<Longrightarrow> R r s;
-                          \<And>e s. E e s \<Longrightarrow> F e s \<rbrakk> \<Longrightarrow>
-                         \<lbrace>P\<rbrace> a \<lbrace>R\<rbrace>,\<lbrace>F\<rbrace>"
- apply (blast intro: hoare_post_impErr')
- done
-
-lemma hoare_validE_cases:
-  "\<lbrakk> \<lbrace> P \<rbrace> f \<lbrace> Q \<rbrace>, \<lbrace> \<lambda>_ _. True \<rbrace>; \<lbrace> P \<rbrace> f \<lbrace> \<lambda>_ _. True \<rbrace>, \<lbrace> R \<rbrace> \<rbrakk>
-  \<Longrightarrow> \<lbrace> P \<rbrace> f \<lbrace> Q \<rbrace>, \<lbrace> R \<rbrace>"
-  by (simp add: validE_def valid_def split: sum.splits) blast
-
-lemma hoare_post_imp_dc:
-  "\<lbrakk>\<lbrace>P\<rbrace> a \<lbrace>\<lambda>r. Q\<rbrace>; \<And>s. Q s \<Longrightarrow> R s\<rbrakk> \<Longrightarrow> \<lbrace>P\<rbrace> a \<lbrace>\<lambda>r. R\<rbrace>,\<lbrace>\<lambda>r. R\<rbrace>"
-  by (simp add: validE_def valid_def split: sum.splits) blast
-
-lemma hoare_post_imp_dc2:
-  "\<lbrakk>\<lbrace>P\<rbrace> a \<lbrace>\<lambda>r. Q\<rbrace>; \<And>s. Q s \<Longrightarrow> R s\<rbrakk> \<Longrightarrow> \<lbrace>P\<rbrace> a \<lbrace>\<lambda>r. R\<rbrace>,\<lbrace>\<lambda>r s. True\<rbrace>"
-  by (simp add: validE_def valid_def split: sum.splits) blast
-
-lemma hoare_post_imp_dc2E:
-  "\<lbrakk>\<lbrace>P\<rbrace> a \<lbrace>\<lambda>r. Q\<rbrace>; \<And>s. Q s \<Longrightarrow> R s\<rbrakk> \<Longrightarrow> \<lbrace>P\<rbrace> a \<lbrace>\<lambda>r s. True\<rbrace>, \<lbrace>\<lambda>r. R\<rbrace>"
-  by (simp add: validE_def valid_def split: sum.splits) fast
-
-lemma hoare_post_imp_dc2E_actual:
-  "\<lbrakk>\<lbrace>P\<rbrace> a \<lbrace>\<lambda>r. R\<rbrace>\<rbrakk> \<Longrightarrow> \<lbrace>P\<rbrace> a \<lbrace>\<lambda>r s. True\<rbrace>, \<lbrace>\<lambda>r. R\<rbrace>"
-  by (simp add: validE_def valid_def split: sum.splits) fast
-
-lemma hoare_post_imp_dc2_actual:
-  "\<lbrakk>\<lbrace>P\<rbrace> a \<lbrace>\<lambda>r. R\<rbrace>\<rbrakk> \<Longrightarrow> \<lbrace>P\<rbrace> a \<lbrace>\<lambda>r. R\<rbrace>, \<lbrace>\<lambda>r s. True\<rbrace>"
-  by (simp add: validE_def valid_def split: sum.splits) fast
-
-lemma hoare_post_impE: "\<lbrakk> \<And>r s. Q r s \<Longrightarrow> R r s; \<lbrace>P\<rbrace> a \<lbrace>Q\<rbrace> \<rbrakk> \<Longrightarrow> \<lbrace>P\<rbrace> a \<lbrace>R\<rbrace>"
-  by (fastforce simp:valid_def split_def)
-
-lemma hoare_conjD1:
-  "\<lbrace>P\<rbrace> f \<lbrace>\<lambda>rv. Q rv and R rv\<rbrace> \<Longrightarrow> \<lbrace>P\<rbrace> f \<lbrace>\<lambda>rv. Q rv\<rbrace>"
-  unfolding valid_def by auto
-
-lemma hoare_conjD2:
-  "\<lbrace>P\<rbrace> f \<lbrace>\<lambda>rv. Q rv and R rv\<rbrace> \<Longrightarrow> \<lbrace>P\<rbrace> f \<lbrace>\<lambda>rv. R rv\<rbrace>"
-  unfolding valid_def by auto
-
-lemma hoare_post_disjI1:
-  "\<lbrace>P\<rbrace> f \<lbrace>\<lambda>rv. Q rv\<rbrace> \<Longrightarrow> \<lbrace>P\<rbrace> f \<lbrace>\<lambda>rv. Q rv or R rv\<rbrace>"
-  unfolding valid_def by auto
-
-lemma hoare_post_disjI2:
-  "\<lbrace>P\<rbrace> f \<lbrace>\<lambda>rv. R rv\<rbrace> \<Longrightarrow> \<lbrace>P\<rbrace> f \<lbrace>\<lambda>rv. Q rv or R rv\<rbrace>"
-  unfolding valid_def by auto
-
-lemma hoare_weaken_pre:
-  "\<lbrakk>\<lbrace>Q\<rbrace> a \<lbrace>R\<rbrace>; \<And>s. P s \<Longrightarrow> Q s\<rbrakk> \<Longrightarrow> \<lbrace>P\<rbrace> a \<lbrace>R\<rbrace>"
-  apply (rule hoare_pre_imp)
-   prefer 2
-   apply assumption
-  apply blast
-  done
-
-lemma hoare_strengthen_post:
-  "\<lbrakk>\<lbrace>P\<rbrace> a \<lbrace>Q\<rbrace>; \<And>r s. Q r s \<Longrightarrow> R r s\<rbrakk> \<Longrightarrow> \<lbrace>P\<rbrace> a \<lbrace>R\<rbrace>"
-  apply (rule hoare_post_imp)
-   prefer 2
-   apply assumption
-  apply blast
-  done
-
-lemma use_valid: "\<lbrakk>(r, s') \<in> mres (f s); \<lbrace>P\<rbrace> f \<lbrace>Q\<rbrace>; P s \<rbrakk> \<Longrightarrow> Q r s'"
-  apply (simp add: valid_def)
-  apply blast
-  done
-
-lemma use_validE_norm: "\<lbrakk> (Inr r', s') \<in> mres (B s); \<lbrace> P \<rbrace> B \<lbrace> Q \<rbrace>,\<lbrace> E \<rbrace>; P s \<rbrakk> \<Longrightarrow> Q r' s'"
-  apply (clarsimp simp: validE_def valid_def)
-  apply force
-  done
-
-lemma use_validE_except: "\<lbrakk> (Inl r', s') \<in> mres (B s); \<lbrace> P \<rbrace> B \<lbrace> Q \<rbrace>,\<lbrace> E \<rbrace>; P s \<rbrakk> \<Longrightarrow> E r' s'"
-  apply (clarsimp simp: validE_def valid_def)
-  apply force
-  done
-
-lemma in_inv_by_hoareD:
-  "\<lbrakk> \<And>P. \<lbrace>P\<rbrace> f \<lbrace>\<lambda>_. P\<rbrace>; (x,s') \<in> mres (f s) \<rbrakk> \<Longrightarrow> s' = s"
-  apply (drule_tac x="(=) s" in meta_spec)
-  apply (auto simp add: valid_def mres_def)
-  done
-
-subsection "Satisfiability"
-
-lemma exs_hoare_post_imp: "\<lbrakk>\<And>r s. Q r s \<Longrightarrow> R r s; \<lbrace>P\<rbrace> a \<exists>\<lbrace>Q\<rbrace>\<rbrakk> \<Longrightarrow> \<lbrace>P\<rbrace> a \<exists>\<lbrace>R\<rbrace>"
-  apply (simp add: exs_valid_def)
-  apply safe
-  apply (erule_tac x=s in allE, simp)
-  apply blast
-  done
-
-lemma use_exs_valid: "\<lbrakk>\<lbrace>P\<rbrace> f \<exists>\<lbrace>Q\<rbrace>; P s \<rbrakk> \<Longrightarrow> \<exists>(r, s') \<in> mres (f s). Q r s'"
-  by (simp add: exs_valid_def)
-
-definition "exs_postcondition P f \<equiv> (\<lambda>a b. \<exists>(rv, s)\<in> f a b. P rv s)"
-
-lemma exs_valid_is_triple:
-  "exs_valid P f Q = triple_judgement P f (exs_postcondition Q (\<lambda>s f. mres (f s)))"
-  by (simp add: triple_judgement_def exs_postcondition_def exs_valid_def)
-
-lemmas [wp_trip] = exs_valid_is_triple
-
-lemma exs_valid_weaken_pre [wp_comb]:
-  "\<lbrakk> \<lbrace> P' \<rbrace> f \<exists>\<lbrace> Q \<rbrace>; \<And>s. P s \<Longrightarrow> P' s \<rbrakk> \<Longrightarrow> \<lbrace> P \<rbrace> f \<exists>\<lbrace> Q \<rbrace>"
-  apply atomize
-  apply (clarsimp simp: exs_valid_def)
-  done
-
-lemma exs_valid_chain:
-  "\<lbrakk> \<lbrace> P \<rbrace> f \<exists>\<lbrace> Q \<rbrace>; \<And>s. R s \<Longrightarrow> P s; \<And>r s. Q r s \<Longrightarrow> S r s \<rbrakk> \<Longrightarrow> \<lbrace> R \<rbrace> f \<exists>\<lbrace> S \<rbrace>"
-  by (fastforce simp only: exs_valid_def Bex_def )
-
-lemma exs_valid_assume_pre:
-  "\<lbrakk> \<And>s. P s \<Longrightarrow> \<lbrace> P \<rbrace> f \<exists>\<lbrace> Q \<rbrace> \<rbrakk> \<Longrightarrow> \<lbrace> P \<rbrace> f \<exists>\<lbrace> Q \<rbrace>"
-  apply (fastforce simp: exs_valid_def)
-  done
-
-lemma exs_valid_bind [wp_split]:
-    "\<lbrakk> \<And>x. \<lbrace>B x\<rbrace> g x \<exists>\<lbrace>C\<rbrace>; \<lbrace>A\<rbrace> f \<exists>\<lbrace>B\<rbrace> \<rbrakk> \<Longrightarrow> \<lbrace> A \<rbrace> f >>= (\<lambda>x. g x) \<exists>\<lbrace> C \<rbrace>"
-  apply atomize
-  apply (clarsimp simp: exs_valid_def bind_def2 mres_def)
-  apply (drule spec, drule(1) mp, clarsimp)
-  apply (drule spec2, drule(1) mp, clarsimp)
-  apply (simp add: image_def bex_Un)
-  apply (strengthen subst[where P="\<lambda>x. x \<in> f s" for s, mk_strg I _ E], simp)
-  apply (fastforce elim: rev_bexI)
-  done
-
-lemma exs_valid_return [wp]:
-    "\<lbrace> Q v \<rbrace> return v \<exists>\<lbrace> Q \<rbrace>"
-  by (clarsimp simp: exs_valid_def return_def mres_def)
-
-lemma exs_valid_select [wp]:
-    "\<lbrace> \<lambda>s. \<exists>r \<in> S. Q r s \<rbrace> select S \<exists>\<lbrace> Q \<rbrace>"
-  apply (clarsimp simp: exs_valid_def select_def mres_def)
-  apply (auto simp add: image_def)
-  done
-
-lemma exs_valid_get [wp]:
-    "\<lbrace> \<lambda>s. Q s s \<rbrace> get \<exists>\<lbrace> Q \<rbrace>"
-  by (clarsimp simp: exs_valid_def get_def mres_def)
-
-lemma exs_valid_gets [wp]:
-    "\<lbrace> \<lambda>s. Q (f s) s \<rbrace> gets f \<exists>\<lbrace> Q \<rbrace>"
-  by (clarsimp simp: gets_def) wp
-
-lemma exs_valid_put [wp]:
-    "\<lbrace> Q v \<rbrace> put v \<exists>\<lbrace> Q \<rbrace>"
-  by (clarsimp simp: put_def exs_valid_def mres_def)
-
-lemma exs_valid_state_assert [wp]:
-    "\<lbrace> \<lambda>s. Q () s \<and> G s \<rbrace> state_assert G \<exists>\<lbrace> Q \<rbrace>"
-  by (clarsimp simp: state_assert_def exs_valid_def get_def
-           assert_def bind_def2 return_def mres_def)
-
-lemmas exs_valid_guard = exs_valid_state_assert
-
-lemma exs_valid_fail [wp]:
-    "\<lbrace> \<lambda>_. False \<rbrace> fail \<exists>\<lbrace> Q \<rbrace>"
-  by (clarsimp simp: fail_def exs_valid_def)
-
-lemma exs_valid_condition [wp]:
-    "\<lbrakk> \<lbrace> P \<rbrace> L \<exists>\<lbrace> Q \<rbrace>; \<lbrace> P' \<rbrace> R \<exists>\<lbrace> Q \<rbrace> \<rbrakk> \<Longrightarrow>
-          \<lbrace> \<lambda>s. (C s \<and> P s) \<or> (\<not> C s \<and> P' s) \<rbrace> condition C L R \<exists>\<lbrace> Q \<rbrace>"
-  by (clarsimp simp: condition_def exs_valid_def split: sum.splits)
-
-
-subsection MISC
-
-lemma hoare_return_simp:
-  "\<lbrace>P\<rbrace> return x \<lbrace>Q\<rbrace> = (\<forall>s. P s \<longrightarrow> Q x s)"
-  by (simp add: valid_def return_def mres_def)
-
-lemma hoare_gen_asm:
-  "(P \<Longrightarrow> \<lbrace>P'\<rbrace> f \<lbrace>Q\<rbrace>) \<Longrightarrow> \<lbrace>P' and K P\<rbrace> f \<lbrace>Q\<rbrace>"
-  by (fastforce simp add: valid_def)
-
-lemma when_wp [wp]:
- "\<lbrakk> P \<Longrightarrow> \<lbrace>Q\<rbrace> f \<lbrace>R\<rbrace> \<rbrakk> \<Longrightarrow> \<lbrace>if P then Q else R ()\<rbrace> when P f \<lbrace>R\<rbrace>"
-  by (clarsimp simp: when_def valid_def return_def mres_def)
-
-lemma hoare_conjI:
-  "\<lbrakk> \<lbrace>P\<rbrace> f \<lbrace>Q\<rbrace>; \<lbrace>P\<rbrace> f \<lbrace>R\<rbrace> \<rbrakk> \<Longrightarrow> \<lbrace>P\<rbrace> f \<lbrace>\<lambda>r s. Q r s \<and> R r s\<rbrace>"
-  unfolding valid_def by blast
-
-lemma hoare_disjI1:
-  "\<lbrakk> \<lbrace>P\<rbrace> f \<lbrace>Q\<rbrace> \<rbrakk> \<Longrightarrow> \<lbrace>P\<rbrace> f \<lbrace>\<lambda>r s. Q r s \<or>  R r s \<rbrace>"
-  unfolding valid_def by blast
-
-lemma hoare_disjI2:
-  "\<lbrakk> \<lbrace>P\<rbrace> f \<lbrace>R\<rbrace> \<rbrakk> \<Longrightarrow> \<lbrace>P\<rbrace> f \<lbrace>\<lambda>r s. Q r s \<or>  R r s \<rbrace>"
-  unfolding valid_def by blast
-
-lemma hoare_assume_pre:
-  "(\<And>s. P s \<Longrightarrow> \<lbrace>P\<rbrace> f \<lbrace>Q\<rbrace>) \<Longrightarrow> \<lbrace>P\<rbrace> f \<lbrace>Q\<rbrace>"
-  by (auto simp: valid_def)
-
-lemma hoare_returnOk_sp:
-  "\<lbrace>P\<rbrace> returnOk x \<lbrace>\<lambda>r s. r = x \<and> P s\<rbrace>, \<lbrace>Q\<rbrace>"
-  by (simp add: valid_def validE_def returnOk_def return_def mres_def)
-
-lemma hoare_assume_preE:
-  "(\<And>s. P s \<Longrightarrow> \<lbrace>P\<rbrace> f \<lbrace>Q\<rbrace>,\<lbrace>R\<rbrace>) \<Longrightarrow> \<lbrace>P\<rbrace> f \<lbrace>Q\<rbrace>,\<lbrace>R\<rbrace>"
-  by (auto simp: valid_def validE_def)
-
-lemma hoare_allI:
-  "(\<And>x. \<lbrace>P\<rbrace>f\<lbrace>Q x\<rbrace>) \<Longrightarrow> \<lbrace>P\<rbrace>f\<lbrace>\<lambda>r s. \<forall>x. Q x r s\<rbrace>"
-  by (simp add: valid_def) blast
-
-lemma validE_allI:
-  "(\<And>x. \<lbrace>P\<rbrace> f \<lbrace>\<lambda>r s. Q x r s\<rbrace>,\<lbrace>E\<rbrace>) \<Longrightarrow> \<lbrace>P\<rbrace> f \<lbrace>\<lambda>r s. \<forall>x. Q x r s\<rbrace>,\<lbrace>E\<rbrace>"
-  by (fastforce simp: valid_def validE_def split: sum.splits)
-
-lemma hoare_exI:
-  "\<lbrace>P\<rbrace> f \<lbrace>Q x\<rbrace> \<Longrightarrow> \<lbrace>P\<rbrace> f \<lbrace>\<lambda>r s. \<exists>x. Q x r s\<rbrace>"
-  by (simp add: valid_def) blast
-
-lemma hoare_impI:
-  "(R \<Longrightarrow> \<lbrace>P\<rbrace>f\<lbrace>Q\<rbrace>) \<Longrightarrow> \<lbrace>P\<rbrace>f\<lbrace>\<lambda>r s. R \<longrightarrow> Q r s\<rbrace>"
-  by (simp add: valid_def) blast
-
-lemma validE_impI:
-  " \<lbrakk>\<And>E. \<lbrace>P\<rbrace> f \<lbrace>\<lambda>_ _. True\<rbrace>,\<lbrace>E\<rbrace>; (P' \<Longrightarrow> \<lbrace>P\<rbrace> f \<lbrace>Q\<rbrace>,\<lbrace>E\<rbrace>)\<rbrakk> \<Longrightarrow>
-         \<lbrace>P\<rbrace> f \<lbrace>\<lambda>r s. P' \<longrightarrow> Q r s\<rbrace>, \<lbrace>E\<rbrace>"
-  by (fastforce simp: validE_def valid_def split: sum.splits)
-
-lemma hoare_case_option_wp:
-  "\<lbrakk> \<lbrace>P\<rbrace> f None \<lbrace>Q\<rbrace>;
-     \<And>x.  \<lbrace>P' x\<rbrace> f (Some x) \<lbrace>Q' x\<rbrace> \<rbrakk>
-  \<Longrightarrow> \<lbrace>case_option P P' v\<rbrace> f v \<lbrace>\<lambda>rv. case v of None \<Rightarrow> Q rv | Some x \<Rightarrow> Q' x rv\<rbrace>"
-  by (cases v) auto
-
-subsection "Reasoning directly about states"
-
-lemma in_throwError:
-  "((v, s') \<in> mres (throwError e s)) = (v = Inl e \<and> s' = s)"
-  by (simp add: throwError_def return_def mres_def)
-
-lemma in_returnOk:
-  "((v', s') \<in> mres (returnOk v s)) = (v' = Inr v \<and> s' = s)"
-  by (simp add: returnOk_def return_def mres_def)
-
-lemma in_bind:
-  "((r,s') \<in> mres ((do x \<leftarrow> f; g x od) s)) =
-   (\<exists>s'' x. (x, s'') \<in> mres (f s) \<and> (r, s') \<in> mres (g x s''))"
-  apply (simp add: bind_def split_def mres_def)
-  apply (auto split: tmres.splits; force elim: rev_bexI image_eqI[rotated])
-  done
-
-lemma in_bindE_R:
-  "((Inr r,s') \<in> mres ((doE x \<leftarrow> f; g x odE) s)) =
-  (\<exists>s'' x. (Inr x, s'') \<in> mres (f s) \<and> (Inr r, s') \<in> mres (g x s''))"
-  apply (simp add: bindE_def in_bind)
-  apply (simp add: lift_def split_def)
-  apply (clarsimp simp: throwError_def return_def lift_def mres_def split: sum.splits)
-  apply force
-  done
-
-lemma in_bindE_L:
-  "((Inl r, s') \<in> mres ((doE x \<leftarrow> f; g x odE) s)) \<Longrightarrow>
-  (\<exists>s'' x. (Inr x, s'') \<in> mres (f s) \<and> (Inl r, s') \<in> mres (g x s'')) \<or> ((Inl r, s') \<in> mres (f s))"
-  apply (simp add: bindE_def in_bind lift_def)
-  apply safe
-  apply (simp add: return_def throwError_def lift_def split_def mres_def split: sum.splits if_split_asm)
-  apply force+
-  done
-
-lemma in_return:
-  "(r, s') \<in> mres (return v s) = (r = v \<and> s' = s)"
-  by (simp add: return_def mres_def)
-
-lemma in_liftE:
-  "((v, s') \<in> mres (liftE f s)) = (\<exists>v'. v = Inr v' \<and> (v', s') \<in> mres (f s))"
-  by (auto simp add: liftE_def in_bind in_return)
-
-lemma in_whenE:  "((v, s') \<in> mres (whenE P f s)) = ((P \<longrightarrow> (v, s') \<in> mres (f s)) \<and>
-                                                   (\<not>P \<longrightarrow> v = Inr () \<and> s' = s))"
-  by (simp add: whenE_def in_returnOk)
-
-lemma inl_whenE:
-  "((Inl x, s') \<in> mres (whenE P f s)) = (P \<and> (Inl x, s') \<in> mres (f s))"
-  by (auto simp add: in_whenE)
-
-lemma in_fail:
-  "r \<in> mres (fail s) = False"
-  by (simp add: fail_def mres_def)
-
-lemma in_assert:
-  "(r, s') \<in> mres (assert P s) = (P \<and> s' = s)"
-  by (auto simp add: assert_def return_def fail_def mres_def)
-
-lemma in_assertE:
-  "(r, s') \<in> mres (assertE P s) = (P \<and> r = Inr () \<and> s' = s)"
-  by (auto simp add: assertE_def returnOk_def return_def fail_def mres_def)
-
-lemma in_assert_opt:
-  "(r, s') \<in> mres (assert_opt v s) = (v = Some r \<and> s' = s)"
-  by (auto simp: assert_opt_def in_fail in_return split: option.splits)
-
-lemma in_get:
-  "(r, s') \<in> mres (get s) = (r = s \<and> s' = s)"
-  by (simp add: get_def mres_def)
-
-lemma in_gets:
-  "(r, s') \<in> mres (gets f s) = (r = f s \<and> s' = s)"
-  by (simp add: simpler_gets_def mres_def)
-
-lemma in_put:
-  "(r, s') \<in> mres (put x s) = (s' = x \<and> r = ())"
-  by (simp add: put_def mres_def)
-
-lemma in_when:
-  "(v, s') \<in> mres (when P f s) = ((P \<longrightarrow> (v, s') \<in> mres (f s)) \<and> (\<not>P \<longrightarrow> v = () \<and> s' = s))"
-  by (simp add: when_def in_return)
-
-lemma in_modify:
-  "(v, s') \<in> mres (modify f s) = (s'=f s \<and> v = ())"
-  by (auto simp add: modify_def bind_def get_def put_def mres_def)
-
-lemma gets_the_in_monad:
-  "((v, s') \<in> mres (gets_the f s)) = (s' = s \<and> f s = Some v)"
-  by (auto simp: gets_the_def in_bind in_gets in_assert_opt split: option.split)
-
-lemma in_alternative:
-  "(r,s') \<in> mres ((f \<sqinter> g) s) = ((r,s') \<in> mres (f s) \<or> (r,s') \<in> mres (g s))"
-  by (auto simp add: alternative_def mres_def)
-
-lemmas in_monad = inl_whenE in_whenE in_liftE in_bind in_bindE_L
-                  in_bindE_R in_returnOk in_throwError in_fail
-                  in_assertE in_assert in_return in_assert_opt
-                  in_get in_gets in_put in_when (* unlessE_whenE *)
-                  (* unless_when *) in_modify gets_the_in_monad
-                  in_alternative
-
-subsection "Non-Failure"
-
-lemma no_failD:
-  "\<lbrakk> no_fail P m; P s \<rbrakk> \<Longrightarrow> Failed \<notin> snd ` m s"
-  by (simp add: no_fail_def)
-
-lemma no_fail_modify [wp,simp]:
-  "no_fail \<top> (modify f)"
-  by (simp add: no_fail_def modify_def get_def put_def bind_def)
-
-lemma no_fail_gets_simp[simp]:
-  "no_fail P (gets f)"
-  unfolding no_fail_def gets_def get_def return_def bind_def
-  by simp
-
-lemma no_fail_gets:
-  "no_fail \<top> (gets f)"
-  by simp
-
-lemma snd_pair_image:
- "snd ` Pair x ` S = S"
-  by (simp add: image_def)
-
-lemma no_fail_select [simp]:
-  "no_fail \<top> (select S)"
-  by (simp add: no_fail_def select_def image_def)
-
-lemma no_fail_pre:
-  "\<lbrakk> no_fail P f; \<And>s. Q s \<Longrightarrow> P s\<rbrakk> \<Longrightarrow> no_fail Q f"
-  by (simp add: no_fail_def)
-
-lemma no_fail_alt [wp]:
-  "\<lbrakk> no_fail P f; no_fail Q g \<rbrakk> \<Longrightarrow> no_fail (P and Q) (f \<sqinter> g)"
-  by (auto simp add: no_fail_def alternative_def)
-
-lemma no_fail_return [simp, wp]:
-  "no_fail \<top> (return x)"
-  by (simp add: return_def no_fail_def)
-
-lemma no_fail_get [simp, wp]:
-  "no_fail \<top> get"
-  by (simp add: get_def no_fail_def)
-
-lemma no_fail_put [simp, wp]:
-  "no_fail \<top> (put s)"
-  by (simp add: put_def no_fail_def)
-
-lemma no_fail_when [wp]:
-  "(P \<Longrightarrow> no_fail Q f) \<Longrightarrow> no_fail (if P then Q else \<top>) (when P f)"
-  by (simp add: when_def)
-
-lemma no_fail_unless [wp]:
-  "(\<not>P \<Longrightarrow> no_fail Q f) \<Longrightarrow> no_fail (if P then \<top> else Q) (unless P f)"
-  by (simp add: unless_def when_def)
-
-lemma no_fail_fail [simp, wp]:
-  "no_fail \<bottom> fail"
-  by (simp add: fail_def no_fail_def)
-
-lemmas [wp] = no_fail_gets
-
-lemma no_fail_assert [simp, wp]:
-  "no_fail (\<lambda>_. P) (assert P)"
-  by (simp add: assert_def)
-
-lemma no_fail_assert_opt [simp, wp]:
-  "no_fail (\<lambda>_. P \<noteq> None) (assert_opt P)"
-  by (simp add: assert_opt_def split: option.splits)
-
-lemma no_fail_case_option [wp]:
-  assumes f: "no_fail P f"
-  assumes g: "\<And>x. no_fail (Q x) (g x)"
-  shows "no_fail (if x = None then P else Q (the x)) (case_option f g x)"
-  by (clarsimp simp add: f g)
-
-lemma no_fail_if [wp]:
-  "\<lbrakk> P \<Longrightarrow> no_fail Q f; \<not>P \<Longrightarrow> no_fail R g \<rbrakk> \<Longrightarrow>
-  no_fail (if P then Q else R) (if P then f else g)"
-  by simp
-
-lemma no_fail_apply [wp]:
-  "no_fail P (f (g x)) \<Longrightarrow> no_fail P (f $ g x)"
-  by simp
-
-lemma no_fail_undefined [simp, wp]:
-  "no_fail \<bottom> undefined"
-  by (simp add: no_fail_def)
-
-lemma no_fail_returnOK [simp, wp]:
-  "no_fail \<top> (returnOk x)"
-  by (simp add: returnOk_def)
-
-(* text {* Empty results implies non-failure *}
-
-lemma empty_fail_modify [simp]:
-  "empty_fail (modify f)"
-  by (simp add: empty_fail_def simpler_modify_def)
-
-lemma empty_fail_gets [simp]:
-  "empty_fail (gets f)"
-  by (simp add: empty_fail_def simpler_gets_def)
-
-lemma empty_failD:
-  "\<lbrakk> empty_fail m; fst (m s) = {} \<rbrakk> \<Longrightarrow> snd (m s)"
-  by (simp add: empty_fail_def)
-
-lemma empty_fail_select_f [simp]:
-  assumes ef: "fst S = {} \<Longrightarrow> snd S"
-  shows "empty_fail (select_f S)"
-  by (fastforce simp add: empty_fail_def select_f_def intro: ef)
-
-lemma empty_fail_bind [simp]:
-  "\<lbrakk> empty_fail a; \<And>x. empty_fail (b x) \<rbrakk> \<Longrightarrow> empty_fail (a >>= b)"
-  apply (simp add: bind_def empty_fail_def split_def)
-  apply clarsimp
-  apply (case_tac "fst (a s) = {}")
-   apply blast
-  apply (clarsimp simp: ex_in_conv [symmetric])
-  done
-
-lemma empty_fail_return [simp]:
-  "empty_fail (return x)"
-  by (simp add: empty_fail_def return_def)
-
-lemma empty_fail_mapM [simp]:
-  assumes m: "\<And>x. empty_fail (m x)"
-  shows "empty_fail (mapM m xs)"
-proof (induct xs)
-  case Nil
-  thus ?case by (simp add: mapM_def sequence_def)
-next
-  case Cons
-  have P: "\<And>m x xs. mapM m (x # xs) = (do y \<leftarrow> m x; ys \<leftarrow> (mapM m xs); return (y # ys) od)"
-    by (simp add: mapM_def sequence_def Let_def)
-  from Cons
-  show ?case by (simp add: P m)
-qed
-
-lemma empty_fail [simp]:
-  "empty_fail fail"
-  by (simp add: fail_def empty_fail_def)
-
-lemma empty_fail_assert_opt [simp]:
-  "empty_fail (assert_opt x)"
-  by (simp add: assert_opt_def split: option.splits)
-
-lemma empty_fail_mk_ef:
-  "empty_fail (mk_ef o m)"
-  by (simp add: empty_fail_def mk_ef_def)
- *)
-subsection "Failure"
-
-lemma fail_wp: "\<lbrace>\<lambda>x. True\<rbrace> fail \<lbrace>Q\<rbrace>"
-  by (simp add: valid_def fail_def mres_def vimage_def)
-
-lemma failE_wp: "\<lbrace>\<lambda>x. True\<rbrace> fail \<lbrace>Q\<rbrace>,\<lbrace>E\<rbrace>"
-  by (simp add: validE_def fail_wp)
-
-lemma fail_update [iff]:
-  "fail (f s) = fail s"
-  by (simp add: fail_def)
-
-
-text \<open>We can prove postconditions using hoare triples\<close>
-
-lemma post_by_hoare: "\<lbrakk> \<lbrace>P\<rbrace> f \<lbrace>Q\<rbrace>; P s; (r, s') \<in> mres (f s) \<rbrakk> \<Longrightarrow> Q r s'"
-  apply (simp add: valid_def)
-  apply blast
-  done
-
-text \<open>Weakest Precondition Rules\<close>
-
-lemma hoare_vcg_prop:
-  "\<lbrace>\<lambda>s. P\<rbrace> f \<lbrace>\<lambda>rv s. P\<rbrace>"
-  by (simp add: valid_def)
-
-lemma return_wp:
-  "\<lbrace>P x\<rbrace> return x \<lbrace>P\<rbrace>"
-  by(simp add:valid_def return_def mres_def)
-
-(* lemma get_wp:
-  "\<lbrace>\<lambda>s. P s s\<rbrace> get \<lbrace>P\<rbrace>"
-  by(auto simp add:valid_def split_def get_def mres_def)
- *)
-lemma gets_wp:
-  "\<lbrace>\<lambda>s. P (f s) s\<rbrace> gets f \<lbrace>P\<rbrace>"
-  by(simp add:valid_def split_def gets_def return_def get_def bind_def mres_def)
-
-(* lemma modify_wp:
-  "\<lbrace>\<lambda>s. P () (f s)\<rbrace> modify f \<lbrace>P\<rbrace>"
-  by(simp add:valid_def split_def modify_def get_def put_def bind_def )
- *)
-(* lemma put_wp:
- "\<lbrace>\<lambda>s. P () x\<rbrace> put x \<lbrace>P\<rbrace>"
- by(simp add:valid_def put_def)
- *)
-lemma returnOk_wp:
-  "\<lbrace>P x\<rbrace> returnOk x \<lbrace>P\<rbrace>,\<lbrace>E\<rbrace>"
- by(simp add:validE_def2 returnOk_def return_def mres_def)
-
-lemma throwError_wp:
-  "\<lbrace>E e\<rbrace> throwError e \<lbrace>P\<rbrace>,\<lbrace>E\<rbrace>"
-  by(simp add:validE_def2 throwError_def return_def mres_def)
-
-lemma returnOKE_R_wp : "\<lbrace>P x\<rbrace> returnOk x \<lbrace>P\<rbrace>, -"
-  by (simp add: validE_R_def validE_def valid_def returnOk_def return_def mres_def)
-
-lemma catch_wp:
-  "\<lbrakk> \<And>x. \<lbrace>E x\<rbrace> handler x \<lbrace>Q\<rbrace>; \<lbrace>P\<rbrace> f \<lbrace>Q\<rbrace>,\<lbrace>E\<rbrace> \<rbrakk> \<Longrightarrow>
-   \<lbrace>P\<rbrace> catch f handler \<lbrace>Q\<rbrace>"
-  apply (unfold catch_def validE_def)
-  apply (erule seq_ext)
-  apply (simp add: return_wp split: sum.splits)
-  done
-
-lemma handleE'_wp:
-  "\<lbrakk> \<And>x. \<lbrace>F x\<rbrace> handler x \<lbrace>Q\<rbrace>,\<lbrace>E\<rbrace>; \<lbrace>P\<rbrace> f \<lbrace>Q\<rbrace>,\<lbrace>F\<rbrace> \<rbrakk> \<Longrightarrow>
-   \<lbrace>P\<rbrace> f <handle2> handler \<lbrace>Q\<rbrace>,\<lbrace>E\<rbrace>"
-  apply (unfold handleE'_def validE_def)
-  apply (erule seq_ext)
-  apply (clarsimp split: sum.splits)
-  apply (simp add: valid_def return_def mres_def)
-  done
-
-lemma handleE_wp:
-  assumes x: "\<And>x. \<lbrace>F x\<rbrace> handler x \<lbrace>Q\<rbrace>,\<lbrace>E\<rbrace>"
-  assumes y: "\<lbrace>P\<rbrace> f \<lbrace>Q\<rbrace>,\<lbrace>F\<rbrace>"
-  shows      "\<lbrace>P\<rbrace> f <handle> handler \<lbrace>Q\<rbrace>,\<lbrace>E\<rbrace>"
-  by (simp add: handleE_def handleE'_wp [OF x y])
-
-lemma hoare_vcg_split_if:
- "\<lbrakk> P \<Longrightarrow> \<lbrace>Q\<rbrace> f \<lbrace>S\<rbrace>; \<not>P \<Longrightarrow> \<lbrace>R\<rbrace> g \<lbrace>S\<rbrace> \<rbrakk> \<Longrightarrow>
-  \<lbrace>\<lambda>s. (P \<longrightarrow> Q s) \<and> (\<not>P \<longrightarrow> R s)\<rbrace> if P then f else g \<lbrace>S\<rbrace>"
-  by simp
-
-lemma hoare_vcg_split_ifE:
- "\<lbrakk> P \<Longrightarrow> \<lbrace>Q\<rbrace> f \<lbrace>S\<rbrace>,\<lbrace>E\<rbrace>; \<not>P \<Longrightarrow> \<lbrace>R\<rbrace> g \<lbrace>S\<rbrace>,\<lbrace>E\<rbrace> \<rbrakk> \<Longrightarrow>
-  \<lbrace>\<lambda>s. (P \<longrightarrow> Q s) \<and> (\<not>P \<longrightarrow> R s)\<rbrace> if P then f else g \<lbrace>S\<rbrace>,\<lbrace>E\<rbrace>"
-  by simp
-
-lemma in_image_constant:
-  "(x \<in> (\<lambda>_. v) ` S) = (x = v \<and> S \<noteq> {})"
-  by (simp add: image_constant_conv)
-
-lemma hoare_liftM_subst: "\<lbrace>P\<rbrace> liftM f m \<lbrace>Q\<rbrace> = \<lbrace>P\<rbrace> m \<lbrace>Q \<circ> f\<rbrace>"
-  apply (simp add: liftM_def bind_def2 return_def split_def mres_def)
-  apply (simp add: valid_def Ball_def mres_def image_Un)
-  apply (simp add: image_image in_image_constant)
-  apply (rule_tac f=All in arg_cong)
-  apply (rule ext)
-  apply force
-  done
-
-lemma liftE_validE[simp]: "\<lbrace>P\<rbrace> liftE f \<lbrace>Q\<rbrace>,\<lbrace>E\<rbrace> = \<lbrace>P\<rbrace> f \<lbrace>Q\<rbrace>"
-  apply (simp add: liftE_liftM validE_def hoare_liftM_subst o_def)
-  done
-
-lemma liftE_wp:
-  "\<lbrace>P\<rbrace> f \<lbrace>Q\<rbrace> \<Longrightarrow> \<lbrace>P\<rbrace> liftE f \<lbrace>Q\<rbrace>,\<lbrace>E\<rbrace>"
-  by simp
-
-lemma liftM_wp: "\<lbrace>P\<rbrace> m \<lbrace>Q \<circ> f\<rbrace> \<Longrightarrow> \<lbrace>P\<rbrace> liftM f m \<lbrace>Q\<rbrace>"
-  by (simp add: hoare_liftM_subst)
-
-lemma hoare_liftME_subst: "\<lbrace>P\<rbrace> liftME f m \<lbrace>Q\<rbrace>,\<lbrace>E\<rbrace> = \<lbrace>P\<rbrace> m \<lbrace>Q \<circ> f\<rbrace>,\<lbrace>E\<rbrace>"
-  apply (simp add: validE_def liftME_liftM hoare_liftM_subst o_def)
-  apply (rule_tac f="valid P m" in arg_cong)
-  apply (rule ext)+
-  apply (case_tac x, simp_all)
-  done
-
-lemma liftME_wp: "\<lbrace>P\<rbrace> m \<lbrace>Q \<circ> f\<rbrace>,\<lbrace>E\<rbrace> \<Longrightarrow> \<lbrace>P\<rbrace> liftME f m \<lbrace>Q\<rbrace>,\<lbrace>E\<rbrace>"
-  by (simp add: hoare_liftME_subst)
-
-(* FIXME: Move *)
-lemma o_const_simp[simp]: "(\<lambda>x. C) \<circ> f = (\<lambda>x. C)"
-  by (simp add: o_def)
-
-lemma hoare_vcg_split_case_option:
- "\<lbrakk> \<And>x. x = None \<Longrightarrow> \<lbrace>P x\<rbrace> f x \<lbrace>R x\<rbrace>;
-    \<And>x y. x = Some y \<Longrightarrow> \<lbrace>Q x y\<rbrace> g x y \<lbrace>R x\<rbrace> \<rbrakk> \<Longrightarrow>
-  \<lbrace>\<lambda>s. (x = None \<longrightarrow> P x s) \<and>
-       (\<forall>y. x = Some y \<longrightarrow> Q x y s)\<rbrace>
-  case x of None \<Rightarrow> f x
-          | Some y \<Rightarrow> g x y
-  \<lbrace>R x\<rbrace>"
- apply(simp add:valid_def split_def)
- apply(case_tac x, simp_all)
-done
-
-lemma hoare_vcg_split_case_optionE:
- assumes none_case: "\<And>x. x = None \<Longrightarrow> \<lbrace>P x\<rbrace> f x \<lbrace>R x\<rbrace>,\<lbrace>E x\<rbrace>"
- assumes some_case: "\<And>x y. x = Some y \<Longrightarrow> \<lbrace>Q x y\<rbrace> g x y \<lbrace>R x\<rbrace>,\<lbrace>E x\<rbrace>"
- shows "\<lbrace>\<lambda>s. (x = None \<longrightarrow> P x s) \<and>
-             (\<forall>y. x = Some y \<longrightarrow> Q x y s)\<rbrace>
-        case x of None \<Rightarrow> f x
-                | Some y \<Rightarrow> g x y
-        \<lbrace>R x\<rbrace>,\<lbrace>E x\<rbrace>"
- apply(case_tac x, simp_all)
-  apply(rule none_case, simp)
- apply(rule some_case, simp)
-done
-
-lemma hoare_vcg_split_case_sum:
- "\<lbrakk> \<And>x a. x = Inl a \<Longrightarrow> \<lbrace>P x a\<rbrace> f x a \<lbrace>R x\<rbrace>;
-    \<And>x b. x = Inr b \<Longrightarrow> \<lbrace>Q x b\<rbrace> g x b \<lbrace>R x\<rbrace> \<rbrakk> \<Longrightarrow>
-  \<lbrace>\<lambda>s. (\<forall>a. x = Inl a \<longrightarrow> P x a s) \<and>
-       (\<forall>b. x = Inr b \<longrightarrow> Q x b s) \<rbrace>
-  case x of Inl a \<Rightarrow> f x a
-          | Inr b \<Rightarrow> g x b
-  \<lbrace>R x\<rbrace>"
- apply(simp add:valid_def split_def)
- apply(case_tac x, simp_all)
-done
-
-lemma hoare_vcg_split_case_sumE:
-  assumes left_case: "\<And>x a. x = Inl a \<Longrightarrow> \<lbrace>P x a\<rbrace> f x a \<lbrace>R x\<rbrace>"
-  assumes right_case: "\<And>x b. x = Inr b \<Longrightarrow> \<lbrace>Q x b\<rbrace> g x b \<lbrace>R x\<rbrace>"
-  shows "\<lbrace>\<lambda>s. (\<forall>a. x = Inl a \<longrightarrow> P x a s) \<and>
-              (\<forall>b. x = Inr b \<longrightarrow> Q x b s) \<rbrace>
-         case x of Inl a \<Rightarrow> f x a
-                 | Inr b \<Rightarrow> g x b
-         \<lbrace>R x\<rbrace>"
- apply(case_tac x, simp_all)
-  apply(rule left_case, simp)
- apply(rule right_case, simp)
-done
-
-lemma hoare_vcg_precond_imp:
- "\<lbrakk> \<lbrace>Q\<rbrace> f \<lbrace>R\<rbrace>; \<And>s. P s \<Longrightarrow> Q s \<rbrakk> \<Longrightarrow> \<lbrace>P\<rbrace> f \<lbrace>R\<rbrace>"
-  by (fastforce simp add:valid_def)
-
-lemma hoare_vcg_precond_impE:
- "\<lbrakk> \<lbrace>Q\<rbrace> f \<lbrace>R\<rbrace>,\<lbrace>E\<rbrace>; \<And>s. P s \<Longrightarrow> Q s \<rbrakk> \<Longrightarrow> \<lbrace>P\<rbrace> f \<lbrace>R\<rbrace>,\<lbrace>E\<rbrace>"
-  by (fastforce simp add:validE_def2)
-
-lemma hoare_seq_ext:
-  assumes g_valid: "\<And>x. \<lbrace>B x\<rbrace> g x \<lbrace>C\<rbrace>"
-  assumes f_valid: "\<lbrace>A\<rbrace> f \<lbrace>B\<rbrace>"
-  shows "\<lbrace>A\<rbrace> do x \<leftarrow> f; g x od \<lbrace>C\<rbrace>"
- apply(insert f_valid g_valid)
- apply(blast intro: seq_ext')
-done
-
-lemma hoare_vcg_seqE:
-  assumes g_valid: "\<And>x. \<lbrace>B x\<rbrace> g x \<lbrace>C\<rbrace>,\<lbrace>E\<rbrace>"
-  assumes f_valid: "\<lbrace>A\<rbrace> f \<lbrace>B\<rbrace>,\<lbrace>E\<rbrace>"
-  shows "\<lbrace>A\<rbrace> doE x \<leftarrow> f; g x odE \<lbrace>C\<rbrace>,\<lbrace>E\<rbrace>"
- apply(insert f_valid g_valid)
- apply(blast intro: seqE')
-done
-
-lemma hoare_seq_ext_nobind:
-  "\<lbrakk> \<lbrace>B\<rbrace> g \<lbrace>C\<rbrace>;
-     \<lbrace>A\<rbrace> f \<lbrace>\<lambda>r s. B s\<rbrace> \<rbrakk> \<Longrightarrow>
-   \<lbrace>A\<rbrace> do f; g od \<lbrace>C\<rbrace>"
-  apply (erule seq_ext)
-  apply (clarsimp simp: valid_def)
-  done
-
-lemma hoare_seq_ext_nobindE:
-  "\<lbrakk> \<lbrace>B\<rbrace> g \<lbrace>C\<rbrace>,\<lbrace>E\<rbrace>;
-     \<lbrace>A\<rbrace> f \<lbrace>\<lambda>r s. B s\<rbrace>,\<lbrace>E\<rbrace> \<rbrakk> \<Longrightarrow>
-   \<lbrace>A\<rbrace> doE f; g odE \<lbrace>C\<rbrace>,\<lbrace>E\<rbrace>"
-  apply (erule seqE)
-  apply (clarsimp simp:validE_def)
-  done
-
-lemma hoare_chain:
-  "\<lbrakk> \<lbrace>P\<rbrace> f \<lbrace>Q\<rbrace>;
-    \<And>s. R s \<Longrightarrow> P s;
-    \<And>r s. Q r s \<Longrightarrow> S r s \<rbrakk> \<Longrightarrow>
-   \<lbrace>R\<rbrace> f \<lbrace>S\<rbrace>"
-  by(fastforce simp add:valid_def split_def)
-
-lemma validE_weaken:
-  "\<lbrakk> \<lbrace>P'\<rbrace> A \<lbrace>Q'\<rbrace>,\<lbrace>E'\<rbrace>; \<And>s. P s \<Longrightarrow> P' s; \<And>r s. Q' r s \<Longrightarrow> Q r s; \<And>r s. E' r s \<Longrightarrow> E r s \<rbrakk> \<Longrightarrow> \<lbrace>P\<rbrace> A \<lbrace>Q\<rbrace>,\<lbrace>E\<rbrace>"
-  by (fastforce simp: validE_def2 split: sum.splits)
-
-lemmas hoare_chainE = validE_weaken
-
-lemma hoare_vcg_handle_elseE:
-  "\<lbrakk> \<lbrace>P\<rbrace> f \<lbrace>Q\<rbrace>,\<lbrace>E\<rbrace>;
-     \<And>e. \<lbrace>E e\<rbrace> g e \<lbrace>R\<rbrace>,\<lbrace>F\<rbrace>;
-     \<And>x. \<lbrace>Q x\<rbrace> h x \<lbrace>R\<rbrace>,\<lbrace>F\<rbrace> \<rbrakk> \<Longrightarrow>
-   \<lbrace>P\<rbrace> f <handle> g <else> h \<lbrace>R\<rbrace>,\<lbrace>F\<rbrace>"
-  apply (simp add: handle_elseE_def validE_def)
-  apply (rule seq_ext)
-   apply assumption
-  apply (simp split: sum.split)
-  done
-
-lemma in_mres:
-  "(tr, Result (rv, s)) \<in> S \<Longrightarrow> (rv, s) \<in> mres S"
-  by (fastforce simp: mres_def intro: image_eqI[rotated])
-
-lemma alternative_wp:
-  assumes x: "\<lbrace>P\<rbrace> f \<lbrace>Q\<rbrace>"
-  assumes y: "\<lbrace>P'\<rbrace> f' \<lbrace>Q\<rbrace>"
-  shows      "\<lbrace>P and P'\<rbrace> f \<sqinter> f' \<lbrace>Q\<rbrace>"
-  unfolding valid_def alternative_def mres_def
-  using post_by_hoare[OF x _ in_mres] post_by_hoare[OF y _ in_mres]
-  by fastforce
-
-lemma alternativeE_wp:
-  assumes x: "\<lbrace>P\<rbrace> f \<lbrace>Q\<rbrace>,\<lbrace>E\<rbrace>" and y: "\<lbrace>P'\<rbrace> f' \<lbrace>Q\<rbrace>,\<lbrace>E\<rbrace>"
-  shows      "\<lbrace>P and P'\<rbrace> f \<sqinter> f' \<lbrace>Q\<rbrace>,\<lbrace>E\<rbrace>"
-  apply (unfold validE_def)
-  apply (wp add: x y alternative_wp | simp | fold validE_def)+
-  done
-
-lemma alternativeE_R_wp:
-  "\<lbrakk> \<lbrace>P\<rbrace> f \<lbrace>Q\<rbrace>,-; \<lbrace>P'\<rbrace> f' \<lbrace>Q\<rbrace>,- \<rbrakk> \<Longrightarrow> \<lbrace>P and P'\<rbrace> f \<sqinter> f' \<lbrace>Q\<rbrace>,-"
-  apply (simp add: validE_R_def)
-  apply (rule alternativeE_wp)
-   apply assumption+
-  done
-
-lemma alternative_R_wp:
-  "\<lbrakk> \<lbrace>P\<rbrace> f -,\<lbrace>Q\<rbrace>; \<lbrace>P'\<rbrace> g -,\<lbrace>Q\<rbrace> \<rbrakk> \<Longrightarrow> \<lbrace>P and P'\<rbrace> f \<sqinter> g -, \<lbrace>Q\<rbrace>"
-  apply (simp add: validE_E_def)
-  apply (rule alternativeE_wp)
-   apply assumption+
-  done
-
-lemma state_select_wp [wp]: "\<lbrace> \<lambda>s. \<forall>t. (s, t) \<in> f \<longrightarrow> P () t \<rbrace> state_select f \<lbrace> P \<rbrace>"
-  apply (clarsimp simp: state_select_def assert_def)
-  apply (rule hoare_weaken_pre)
-   apply (wp select_wp hoare_vcg_split_if return_wp fail_wp)
-  apply simp
-  done
-
-lemma condition_wp [wp]:
-  "\<lbrakk> \<lbrace> Q \<rbrace> A \<lbrace> P \<rbrace>;  \<lbrace> R \<rbrace> B \<lbrace> P \<rbrace>  \<rbrakk> \<Longrightarrow> \<lbrace> \<lambda>s. if C s then Q s else R s \<rbrace> condition C A B \<lbrace> P \<rbrace>"
-  apply (clarsimp simp: condition_def)
-  apply (clarsimp simp: valid_def pred_conj_def pred_neg_def split_def)
-  done
-
-lemma conditionE_wp [wp]:
-  "\<lbrakk> \<lbrace> P \<rbrace> A \<lbrace> Q \<rbrace>,\<lbrace> R \<rbrace>; \<lbrace> P' \<rbrace> B \<lbrace> Q \<rbrace>,\<lbrace> R \<rbrace> \<rbrakk> \<Longrightarrow>  \<lbrace> \<lambda>s. if C s then P s else P' s \<rbrace> condition C A B \<lbrace>Q\<rbrace>,\<lbrace>R\<rbrace>"
-  apply (clarsimp simp: condition_def)
-  apply (clarsimp simp: validE_def valid_def)
-  done
-
-lemma state_assert_wp [wp]: "\<lbrace> \<lambda>s. f s \<longrightarrow> P () s \<rbrace> state_assert f \<lbrace> P \<rbrace>"
-  apply (clarsimp simp: state_assert_def get_def
-    assert_def bind_def valid_def return_def fail_def mres_def)
-  done
-
-text \<open>The weakest precondition handler which works on conjunction\<close>
-
-lemma hoare_vcg_conj_lift:
-  assumes x: "\<lbrace>P\<rbrace> f \<lbrace>Q\<rbrace>"
-  assumes y: "\<lbrace>P'\<rbrace> f \<lbrace>Q'\<rbrace>"
-  shows      "\<lbrace>\<lambda>s. P s \<and> P' s\<rbrace> f \<lbrace>\<lambda>rv s. Q rv s \<and> Q' rv s\<rbrace>"
-  apply (subst pred_conj_def[symmetric], subst pred_conj_def[symmetric], rule hoare_post_conj)
-   apply (rule hoare_pre_imp [OF _ x], simp)
-  apply (rule hoare_pre_imp [OF _ y], simp)
-  done
-
-lemma hoare_vcg_conj_liftE1:
-  "\<lbrakk> \<lbrace>P\<rbrace> f \<lbrace>Q\<rbrace>,-; \<lbrace>P'\<rbrace> f \<lbrace>Q'\<rbrace>,\<lbrace>E\<rbrace> \<rbrakk> \<Longrightarrow>
-  \<lbrace>P and P'\<rbrace> f \<lbrace>\<lambda>r s. Q r s \<and> Q' r s\<rbrace>,\<lbrace>E\<rbrace>"
-  unfolding valid_def validE_R_def validE_def
-  apply (clarsimp simp: split_def split: sum.splits)
-  apply (erule allE, erule (1) impE)
-  apply (erule allE, erule (1) impE)
-  apply (drule (1) bspec)
-  apply (drule (1) bspec)
-  apply clarsimp
-  done
-
-lemma hoare_vcg_disj_lift:
-  assumes x: "\<lbrace>P\<rbrace>  f \<lbrace>Q\<rbrace>"
-  assumes y: "\<lbrace>P'\<rbrace> f \<lbrace>Q'\<rbrace>"
-  shows      "\<lbrace>\<lambda>s. P s \<or> P' s\<rbrace> f \<lbrace>\<lambda>rv s. Q rv s \<or> Q' rv s\<rbrace>"
-  apply (simp add: valid_def)
-  apply safe
-   apply (erule(1) post_by_hoare [OF x])
-  apply (erule notE)
-  apply (erule(1) post_by_hoare [OF y])
-  done
-
-lemma hoare_vcg_const_Ball_lift:
-  "\<lbrakk> \<And>x. x \<in> S \<Longrightarrow> \<lbrace>P x\<rbrace> f \<lbrace>Q x\<rbrace> \<rbrakk> \<Longrightarrow> \<lbrace>\<lambda>s. \<forall>x\<in>S. P x s\<rbrace> f \<lbrace>\<lambda>rv s. \<forall>x\<in>S. Q x rv s\<rbrace>"
-  by (fastforce simp: valid_def)
-
-lemma hoare_vcg_const_Ball_lift_R:
- "\<lbrakk> \<And>x. x \<in> S \<Longrightarrow> \<lbrace>P x\<rbrace> f \<lbrace>Q x\<rbrace>,- \<rbrakk> \<Longrightarrow>
-   \<lbrace>\<lambda>s. \<forall>x \<in> S. P x s\<rbrace> f \<lbrace>\<lambda>rv s. \<forall>x \<in> S. Q x rv s\<rbrace>,-"
-  apply (simp add: validE_R_def validE_def)
-  apply (rule hoare_strengthen_post)
-   apply (erule hoare_vcg_const_Ball_lift)
-  apply (simp split: sum.splits)
-  done
-
-lemma hoare_vcg_all_lift:
-  "\<lbrakk> \<And>x. \<lbrace>P x\<rbrace> f \<lbrace>Q x\<rbrace> \<rbrakk> \<Longrightarrow> \<lbrace>\<lambda>s. \<forall>x. P x s\<rbrace> f \<lbrace>\<lambda>rv s. \<forall>x. Q x rv s\<rbrace>"
-  by (fastforce simp: valid_def)
-
-lemma hoare_vcg_all_lift_R:
-  "(\<And>x. \<lbrace>P x\<rbrace> f \<lbrace>Q x\<rbrace>, -) \<Longrightarrow> \<lbrace>\<lambda>s. \<forall>x. P x s\<rbrace> f \<lbrace>\<lambda>rv s. \<forall>x. Q x rv s\<rbrace>, -"
-  by (rule hoare_vcg_const_Ball_lift_R[where S=UNIV, simplified])
-
-lemma hoare_vcg_const_imp_lift:
-  "\<lbrakk> P \<Longrightarrow> \<lbrace>Q\<rbrace> m \<lbrace>R\<rbrace> \<rbrakk> \<Longrightarrow>
-   \<lbrace>\<lambda>s. P \<longrightarrow> Q s\<rbrace> m \<lbrace>\<lambda>rv s. P \<longrightarrow> R rv s\<rbrace>"
-  by (cases P, simp_all add: hoare_vcg_prop)
-
-lemma hoare_vcg_const_imp_lift_R:
-  "(P \<Longrightarrow> \<lbrace>Q\<rbrace> m \<lbrace>R\<rbrace>,-) \<Longrightarrow> \<lbrace>\<lambda>s. P \<longrightarrow> Q s\<rbrace> m \<lbrace>\<lambda>rv s. P \<longrightarrow> R rv s\<rbrace>,-"
-  by (fastforce simp: validE_R_def validE_def valid_def split_def split: sum.splits)
-
-lemma hoare_weak_lift_imp:
-  "\<lbrace>P'\<rbrace> f \<lbrace>Q\<rbrace> \<Longrightarrow> \<lbrace>\<lambda>s. P \<longrightarrow> P' s\<rbrace> f \<lbrace>\<lambda>rv s. P \<longrightarrow> Q rv s\<rbrace>"
-  by (auto simp add: valid_def split_def)
-
-lemma hoare_vcg_ex_lift:
-  "\<lbrakk> \<And>x. \<lbrace>P x\<rbrace> f \<lbrace>Q x\<rbrace> \<rbrakk> \<Longrightarrow> \<lbrace>\<lambda>s. \<exists>x. P x s\<rbrace> f \<lbrace>\<lambda>rv s. \<exists>x. Q x rv s\<rbrace>"
-  by (clarsimp simp: valid_def, blast)
-
-lemma hoare_vcg_ex_lift_R1:
-  "(\<And>x. \<lbrace>P x\<rbrace> f \<lbrace>Q\<rbrace>, -) \<Longrightarrow> \<lbrace>\<lambda>s. \<exists>x. P x s\<rbrace> f \<lbrace>Q\<rbrace>, -"
-  by (fastforce simp: valid_def validE_R_def validE_def split: sum.splits)
-
-(* for instantiations *)
-lemma hoare_triv:    "\<lbrace>P\<rbrace>f\<lbrace>Q\<rbrace> \<Longrightarrow> \<lbrace>P\<rbrace>f\<lbrace>Q\<rbrace>" .
-lemma hoare_trivE:   "\<lbrace>P\<rbrace> f \<lbrace>Q\<rbrace>,\<lbrace>E\<rbrace> \<Longrightarrow> \<lbrace>P\<rbrace> f \<lbrace>Q\<rbrace>,\<lbrace>E\<rbrace>" .
-lemma hoare_trivE_R: "\<lbrace>P\<rbrace> f \<lbrace>Q\<rbrace>,- \<Longrightarrow> \<lbrace>P\<rbrace> f \<lbrace>Q\<rbrace>,-" .
-lemma hoare_trivR_R: "\<lbrace>P\<rbrace> f -,\<lbrace>E\<rbrace> \<Longrightarrow> \<lbrace>P\<rbrace> f -,\<lbrace>E\<rbrace>" .
-
-lemma hoare_weaken_preE_E:
-  "\<lbrakk> \<lbrace>P'\<rbrace> f -,\<lbrace>Q\<rbrace>; \<And>s. P s \<Longrightarrow> P' s \<rbrakk> \<Longrightarrow> \<lbrace>P\<rbrace> f -,\<lbrace>Q\<rbrace>"
-  by (fastforce simp add: validE_E_def validE_def valid_def)
-
-lemma hoare_vcg_E_conj:
-  "\<lbrakk> \<lbrace>P\<rbrace> f -,\<lbrace>E\<rbrace>; \<lbrace>P'\<rbrace> f \<lbrace>Q'\<rbrace>,\<lbrace>E'\<rbrace> \<rbrakk>
-    \<Longrightarrow> \<lbrace>\<lambda>s. P s \<and> P' s\<rbrace> f \<lbrace>Q'\<rbrace>, \<lbrace>\<lambda>rv s. E rv s \<and> E' rv s\<rbrace>"
-  apply (unfold validE_def validE_E_def)
-  apply (rule hoare_post_imp [OF _ hoare_vcg_conj_lift], simp_all)
-  apply (case_tac r, simp_all)
-  done
-
-lemma hoare_vcg_E_elim:
-  "\<lbrakk> \<lbrace>P\<rbrace> f -,\<lbrace>E\<rbrace>; \<lbrace>P'\<rbrace> f \<lbrace>Q\<rbrace>,- \<rbrakk>
-    \<Longrightarrow> \<lbrace>\<lambda>s. P s \<and> P' s\<rbrace> f \<lbrace>Q\<rbrace>,\<lbrace>E\<rbrace>"
-  by (rule hoare_post_impErr [OF hoare_vcg_E_conj],
-      (simp add: validE_R_def)+)
-
-lemma hoare_vcg_R_conj:
-  "\<lbrakk> \<lbrace>P\<rbrace> f \<lbrace>Q\<rbrace>,-; \<lbrace>P'\<rbrace> f \<lbrace>Q'\<rbrace>,- \<rbrakk>
-    \<Longrightarrow> \<lbrace>\<lambda>s. P s \<and> P' s\<rbrace> f \<lbrace>\<lambda>rv s. Q rv s \<and> Q' rv s\<rbrace>,-"
-  apply (unfold validE_R_def validE_def)
-  apply (rule hoare_post_imp [OF _ hoare_vcg_conj_lift], simp_all)
-  apply (case_tac r, simp_all)
-  done
-
-lemma valid_validE:
-  "\<lbrace>P\<rbrace> f \<lbrace>\<lambda>rv. Q\<rbrace> \<Longrightarrow> \<lbrace>P\<rbrace> f \<lbrace>\<lambda>rv. Q\<rbrace>,\<lbrace>\<lambda>rv. Q\<rbrace>"
-  apply (simp add: validE_def)
-  done
-
-lemma valid_validE2:
-  "\<lbrakk> \<lbrace>P\<rbrace> f \<lbrace>\<lambda>_. Q'\<rbrace>; \<And>s. Q' s \<Longrightarrow> Q s; \<And>s. Q' s \<Longrightarrow> E s \<rbrakk> \<Longrightarrow> \<lbrace>P\<rbrace> f \<lbrace>\<lambda>_. Q\<rbrace>,\<lbrace>\<lambda>_. E\<rbrace>"
-  unfolding valid_def validE_def
-  by (clarsimp split: sum.splits) blast
-
-lemma validE_valid: "\<lbrace>P\<rbrace> f \<lbrace>\<lambda>rv. Q\<rbrace>,\<lbrace>\<lambda>rv. Q\<rbrace> \<Longrightarrow> \<lbrace>P\<rbrace> f \<lbrace>\<lambda>rv. Q\<rbrace>"
-  apply (unfold validE_def)
-  apply (rule hoare_post_imp)
-   defer
-   apply assumption
-  apply (case_tac r, simp_all)
-  done
-
-lemma valid_validE_R:
-  "\<lbrace>P\<rbrace> f \<lbrace>\<lambda>rv. Q\<rbrace> \<Longrightarrow> \<lbrace>P\<rbrace> f \<lbrace>\<lambda>rv. Q\<rbrace>,-"
-  by (simp add: validE_R_def hoare_post_impErr [OF valid_validE])
-
-lemma valid_validE_E:
-  "\<lbrace>P\<rbrace> f \<lbrace>\<lambda>rv. Q\<rbrace> \<Longrightarrow> \<lbrace>P\<rbrace> f -,\<lbrace>\<lambda>rv. Q\<rbrace>"
-  by (simp add: validE_E_def hoare_post_impErr [OF valid_validE])
-
-lemma validE_validE_R: "\<lbrace>P\<rbrace> f \<lbrace>Q\<rbrace>,\<lbrace>\<top>\<top>\<rbrace> \<Longrightarrow> \<lbrace>P\<rbrace> f \<lbrace>Q\<rbrace>,-"
-  by (simp add: validE_R_def)
-
-lemma validE_R_validE: "\<lbrace>P\<rbrace> f \<lbrace>Q\<rbrace>,- \<Longrightarrow> \<lbrace>P\<rbrace> f \<lbrace>Q\<rbrace>,\<lbrace>\<top>\<top>\<rbrace>"
-  by (simp add: validE_R_def)
-
-lemma hoare_post_imp_R: "\<lbrakk> \<lbrace>P\<rbrace> f \<lbrace>Q'\<rbrace>,-; \<And>r s. Q' r s \<Longrightarrow> Q r s \<rbrakk> \<Longrightarrow> \<lbrace>P\<rbrace> f \<lbrace>Q\<rbrace>,-"
-  apply (unfold validE_R_def)
-  apply (rule hoare_post_impErr, simp+)
-  done
-
-lemma hoare_post_comb_imp_conj:
-  "\<lbrakk> \<lbrace>P'\<rbrace> f \<lbrace>Q\<rbrace>; \<lbrace>P\<rbrace> f \<lbrace>Q'\<rbrace>; \<And>s. P s \<Longrightarrow> P' s \<rbrakk> \<Longrightarrow> \<lbrace>P\<rbrace> f \<lbrace>\<lambda>rv s. Q rv s \<and> Q' rv s\<rbrace>"
-  apply (rule hoare_pre_imp)
-   defer
-   apply (rule hoare_vcg_conj_lift)
-    apply assumption+
-  apply simp
-  done
-
-lemma hoare_vcg_precond_impE_R: "\<lbrakk> \<lbrace>P'\<rbrace> f \<lbrace>Q\<rbrace>,-; \<And>s. P s \<Longrightarrow> P' s \<rbrakk> \<Longrightarrow> \<lbrace>P\<rbrace> f \<lbrace>Q\<rbrace>,-"
-  by (unfold validE_R_def, rule hoare_vcg_precond_impE, simp+)
-
-(* lemma valid_is_triple:
-  "valid P f Q = triple_judgement P f (postcondition Q (\<lambda>s f. fst (f s)))"
-  by (simp add: triple_judgement_def valid_def postcondition_def)
- *)
-
-lemma validE_is_triple:
-  "validE P f Q E = triple_judgement P f
-    (postconditions (\<lambda>s f. (\<forall>(r,s') \<in> {(rv, s'). (Inr rv, s') \<in> (mres (f s))}. Q r s'))
-          (\<lambda>s f. (\<forall>(r,s') \<in> {(rv, s'). (Inl rv, s') \<in> (mres (f s))}. E r s')))"
-  apply (simp add: validE_def triple_judgement_def valid_def postcondition_def
-                   postconditions_def split_def split: sum.split)
-  apply (fastforce elim: image_eqI[rotated])
-  done
-
-lemma validE_R_is_triple:
-  "validE_R P f Q = triple_judgement P f
-     (\<lambda>s f. (\<forall>(r,s') \<in> {(rv, s'). (Inr rv, s') \<in> mres (f s)}. Q r s'))"
-  by (simp add: validE_R_def validE_is_triple postconditions_def postcondition_def)
-
-lemma validE_E_is_triple:
-  "validE_E P f E = triple_judgement P f
-     (\<lambda>s f. (\<forall>(r,s') \<in> {(rv, s'). (Inl rv, s') \<in> mres (f s)}. E r s'))"
-  by (simp add: validE_E_def validE_is_triple postconditions_def postcondition_def)
-
-lemmas hoare_wp_combs =
-  hoare_post_comb_imp_conj hoare_vcg_precond_imp hoare_vcg_conj_lift
-
-lemmas hoare_wp_combsE =
-  hoare_vcg_precond_impE
-  hoare_vcg_precond_impE_R
-  validE_validE_R
-  hoare_vcg_R_conj
-  hoare_vcg_E_elim
-  hoare_vcg_E_conj
-
-lemmas hoare_wp_state_combsE =
-  hoare_vcg_precond_impE[OF valid_validE]
-  hoare_vcg_precond_impE_R[OF valid_validE_R]
-  valid_validE_R
-  hoare_vcg_R_conj[OF valid_validE_R]
-  hoare_vcg_E_elim[OF valid_validE_E]
-  hoare_vcg_E_conj[OF valid_validE_E]
-
-lemmas hoare_wp_splits [wp_split] =
-  hoare_seq_ext hoare_vcg_seqE handleE'_wp handleE_wp
-  validE_validE_R [OF hoare_vcg_seqE [OF validE_R_validE]]
-  validE_validE_R [OF handleE'_wp [OF validE_R_validE]]
-  validE_validE_R [OF handleE_wp [OF validE_R_validE]]
-  catch_wp hoare_vcg_split_if hoare_vcg_split_ifE
-  validE_validE_R [OF hoare_vcg_split_ifE [OF validE_R_validE validE_R_validE]]
-  liftM_wp liftME_wp
-  validE_validE_R [OF liftME_wp [OF validE_R_validE]]
-  validE_valid
-
-lemmas [wp_comb] = hoare_wp_state_combsE hoare_wp_combsE  hoare_wp_combs
-
-lemmas [wp] = hoare_vcg_prop
-              wp_post_taut
-              return_wp
-              put_wp
-              get_wp
-              gets_wp
-              modify_wp
-              returnOk_wp
-              throwError_wp
-              fail_wp
-              failE_wp
-              liftE_wp
-
-lemmas [wp_trip] = valid_is_triple validE_is_triple validE_E_is_triple validE_R_is_triple
-
-
-text \<open>Simplifications on conjunction\<close>
-
-lemma hoare_post_eq: "\<lbrakk> Q = Q'; \<lbrace>P\<rbrace> f \<lbrace>Q'\<rbrace> \<rbrakk> \<Longrightarrow> \<lbrace>P\<rbrace> f \<lbrace>Q\<rbrace>"
-  by simp
-lemma hoare_post_eqE1: "\<lbrakk> Q = Q'; \<lbrace>P\<rbrace> f \<lbrace>Q'\<rbrace>,\<lbrace>E\<rbrace> \<rbrakk> \<Longrightarrow> \<lbrace>P\<rbrace> f \<lbrace>Q\<rbrace>,\<lbrace>E\<rbrace>"
-  by simp
-lemma hoare_post_eqE2: "\<lbrakk> E = E'; \<lbrace>P\<rbrace> f \<lbrace>Q\<rbrace>,\<lbrace>E'\<rbrace> \<rbrakk> \<Longrightarrow> \<lbrace>P\<rbrace> f \<lbrace>Q\<rbrace>,\<lbrace>E\<rbrace>"
-  by simp
-lemma hoare_post_eqE_R: "\<lbrakk> Q = Q'; \<lbrace>P\<rbrace> f \<lbrace>Q'\<rbrace>,- \<rbrakk> \<Longrightarrow> \<lbrace>P\<rbrace> f \<lbrace>Q\<rbrace>,-"
-  by simp
-
-lemma pred_conj_apply_elim: "(\<lambda>r. Q r and Q' r) = (\<lambda>r s. Q r s \<and> Q' r s)"
-  by (simp add: pred_conj_def)
-lemma pred_conj_conj_elim: "(\<lambda>r s. (Q r and Q' r) s \<and> Q'' r s) = (\<lambda>r s. Q r s \<and> Q' r s \<and> Q'' r s)"
-  by simp
-lemma conj_assoc_apply: "(\<lambda>r s. (Q r s \<and> Q' r s) \<and> Q'' r s) = (\<lambda>r s. Q r s \<and> Q' r s \<and> Q'' r s)"
-  by simp
-lemma all_elim: "(\<lambda>rv s. \<forall>x. P rv s) = P"
-  by simp
-lemma all_conj_elim: "(\<lambda>rv s. (\<forall>x. P rv s) \<and> Q rv s) = (\<lambda>rv s. P rv s \<and> Q rv s)"
-  by simp
-
-lemmas vcg_rhs_simps = pred_conj_apply_elim pred_conj_conj_elim
-          conj_assoc_apply all_elim all_conj_elim
-
-lemma if_apply_reduct: "\<lbrace>P\<rbrace> If P' (f x) (g x) \<lbrace>Q\<rbrace> \<Longrightarrow> \<lbrace>P\<rbrace> If P' f g x \<lbrace>Q\<rbrace>"
-  by (cases P', simp_all)
-lemma if_apply_reductE: "\<lbrace>P\<rbrace> If P' (f x) (g x) \<lbrace>Q\<rbrace>,\<lbrace>E\<rbrace> \<Longrightarrow> \<lbrace>P\<rbrace> If P' f g x \<lbrace>Q\<rbrace>,\<lbrace>E\<rbrace>"
-  by (cases P', simp_all)
-lemma if_apply_reductE_R: "\<lbrace>P\<rbrace> If P' (f x) (g x) \<lbrace>Q\<rbrace>,- \<Longrightarrow> \<lbrace>P\<rbrace> If P' f g x \<lbrace>Q\<rbrace>,-"
-  by (cases P', simp_all)
-
-lemmas hoare_wp_simps [wp_split] =
-  vcg_rhs_simps [THEN hoare_post_eq] vcg_rhs_simps [THEN hoare_post_eqE1]
-  vcg_rhs_simps [THEN hoare_post_eqE2] vcg_rhs_simps [THEN hoare_post_eqE_R]
-  if_apply_reduct if_apply_reductE if_apply_reductE_R TrueI
-
-schematic_goal if_apply_test: "\<lbrace>?Q\<rbrace> (if A then returnOk else K fail) x \<lbrace>P\<rbrace>,\<lbrace>E\<rbrace>"
-  by wpsimp
-
-lemma hoare_elim_pred_conj:
-  "\<lbrace>P\<rbrace> f \<lbrace>\<lambda>r s. Q r s \<and> Q' r s\<rbrace> \<Longrightarrow> \<lbrace>P\<rbrace> f \<lbrace>\<lambda>r. Q r and Q' r\<rbrace>"
-  by (unfold pred_conj_def)
-
-lemma hoare_elim_pred_conjE1:
-  "\<lbrace>P\<rbrace> f \<lbrace>\<lambda>r s. Q r s \<and> Q' r s\<rbrace>,\<lbrace>E\<rbrace> \<Longrightarrow> \<lbrace>P\<rbrace> f \<lbrace>\<lambda>r. Q r and Q' r\<rbrace>,\<lbrace>E\<rbrace>"
-  by (unfold pred_conj_def)
-
-lemma hoare_elim_pred_conjE2:
-  "\<lbrace>P\<rbrace> f \<lbrace>Q\<rbrace>, \<lbrace>\<lambda>x s. E x s \<and> E' x s\<rbrace> \<Longrightarrow> \<lbrace>P\<rbrace> f \<lbrace>Q\<rbrace>,\<lbrace>\<lambda>x. E x and E' x\<rbrace>"
-  by (unfold pred_conj_def)
-
-lemma hoare_elim_pred_conjE_R:
-  "\<lbrace>P\<rbrace> f \<lbrace>\<lambda>r s. Q r s \<and> Q' r s\<rbrace>,- \<Longrightarrow> \<lbrace>P\<rbrace> f \<lbrace>\<lambda>r. Q r and Q' r\<rbrace>,-"
-  by (unfold pred_conj_def)
-
-lemmas hoare_wp_pred_conj_elims =
-  hoare_elim_pred_conj hoare_elim_pred_conjE1
-  hoare_elim_pred_conjE2 hoare_elim_pred_conjE_R
-
-lemmas hoare_weaken_preE = hoare_vcg_precond_impE
-
-lemmas hoare_pre [wp_pre] =
-  hoare_weaken_pre
-  hoare_weaken_preE
-  hoare_vcg_precond_impE_R
-  hoare_weaken_preE_E
-
-declare no_fail_pre [wp_pre]
-
-bundle no_pre = hoare_pre [wp_pre del] no_fail_pre [wp_pre del]
-
-text \<open>Miscellaneous lemmas on hoare triples\<close>
-
-lemma hoare_vcg_mp:
-  assumes a: "\<lbrace>P\<rbrace> f \<lbrace>Q\<rbrace>"
-  assumes b: "\<lbrace>P\<rbrace> f \<lbrace>\<lambda>r s. Q r s \<longrightarrow> Q' r s\<rbrace>"
-  shows "\<lbrace>P\<rbrace> f \<lbrace>Q'\<rbrace>"
-  using assms
-  by (auto simp: valid_def split_def)
-
-(* note about this precond stuff: rules get a chance to bind directly
-   before any of their combined forms. As a result, these precondition
-   implication rules are only used when needed. *)
-
-lemma hoare_add_post:
-  assumes r: "\<lbrace>P'\<rbrace> f \<lbrace>Q'\<rbrace>"
-  assumes impP: "\<And>s. P s \<Longrightarrow> P' s"
-  assumes impQ: "\<lbrace>P\<rbrace> f \<lbrace>\<lambda>rv s. Q' rv s \<longrightarrow> Q rv s\<rbrace>"
-  shows "\<lbrace>P\<rbrace> f \<lbrace>Q\<rbrace>"
-  apply (rule hoare_chain)
-    apply (rule hoare_vcg_conj_lift)
-     apply (rule r)
-    apply (rule impQ)
-   apply simp
-   apply (erule impP)
-  apply simp
-  done
-
-lemma whenE_wp:
-  "(P \<Longrightarrow> \<lbrace>Q\<rbrace> f \<lbrace>R\<rbrace>, \<lbrace>E\<rbrace>) \<Longrightarrow> \<lbrace>if P then Q else R ()\<rbrace> whenE P f \<lbrace>R\<rbrace>, \<lbrace>E\<rbrace>"
-  unfolding whenE_def by clarsimp wp
-
-lemma hoare_gen_asmE:
-  "(P \<Longrightarrow> \<lbrace>P'\<rbrace> f \<lbrace>Q\<rbrace>,-) \<Longrightarrow> \<lbrace>P' and K P\<rbrace> f \<lbrace>Q\<rbrace>, -"
-  by (simp add: validE_R_def validE_def valid_def) blast
-
-lemma hoare_list_case:
-  assumes P1: "\<lbrace>P1\<rbrace> f f1 \<lbrace>Q\<rbrace>"
-  assumes P2: "\<And>y ys. xs = y#ys \<Longrightarrow> \<lbrace>P2 y ys\<rbrace> f (f2 y ys) \<lbrace>Q\<rbrace>"
-  shows "\<lbrace>case xs of [] \<Rightarrow> P1 | y#ys \<Rightarrow> P2 y ys\<rbrace>
-         f (case xs of [] \<Rightarrow> f1 | y#ys \<Rightarrow> f2 y ys)
-         \<lbrace>Q\<rbrace>"
-  apply (cases xs; simp)
-   apply (rule P1)
-  apply (rule P2)
-  apply simp
-  done
-
-lemma unless_wp:
-  "(\<not>P \<Longrightarrow> \<lbrace>Q\<rbrace> f \<lbrace>R\<rbrace>) \<Longrightarrow> \<lbrace>if P then R () else Q\<rbrace> unless P f \<lbrace>R\<rbrace>"
-  unfolding unless_def by wp auto
-
-lemma hoare_use_eq:
-  assumes x: "\<And>P. \<lbrace>\<lambda>s. P (f s)\<rbrace> m \<lbrace>\<lambda>rv s. P (f s)\<rbrace>"
-  assumes y: "\<And>f. \<lbrace>\<lambda>s. P f s\<rbrace> m \<lbrace>\<lambda>rv s. Q f s\<rbrace>"
-  shows "\<lbrace>\<lambda>s. P (f s) s\<rbrace> m \<lbrace>\<lambda>rv s. Q (f s :: 'c :: type) s \<rbrace>"
-  apply (rule_tac Q="\<lambda>rv s. \<exists>f'. f' = f s \<and> Q f' s" in hoare_post_imp)
-   apply simp
-  apply (wpsimp wp: hoare_vcg_ex_lift x y)
-  done
-
-lemma hoare_return_sp:
-  "\<lbrace>P\<rbrace> return x \<lbrace>\<lambda>r. P and K (r = x)\<rbrace>"
-  by (simp add: valid_def return_def mres_def)
-
-lemma hoare_fail_any [simp]:
-  "\<lbrace>P\<rbrace> fail \<lbrace>Q\<rbrace>" by wp
-
-lemma hoare_failE [simp]: "\<lbrace>P\<rbrace> fail \<lbrace>Q\<rbrace>,\<lbrace>E\<rbrace>" by  wp
-
-lemma hoare_FalseE [simp]:
-  "\<lbrace>\<lambda>s. False\<rbrace> f \<lbrace>Q\<rbrace>,\<lbrace>E\<rbrace>"
-  by (simp add: valid_def validE_def)
-
-lemma hoare_K_bind [wp]:
-  "\<lbrace>P\<rbrace> f \<lbrace>Q\<rbrace> \<Longrightarrow> \<lbrace>P\<rbrace> K_bind f x \<lbrace>Q\<rbrace>"
-  by simp
-
-text \<open>Setting up the precondition case splitter.\<close>
-
-lemma wpc_helper_valid:
-  "\<lbrace>Q\<rbrace> g \<lbrace>S\<rbrace> \<Longrightarrow> wpc_helper (P, P', P'') (Q, Q', Q'') \<lbrace>P\<rbrace> g \<lbrace>S\<rbrace>"
-  by (clarsimp simp: wpc_helper_def elim!: hoare_pre)
-
-lemma wpc_helper_validE:
-  "\<lbrace>Q\<rbrace> f \<lbrace>R\<rbrace>,\<lbrace>E\<rbrace> \<Longrightarrow> wpc_helper (P, P', P'') (Q, Q', Q'') \<lbrace>P\<rbrace> f \<lbrace>R\<rbrace>,\<lbrace>E\<rbrace>"
-  by (clarsimp simp: wpc_helper_def elim!: hoare_pre)
-
-lemma wpc_helper_validE_R:
-  "\<lbrace>Q\<rbrace> f \<lbrace>R\<rbrace>,- \<Longrightarrow> wpc_helper (P, P', P'') (Q, Q', Q'') \<lbrace>P\<rbrace> f \<lbrace>R\<rbrace>,-"
-  by (clarsimp simp: wpc_helper_def elim!: hoare_pre)
-
-lemma wpc_helper_validR_R:
-  "\<lbrace>Q\<rbrace> f -,\<lbrace>E\<rbrace> \<Longrightarrow> wpc_helper (P, P', P'') (Q, Q', Q'') \<lbrace>P\<rbrace> f -,\<lbrace>E\<rbrace>"
-  by (clarsimp simp: wpc_helper_def elim!: hoare_pre)
-
-lemma wpc_helper_no_fail_final:
-  "no_fail Q f \<Longrightarrow> wpc_helper (P, P', P'') (Q, Q', Q'') (no_fail P f)"
-  by (clarsimp simp: wpc_helper_def elim!: no_fail_pre)
-
-lemma wpc_helper_validNF:
-  "\<lbrace>Q\<rbrace> g \<lbrace>S\<rbrace>! \<Longrightarrow> wpc_helper (P, P', P'') (Q, Q', Q'') \<lbrace>P\<rbrace> g \<lbrace>S\<rbrace>!"
-  apply (clarsimp simp: wpc_helper_def)
-  by (metis hoare_wp_combs(2) no_fail_pre validNF_def)
-
 (* FIXME: this needs adjustment, case_prod Q is unlikely to unify *)
 lemma wpc_helper_validI:
   "(\<lbrace>Q\<rbrace>,\<lbrace>R\<rbrace> g \<lbrace>G\<rbrace>,\<lbrace>S\<rbrace>) \<Longrightarrow> wpc_helper (P, P', P'') (case_prod Q, Q', Q'') (\<lbrace>curry P\<rbrace>,\<lbrace>R\<rbrace> g \<lbrace>G\<rbrace>,\<lbrace>S\<rbrace>)"
   by (clarsimp simp: wpc_helper_def elim!: validI_weaken_pre)
 
-wpc_setup "\<lambda>m. \<lbrace>P\<rbrace> m \<lbrace>Q\<rbrace>" wpc_helper_valid
-wpc_setup "\<lambda>m. \<lbrace>P\<rbrace> m \<lbrace>Q\<rbrace>,\<lbrace>E\<rbrace>" wpc_helper_validE
-wpc_setup "\<lambda>m. \<lbrace>P\<rbrace> m \<lbrace>Q\<rbrace>,-" wpc_helper_validE_R
-wpc_setup "\<lambda>m. \<lbrace>P\<rbrace> m -,\<lbrace>E\<rbrace>" wpc_helper_validR_R
-wpc_setup "\<lambda>m. no_fail P m" wpc_helper_no_fail_final
-wpc_setup "\<lambda>m. \<lbrace>P\<rbrace> m \<lbrace>Q\<rbrace>!" wpc_helper_validNF
 wpc_setup "\<lambda>m. \<lbrace>P\<rbrace>,\<lbrace>R\<rbrace> m \<lbrace>G\<rbrace>,\<lbrace>S\<rbrace>" wpc_helper_validI
 
-lemma in_liftM:
- "((r, s') \<in> mres (liftM t f s)) = (\<exists>r'. (r', s') \<in> mres (f s) \<and> r = t r')"
-  by (simp add: liftM_def in_return in_bind)
-
-lemma hoare_fun_app_wp[wp]:
-  "\<lbrace>P\<rbrace> f' x \<lbrace>Q'\<rbrace> \<Longrightarrow> \<lbrace>P\<rbrace> f' $ x \<lbrace>Q'\<rbrace>"
-  "\<lbrace>P\<rbrace> f x \<lbrace>Q\<rbrace>,\<lbrace>E\<rbrace> \<Longrightarrow> \<lbrace>P\<rbrace> f $ x \<lbrace>Q\<rbrace>,\<lbrace>E\<rbrace>"
-  "\<lbrace>P\<rbrace> f x \<lbrace>Q\<rbrace>,- \<Longrightarrow> \<lbrace>P\<rbrace> f $ x \<lbrace>Q\<rbrace>,-"
-  "\<lbrace>P\<rbrace> f x -,\<lbrace>E\<rbrace> \<Longrightarrow> \<lbrace>P\<rbrace> f $ x -,\<lbrace>E\<rbrace>"
-  by simp+
-
-lemma hoare_validE_pred_conj:
-  "\<lbrakk> \<lbrace>P\<rbrace>f\<lbrace>Q\<rbrace>,\<lbrace>E\<rbrace>; \<lbrace>P\<rbrace>f\<lbrace>R\<rbrace>,\<lbrace>E\<rbrace> \<rbrakk> \<Longrightarrow> \<lbrace>P\<rbrace>f\<lbrace>Q and R\<rbrace>,\<lbrace>E\<rbrace>"
-  unfolding valid_def validE_def by (simp add: split_def split: sum.splits)
-
-lemma hoare_validE_conj:
-  "\<lbrakk> \<lbrace>P\<rbrace>f\<lbrace>Q\<rbrace>,\<lbrace>E\<rbrace>; \<lbrace>P\<rbrace>f\<lbrace>R\<rbrace>,\<lbrace>E\<rbrace> \<rbrakk> \<Longrightarrow> \<lbrace>P\<rbrace> f \<lbrace>\<lambda>r s. Q r s \<and> R r s\<rbrace>,\<lbrace>E\<rbrace>"
-  unfolding valid_def validE_def by (simp add: split_def split: sum.splits)
-
-lemma hoare_valid_validE:
-  "\<lbrace>P\<rbrace>f\<lbrace>\<lambda>r. Q\<rbrace> \<Longrightarrow> \<lbrace>P\<rbrace>f\<lbrace>\<lambda>r. Q\<rbrace>,\<lbrace>\<lambda>r. Q\<rbrace>"
-  unfolding valid_def validE_def by (simp add: split_def split: sum.splits)
-
-lemma liftE_validE_E [wp]:
-  "\<lbrace>\<top>\<rbrace> liftE f -, \<lbrace>Q\<rbrace>"
-  by (clarsimp simp: validE_E_def valid_def)
-
-lemma validE_validE_E [wp_comb]:
-  "\<lbrace>P\<rbrace> f \<lbrace>\<top>\<top>\<rbrace>, \<lbrace>E\<rbrace> \<Longrightarrow> \<lbrace>P\<rbrace> f -, \<lbrace>E\<rbrace>"
-  by (simp add: validE_E_def)
-
-lemma validE_E_validE:
-  "\<lbrace>P\<rbrace> f -, \<lbrace>E\<rbrace> \<Longrightarrow> \<lbrace>P\<rbrace> f \<lbrace>\<top>\<top>\<rbrace>, \<lbrace>E\<rbrace>"
-  by (simp add: validE_E_def)
-
-(*
- * if_validE_E:
- *
- * \<lbrakk>?P1 \<Longrightarrow> \<lbrace>?Q1\<rbrace> ?f1 -, \<lbrace>?E\<rbrace>; \<not> ?P1 \<Longrightarrow> \<lbrace>?R1\<rbrace> ?g1 -, \<lbrace>?E\<rbrace>\<rbrakk> \<Longrightarrow> \<lbrace>\<lambda>s. (?P1 \<longrightarrow> ?Q1 s) \<and> (\<not> ?P1 \<longrightarrow> ?R1 s)\<rbrace> if ?P1 then ?f1 else ?g1 -, \<lbrace>?E\<rbrace>
- *)
-lemmas if_validE_E [wp_split] =
-  validE_validE_E [OF hoare_vcg_split_ifE [OF validE_E_validE validE_E_validE]]
-
-lemma returnOk_E [wp]:
-  "\<lbrace>\<top>\<rbrace> returnOk r -, \<lbrace>Q\<rbrace>"
-  by (simp add: validE_E_def) wp
-
-lemma hoare_drop_imp:
-  "\<lbrace>P\<rbrace> f \<lbrace>Q\<rbrace> \<Longrightarrow> \<lbrace>P\<rbrace> f \<lbrace>\<lambda>r s. R r s \<longrightarrow> Q r s\<rbrace>"
-  by (auto simp: valid_def)
-
-lemma hoare_drop_impE:
-  "\<lbrakk>\<lbrace>P\<rbrace> f \<lbrace>\<lambda>r. Q\<rbrace>, \<lbrace>E\<rbrace>\<rbrakk> \<Longrightarrow> \<lbrace>P\<rbrace> f \<lbrace>\<lambda>r s. R r s \<longrightarrow> Q s\<rbrace>, \<lbrace>E\<rbrace>"
-  by (simp add: validE_weaken)
-
-lemma hoare_drop_impE_R:
-  "\<lbrace>P\<rbrace> f \<lbrace>Q\<rbrace>,- \<Longrightarrow> \<lbrace>P\<rbrace> f \<lbrace>\<lambda>r s. R r s \<longrightarrow> Q r s\<rbrace>, -"
-  by (auto simp: validE_R_def validE_def valid_def split_def split: sum.splits)
-
-lemma hoare_drop_impE_E:
-  "\<lbrace>P\<rbrace> f -,\<lbrace>Q\<rbrace> \<Longrightarrow> \<lbrace>P\<rbrace> f -,\<lbrace>\<lambda>r s. R r s \<longrightarrow> Q r s\<rbrace>"
-  by (auto simp: validE_E_def validE_def valid_def split_def split: sum.splits)
-
-lemmas hoare_drop_imps = hoare_drop_imp hoare_drop_impE_R hoare_drop_impE_E
 lemma mres_union:
  "mres (a \<union> b) = mres a \<union> mres b"
   by (simp add: mres_def image_Un)
@@ -2084,450 +1585,6 @@ lemma det_set_option_eq':
   "(\<Union>a\<in>m. set_option (snd a)) = {(r, s')} \<Longrightarrow>
        Some (r, s') \<in> snd ` m"
   using image_iff by fastforce
-
-lemma bind_det_exec:
-  "mres (a s) = {(r,s')} \<Longrightarrow> mres ((a >>= b) s) = mres (b r s')"
-  by (simp add: in_bind set_eq_iff)
-
-lemma in_bind_det_exec:
-  "mres (a s) = {(r,s')} \<Longrightarrow> (s'' \<in> mres ((a >>= b) s)) = (s'' \<in> mres (b r s'))"
-  by (cases s'', simp add: in_bind)
-
-lemma exec_put:
-  "(put s' >>= m) s = m () s'"
-  by (auto simp add: bind_def put_def mres_def split_def)
-
-lemma bind_execI:
-  "\<lbrakk> (r'',s'') \<in> mres (f s); \<exists>x \<in> mres (g r'' s''). P x \<rbrakk> \<Longrightarrow>
-  \<exists>x \<in> mres ((f >>= g) s). P x"
-  by (fastforce simp add: Bex_def in_bind)
-
-lemma True_E_E [wp]: "\<lbrace>\<top>\<rbrace> f -,\<lbrace>\<top>\<top>\<rbrace>"
-  by (auto simp: validE_E_def validE_def valid_def split: sum.splits)
-
-(*
- * \<lbrakk>\<And>x. \<lbrace>?B1 x\<rbrace> ?g1 x -, \<lbrace>?E\<rbrace>; \<lbrace>?P\<rbrace> ?f1 \<lbrace>?B1\<rbrace>, \<lbrace>?E\<rbrace>\<rbrakk> \<Longrightarrow> \<lbrace>?P\<rbrace> ?f1 >>=E ?g1 -, \<lbrace>?E\<rbrace>
- *)
-lemmas [wp_split] =
-  validE_validE_E [OF hoare_vcg_seqE [OF validE_E_validE]]
-
-lemma case_option_wp:
-  assumes x: "\<And>x. \<lbrace>P x\<rbrace> m x \<lbrace>Q\<rbrace>"
-  assumes y: "\<lbrace>P'\<rbrace> m' \<lbrace>Q\<rbrace>"
-  shows      "\<lbrace>\<lambda>s. (x = None \<longrightarrow> P' s) \<and> (x \<noteq> None \<longrightarrow> P (the x) s)\<rbrace>
-                case_option m' m x \<lbrace>Q\<rbrace>"
-  apply (cases x; simp)
-   apply (rule y)
-  apply (rule x)
-  done
-
-lemma case_option_wpE:
-  assumes x: "\<And>x. \<lbrace>P x\<rbrace> m x \<lbrace>Q\<rbrace>,\<lbrace>E\<rbrace>"
-  assumes y: "\<lbrace>P'\<rbrace> m' \<lbrace>Q\<rbrace>,\<lbrace>E\<rbrace>"
-  shows      "\<lbrace>\<lambda>s. (x = None \<longrightarrow> P' s) \<and> (x \<noteq> None \<longrightarrow> P (the x) s)\<rbrace>
-                case_option m' m x \<lbrace>Q\<rbrace>,\<lbrace>E\<rbrace>"
-  apply (cases x; simp)
-   apply (rule y)
-  apply (rule x)
-  done
-
-lemma in_bindE:
-  "(rv, s') \<in> mres ((f >>=E (\<lambda>rv'. g rv')) s) =
-  ((\<exists>ex. rv = Inl ex \<and> (Inl ex, s') \<in> mres (f s)) \<or>
-  (\<exists>rv' s''. (rv, s') \<in> mres (g rv' s'') \<and> (Inr rv', s'') \<in> mres (f s)))"
-  apply (clarsimp simp: bindE_def in_bind lift_def in_throwError)
-  apply (safe del: disjCI; strengthen subst[where P="\<lambda>x. x \<in> mres (f s)", mk_strg I _ E];
-    auto simp: in_throwError split: sum.splits)
-  done
-
-(*
- * \<lbrace>?P\<rbrace> ?m1 -, \<lbrace>?E\<rbrace> \<Longrightarrow> \<lbrace>?P\<rbrace> liftME ?f1 ?m1 -, \<lbrace>?E\<rbrace>
- *)
-lemmas [wp_split] = validE_validE_E [OF liftME_wp, simplified, OF validE_E_validE]
-
-lemma assert_A_True[simp]: "assert True = return ()"
-  by (simp add: assert_def)
-
-lemma assert_wp [wp]: "\<lbrace>\<lambda>s. P \<longrightarrow> Q () s\<rbrace> assert P \<lbrace>Q\<rbrace>"
-  by (cases P, (simp add: assert_def | wp)+)
-
-lemma list_cases_wp:
-  assumes a: "\<lbrace>P_A\<rbrace> a \<lbrace>Q\<rbrace>"
-  assumes b: "\<And>x xs. ts = x#xs \<Longrightarrow> \<lbrace>P_B x xs\<rbrace> b x xs \<lbrace>Q\<rbrace>"
-  shows "\<lbrace>case_list P_A P_B ts\<rbrace> case ts of [] \<Rightarrow> a | x # xs \<Rightarrow> b x xs \<lbrace>Q\<rbrace>"
-  by (cases ts, auto simp: a b)
-
-(* FIXME: make wp *)
-lemma whenE_throwError_wp:
-  "\<lbrace>\<lambda>s. \<not>Q \<longrightarrow> P s\<rbrace> whenE Q (throwError e) \<lbrace>\<lambda>rv. P\<rbrace>, -"
-  unfolding whenE_def by wp blast
-
-lemma select_throwError_wp:
-  "\<lbrace>\<lambda>s. \<forall>x\<in>S. Q x s\<rbrace> select S >>= throwError -, \<lbrace>Q\<rbrace>"
-  by (clarsimp simp add: bind_def throwError_def return_def select_def validE_E_def
-                validE_def valid_def mres_def)
-
-
-section "validNF Rules"
-
-subsection "Basic validNF theorems"
-
-lemma validNF [intro?]:
-  "\<lbrakk> \<lbrace> P \<rbrace> f \<lbrace> Q \<rbrace>; no_fail P f \<rbrakk> \<Longrightarrow> \<lbrace> P \<rbrace> f \<lbrace> Q \<rbrace>!"
-  by (clarsimp simp: validNF_def)
-
-lemma validNF_valid: "\<lbrakk> \<lbrace> P \<rbrace> f \<lbrace> Q \<rbrace>! \<rbrakk> \<Longrightarrow> \<lbrace> P \<rbrace> f \<lbrace> Q \<rbrace>"
-  by (clarsimp simp: validNF_def)
-
-lemma validNF_no_fail: "\<lbrakk> \<lbrace> P \<rbrace> f \<lbrace> Q \<rbrace>! \<rbrakk> \<Longrightarrow> no_fail P f"
-  by (clarsimp simp: validNF_def)
-
-lemma snd_validNF:
-  "\<lbrakk> \<lbrace> P \<rbrace> f \<lbrace> Q \<rbrace>!; P s \<rbrakk> \<Longrightarrow> Failed \<notin> snd ` (f s)"
-  by (clarsimp simp: validNF_def no_fail_def)
-
-lemma use_validNF:
-  "\<lbrakk> (r', s') \<in> mres (f s); \<lbrace> P \<rbrace> f \<lbrace> Q \<rbrace>!; P s \<rbrakk> \<Longrightarrow> Q r' s'"
-  by (fastforce simp: validNF_def valid_def)
-
-subsection "validNF weakest pre-condition rules"
-
-lemma validNF_return [wp]:
-  "\<lbrace> P x \<rbrace> return x \<lbrace> P \<rbrace>!"
-  by (wp validNF)+
-
-lemma validNF_get [wp]:
-  "\<lbrace> \<lambda>s. P s s  \<rbrace> get \<lbrace> P \<rbrace>!"
-  by (wp validNF)+
-
-lemma validNF_put [wp]:
-  "\<lbrace> \<lambda>s. P () x  \<rbrace> put x \<lbrace> P \<rbrace>!"
-  by (wp validNF)+
-
-lemma validNF_K_bind [wp]:
-  "\<lbrace> P \<rbrace> x \<lbrace> Q \<rbrace>! \<Longrightarrow> \<lbrace> P \<rbrace> K_bind x f \<lbrace> Q \<rbrace>!"
-  by simp
-
-lemma validNF_fail [wp]:
-  "\<lbrace> \<lambda>s. False \<rbrace> fail \<lbrace> Q \<rbrace>!"
-  by (clarsimp simp: validNF_def fail_def no_fail_def)
-
-lemma validNF_prop [wp_unsafe]:
-  "\<lbrakk> no_fail (\<lambda>s. P) f \<rbrakk> \<Longrightarrow> \<lbrace> \<lambda>s. P \<rbrace> f \<lbrace> \<lambda>rv s. P \<rbrace>!"
-  by (wp validNF)+
-
-lemma validNF_post_conj [intro!]:
-  "\<lbrakk> \<lbrace> P \<rbrace> a \<lbrace> Q \<rbrace>!; \<lbrace> P \<rbrace> a \<lbrace> R \<rbrace>! \<rbrakk> \<Longrightarrow> \<lbrace> P \<rbrace> a \<lbrace> Q and R \<rbrace>!"
-  by (clarsimp simp: validNF_def)
-
-lemma no_fail_or:
-  "\<lbrakk>no_fail P a; no_fail Q a\<rbrakk> \<Longrightarrow> no_fail (P or Q) a"
-  by (clarsimp simp: no_fail_def)
-
-lemma validNF_pre_disj [intro!]:
-  "\<lbrakk> \<lbrace> P \<rbrace> a \<lbrace> R \<rbrace>!; \<lbrace> Q \<rbrace> a \<lbrace> R \<rbrace>! \<rbrakk> \<Longrightarrow> \<lbrace> P or Q \<rbrace> a \<lbrace> R \<rbrace>!"
-  by (rule validNF) (auto dest: validNF_valid validNF_no_fail intro: no_fail_or)
-
-(*
- * Set up combination rules for WP, which also requires
- * a "wp_trip" rule for validNF.
- *)
-
-definition "validNF_property Q s b \<equiv> Failed \<notin> snd ` (b s) \<and> (\<forall>(r', s') \<in> mres (b s). Q r' s')"
-
-lemma validNF_is_triple [wp_trip]:
-  "validNF P f Q = triple_judgement P f (validNF_property Q)"
-  apply (clarsimp simp: validNF_def triple_judgement_def validNF_property_def)
-  apply (auto simp: no_fail_def valid_def)
-  done
-
-lemma validNF_weaken_pre [wp_comb]:
-  "\<lbrakk>\<lbrace>Q\<rbrace> a \<lbrace>R\<rbrace>!; \<And>s. P s \<Longrightarrow> Q s\<rbrakk> \<Longrightarrow> \<lbrace>P\<rbrace> a \<lbrace>R\<rbrace>!"
-  by (metis hoare_pre_imp no_fail_pre validNF_def)
-
-lemma validNF_post_comb_imp_conj:
-  "\<lbrakk> \<lbrace>P'\<rbrace> f \<lbrace>Q\<rbrace>!; \<lbrace>P\<rbrace> f \<lbrace>Q'\<rbrace>!; \<And>s. P s \<Longrightarrow> P' s \<rbrakk> \<Longrightarrow> \<lbrace>P\<rbrace> f \<lbrace>\<lambda>rv s. Q rv s \<and> Q' rv s\<rbrace>!"
-  by (fastforce simp: validNF_def valid_def)
-
-lemma validNF_post_comb_conj_L:
-  "\<lbrakk> \<lbrace>P'\<rbrace> f \<lbrace>Q\<rbrace>!; \<lbrace>P\<rbrace> f \<lbrace>Q'\<rbrace> \<rbrakk> \<Longrightarrow> \<lbrace>\<lambda>s. P s \<and> P' s \<rbrace> f \<lbrace>\<lambda>rv s. Q rv s \<and> Q' rv s\<rbrace>!"
-  apply (clarsimp simp: validNF_def valid_def no_fail_def)
-  apply force
-  done
-
-lemma validNF_post_comb_conj_R:
-  "\<lbrakk> \<lbrace>P'\<rbrace> f \<lbrace>Q\<rbrace>; \<lbrace>P\<rbrace> f \<lbrace>Q'\<rbrace>! \<rbrakk> \<Longrightarrow> \<lbrace>\<lambda>s. P s \<and> P' s \<rbrace> f \<lbrace>\<lambda>rv s. Q rv s \<and> Q' rv s\<rbrace>!"
-  apply (clarsimp simp: validNF_def valid_def no_fail_def)
-  apply force
-  done
-
-lemma validNF_post_comb_conj:
-  "\<lbrakk> \<lbrace>P'\<rbrace> f \<lbrace>Q\<rbrace>!; \<lbrace>P\<rbrace> f \<lbrace>Q'\<rbrace>! \<rbrakk> \<Longrightarrow> \<lbrace>\<lambda>s. P s \<and> P' s \<rbrace> f \<lbrace>\<lambda>rv s. Q rv s \<and> Q' rv s\<rbrace>!"
-  apply (clarsimp simp: validNF_def valid_def no_fail_def)
-  apply force
-  done
-
-lemma validNF_split_if [wp_split]:
-  "\<lbrakk>P \<Longrightarrow> \<lbrace>Q\<rbrace> f \<lbrace>S\<rbrace>!; \<not> P \<Longrightarrow> \<lbrace>R\<rbrace> g \<lbrace>S\<rbrace>!\<rbrakk> \<Longrightarrow> \<lbrace>\<lambda>s. (P \<longrightarrow> Q s) \<and> (\<not> P \<longrightarrow> R s)\<rbrace> if P then f else g \<lbrace>S\<rbrace>!"
-  by simp
-
-lemma validNF_vcg_conj_lift:
-  "\<lbrakk> \<lbrace>P\<rbrace> f \<lbrace>Q\<rbrace>!; \<lbrace>P'\<rbrace> f \<lbrace>Q'\<rbrace>! \<rbrakk> \<Longrightarrow>
-      \<lbrace>\<lambda>s. P s \<and> P' s\<rbrace> f \<lbrace>\<lambda>rv s. Q rv s \<and> Q' rv s\<rbrace>!"
-  apply (subst pred_conj_def[symmetric], subst pred_conj_def[symmetric], rule validNF_post_conj)
-   apply (erule validNF_weaken_pre, fastforce)
-  apply (erule validNF_weaken_pre, fastforce)
-  done
-
-lemma validNF_vcg_disj_lift:
-  "\<lbrakk> \<lbrace>P\<rbrace> f \<lbrace>Q\<rbrace>!; \<lbrace>P'\<rbrace> f \<lbrace>Q'\<rbrace>! \<rbrakk> \<Longrightarrow>
-       \<lbrace>\<lambda>s. P s \<or> P' s\<rbrace> f \<lbrace>\<lambda>rv s. Q rv s \<or> Q' rv s\<rbrace>!"
-  apply (clarsimp simp: validNF_def)
-  apply safe
-   apply (auto intro!: hoare_vcg_disj_lift)[1]
-  apply (clarsimp simp: no_fail_def)
-  done
-
-lemma validNF_vcg_all_lift [wp]:
-  "\<lbrakk> \<And>x. \<lbrace>P x\<rbrace> f \<lbrace>Q x\<rbrace>! \<rbrakk> \<Longrightarrow> \<lbrace>\<lambda>s. \<forall>x. P x s\<rbrace> f \<lbrace>\<lambda>rv s. \<forall>x. Q x rv s\<rbrace>!"
-  apply atomize
-  apply (rule validNF)
-   apply (clarsimp simp: validNF_def)
-   apply (rule hoare_vcg_all_lift)
-   apply force
-  apply (clarsimp simp: no_fail_def validNF_def)
-  done
-
-lemma no_fail_bind[wp_split]:
-  "\<lbrakk> no_fail P f; \<And>x. no_fail (R x) (g x); \<lbrace>Q\<rbrace> f \<lbrace>R\<rbrace> \<rbrakk>
-    \<Longrightarrow> no_fail (P and Q) (do x \<leftarrow> f; g x od)"
-  apply (simp add: no_fail_def bind_def2 image_Un image_image
-                   in_image_constant)
-  apply (intro allI conjI impI)
-   apply (fastforce simp: image_def)
-  apply clarsimp
-  apply (drule(1) post_by_hoare, erule in_mres)
-  apply (fastforce simp: image_def)
-  done
-
-lemma validNF_bind [wp_split]:
-  "\<lbrakk> \<And>x. \<lbrace>B x\<rbrace> g x \<lbrace>C\<rbrace>!; \<lbrace>A\<rbrace> f \<lbrace>B\<rbrace>! \<rbrakk> \<Longrightarrow>
-       \<lbrace>A\<rbrace> do x \<leftarrow> f; g x od \<lbrace>C\<rbrace>!"
-  apply (rule validNF)
-   apply (metis validNF_valid hoare_seq_ext)
-  apply (frule no_fail_bind[OF validNF_no_fail, where g=g])
-    apply (rule validNF_no_fail, assumption)
-   apply (erule validNF_valid)
-  apply (simp add: no_fail_def)
-  done
-
-lemmas validNF_seq_ext = validNF_bind
-
-subsection "validNF compound rules"
-lemma validNF_state_assert [wp]:
-  "\<lbrace> \<lambda>s. P () s \<and> G s  \<rbrace> state_assert G \<lbrace> P \<rbrace>!"
-  apply (rule validNF)
-  apply wpsimp
-  apply (clarsimp simp: no_fail_def state_assert_def
-              bind_def2 assert_def return_def get_def)
-  done
-
-lemma validNF_modify [wp]:
-  "\<lbrace> \<lambda>s. P () (f s) \<rbrace> modify f \<lbrace> P \<rbrace>!"
-  apply (clarsimp simp: modify_def)
-  apply wp
-  done
-
-lemma validNF_gets [wp]:
-  "\<lbrace>\<lambda>s. P (f s) s\<rbrace> gets f \<lbrace>P\<rbrace>!"
-  apply (clarsimp simp: gets_def)
-  apply wp
-  done
-
-lemma validNF_condition [wp]:
-  "\<lbrakk> \<lbrace> Q \<rbrace> A \<lbrace>P\<rbrace>!; \<lbrace> R \<rbrace> B \<lbrace>P\<rbrace>!\<rbrakk> \<Longrightarrow> \<lbrace>\<lambda>s. if C s then Q s else R s\<rbrace> condition C A B \<lbrace>P\<rbrace>!"
-  apply rule
-   apply (drule validNF_valid)+
-   apply (erule (1) condition_wp)
-  apply (drule validNF_no_fail)+
-  apply (clarsimp simp: no_fail_def condition_def)
-  done
-
-lemma validNF_alt_def:
-  "validNF P m Q = (\<forall>s. P s \<longrightarrow> ((\<forall>(r', s') \<in> mres (m s). Q r' s') \<and> Failed \<notin> snd ` (m s)))"
-  by (auto simp: validNF_def valid_def no_fail_def mres_def image_def)
-
-lemma validNF_assert [wp]:
-    "\<lbrace> (\<lambda>s. P) and (R ()) \<rbrace> assert P \<lbrace> R \<rbrace>!"
-  apply (rule validNF)
-   apply (clarsimp simp: valid_def in_return)
-  apply (clarsimp simp: no_fail_def return_def)
-  done
-
-lemma validNF_false_pre:
-  "\<lbrace> \<lambda>_. False \<rbrace> P \<lbrace> Q \<rbrace>!"
-  by (clarsimp simp: validNF_def no_fail_def)
-
-lemma validNF_chain:
-   "\<lbrakk>\<lbrace>P'\<rbrace> a \<lbrace>R'\<rbrace>!; \<And>s. P s \<Longrightarrow> P' s; \<And>r s. R' r s \<Longrightarrow> R r s\<rbrakk> \<Longrightarrow> \<lbrace>P\<rbrace> a \<lbrace>R\<rbrace>!"
-  by (fastforce simp: validNF_def valid_def no_fail_def Ball_def)
-
-lemma validNF_case_prod [wp]:
-  "\<lbrakk> \<And>x y. validNF (P x y) (B x y) Q \<rbrakk> \<Longrightarrow> validNF (case_prod P v) (case_prod (\<lambda>x y. B x y) v) Q"
-  by (metis prod.exhaust split_conv)
-
-lemma validE_NF_case_prod [wp]:
-    "\<lbrakk> \<And>a b. \<lbrace>P a b\<rbrace> f a b \<lbrace>Q\<rbrace>, \<lbrace>E\<rbrace>! \<rbrakk> \<Longrightarrow>
-          \<lbrace>case x of (a, b) \<Rightarrow> P a b\<rbrace> case x of (a, b) \<Rightarrow> f a b \<lbrace>Q\<rbrace>, \<lbrace>E\<rbrace>!"
-  apply (clarsimp simp: validE_NF_alt_def)
-  apply (erule validNF_case_prod)
-  done
-
-lemma no_fail_is_validNF_True: "no_fail P s = (\<lbrace> P \<rbrace> s \<lbrace> \<lambda>_ _. True \<rbrace>!)"
-  by (clarsimp simp: no_fail_def validNF_def valid_def)
-
-subsection "validNF reasoning in the exception monad"
-
-lemma validE_NF [intro?]:
-  "\<lbrakk> \<lbrace> P \<rbrace> f \<lbrace> Q \<rbrace>,\<lbrace> E \<rbrace>; no_fail P f \<rbrakk> \<Longrightarrow> \<lbrace> P \<rbrace> f \<lbrace> Q \<rbrace>,\<lbrace> E \<rbrace>!"
-  apply (clarsimp simp: validE_NF_def)
-  done
-
-lemma validE_NF_valid:
-  "\<lbrakk> \<lbrace> P \<rbrace> f \<lbrace> Q \<rbrace>,\<lbrace> E \<rbrace>! \<rbrakk> \<Longrightarrow> \<lbrace> P \<rbrace> f \<lbrace> Q \<rbrace>,\<lbrace> E \<rbrace>"
-  apply (clarsimp simp: validE_NF_def)
-  done
-
-lemma validE_NF_no_fail:
-  "\<lbrakk> \<lbrace> P \<rbrace> f \<lbrace> Q \<rbrace>,\<lbrace> E \<rbrace>! \<rbrakk> \<Longrightarrow> no_fail P f"
-  apply (clarsimp simp: validE_NF_def)
-  done
-
-lemma validE_NF_weaken_pre [wp_comb]:
-   "\<lbrakk>\<lbrace>Q\<rbrace> a \<lbrace>R\<rbrace>,\<lbrace>E\<rbrace>!; \<And>s. P s \<Longrightarrow> Q s\<rbrakk> \<Longrightarrow> \<lbrace>P\<rbrace> a \<lbrace>R\<rbrace>,\<lbrace>E\<rbrace>!"
-  apply (clarsimp simp: validE_NF_alt_def)
-  apply (erule validNF_weaken_pre)
-  apply simp
-  done
-
-lemma validE_NF_post_comb_conj_L:
-  "\<lbrakk> \<lbrace>P\<rbrace> f \<lbrace>Q\<rbrace>, \<lbrace> E \<rbrace>!; \<lbrace>P'\<rbrace> f \<lbrace>Q'\<rbrace>, \<lbrace> \<lambda>_ _. True \<rbrace> \<rbrakk> \<Longrightarrow> \<lbrace>\<lambda>s. P s \<and> P' s \<rbrace> f \<lbrace>\<lambda>rv s. Q rv s \<and> Q' rv s\<rbrace>, \<lbrace> E \<rbrace>!"
-  apply (clarsimp simp: validE_NF_alt_def validE_def validNF_def
-          valid_def no_fail_def split: sum.splits)
-  apply force
-  done
-
-lemma validE_NF_post_comb_conj_R:
-  "\<lbrakk> \<lbrace>P\<rbrace> f \<lbrace>Q\<rbrace>, \<lbrace> \<lambda>_ _. True \<rbrace>; \<lbrace>P'\<rbrace> f \<lbrace>Q'\<rbrace>, \<lbrace> E \<rbrace>! \<rbrakk> \<Longrightarrow> \<lbrace>\<lambda>s. P s \<and> P' s \<rbrace> f \<lbrace>\<lambda>rv s. Q rv s \<and> Q' rv s\<rbrace>, \<lbrace> E \<rbrace>!"
-  apply (clarsimp simp: validE_NF_alt_def validE_def validNF_def
-          valid_def no_fail_def split: sum.splits)
-  apply force
-  done
-
-lemma validE_NF_post_comb_conj:
-  "\<lbrakk> \<lbrace>P\<rbrace> f \<lbrace>Q\<rbrace>, \<lbrace> E \<rbrace>!; \<lbrace>P'\<rbrace> f \<lbrace>Q'\<rbrace>, \<lbrace> E \<rbrace>! \<rbrakk> \<Longrightarrow> \<lbrace>\<lambda>s. P s \<and> P' s \<rbrace> f \<lbrace>\<lambda>rv s. Q rv s \<and> Q' rv s\<rbrace>, \<lbrace> E \<rbrace>!"
-  apply (clarsimp simp: validE_NF_alt_def validE_def validNF_def
-          valid_def no_fail_def split: sum.splits)
-  apply force
-  done
-
-lemma validE_NF_chain:
-   "\<lbrakk>\<lbrace>P'\<rbrace> a \<lbrace>R'\<rbrace>,\<lbrace>E'\<rbrace>!;
-    \<And>s. P s \<Longrightarrow> P' s;
-    \<And>r' s'. R' r' s' \<Longrightarrow> R r' s';
-    \<And>r'' s''. E' r'' s'' \<Longrightarrow> E r'' s''\<rbrakk> \<Longrightarrow>
-  \<lbrace>\<lambda>s. P s \<rbrace> a \<lbrace>\<lambda>r' s'. R r' s'\<rbrace>,\<lbrace>\<lambda>r'' s''. E r'' s''\<rbrace>!"
-  by (fastforce simp: validE_NF_def validE_def2 no_fail_def Ball_def split: sum.splits)
-
-lemma validE_NF_bind_wp [wp]:
-  "\<lbrakk>\<And>x. \<lbrace>B x\<rbrace> g x \<lbrace>C\<rbrace>, \<lbrace>E\<rbrace>!; \<lbrace>A\<rbrace> f \<lbrace>B\<rbrace>, \<lbrace>E\<rbrace>!\<rbrakk> \<Longrightarrow> \<lbrace>A\<rbrace> f >>=E (\<lambda>x. g x) \<lbrace>C\<rbrace>, \<lbrace>E\<rbrace>!"
-  apply (unfold validE_NF_alt_def bindE_def)
-  apply (rule validNF_bind [rotated])
-   apply assumption
-  apply (clarsimp simp: lift_def throwError_def split: sum.splits)
-    apply wpsimp
-  done
-
-lemma validNF_catch [wp]:
-  "\<lbrakk>\<And>x. \<lbrace>E x\<rbrace> handler x \<lbrace>Q\<rbrace>!; \<lbrace>P\<rbrace> f \<lbrace>Q\<rbrace>, \<lbrace>E\<rbrace>!\<rbrakk> \<Longrightarrow> \<lbrace>P\<rbrace> f <catch> (\<lambda>x. handler x) \<lbrace>Q\<rbrace>!"
-  apply (unfold validE_NF_alt_def catch_def)
-  apply (rule validNF_bind [rotated])
-   apply assumption
-  apply (clarsimp simp: lift_def throwError_def split: sum.splits)
-  apply wp
-  done
-
-lemma validNF_throwError [wp]:
-  "\<lbrace>E e\<rbrace> throwError e \<lbrace>P\<rbrace>, \<lbrace>E\<rbrace>!"
-  by (unfold validE_NF_alt_def throwError_def o_def) wpsimp
-
-lemma validNF_returnOk [wp]:
-  "\<lbrace>P e\<rbrace> returnOk e \<lbrace>P\<rbrace>, \<lbrace>E\<rbrace>!"
- by (clarsimp simp: validE_NF_alt_def returnOk_def) wpsimp
-
-lemma validNF_whenE [wp]:
-  "(P \<Longrightarrow> \<lbrace>Q\<rbrace> f \<lbrace>R\<rbrace>, \<lbrace>E\<rbrace>!) \<Longrightarrow> \<lbrace>if P then Q else R ()\<rbrace> whenE P f \<lbrace>R\<rbrace>, \<lbrace>E\<rbrace>!"
-  unfolding whenE_def by clarsimp wp
-
-lemma validNF_nobindE [wp]:
-  "\<lbrakk> \<lbrace>B\<rbrace> g \<lbrace>C\<rbrace>,\<lbrace>E\<rbrace>!;
-     \<lbrace>A\<rbrace> f \<lbrace>\<lambda>r s. B s\<rbrace>,\<lbrace>E\<rbrace>! \<rbrakk> \<Longrightarrow>
-   \<lbrace>A\<rbrace> doE f; g odE \<lbrace>C\<rbrace>,\<lbrace>E\<rbrace>!"
-  by clarsimp wp
-
-(*
- * Setup triple rules for validE_NF so that we can use the
- * "wp_comb" attribute.
- *)
-
-definition "validE_NF_property Q E s b \<equiv> Failed \<notin> snd ` (b s)
-       \<and> (\<forall>(r', s') \<in> mres (b s). case r' of Inl x \<Rightarrow> E x s' | Inr x \<Rightarrow> Q x s')"
-
-lemma validE_NF_is_triple [wp_trip]:
-  "validE_NF P f Q E = triple_judgement P f (validE_NF_property Q E)"
-  apply (clarsimp simp: validE_NF_def validE_def2 no_fail_def triple_judgement_def
-           validE_NF_property_def split: sum.splits)
-  apply blast
-  done
-
-lemmas [wp_comb] = validE_NF_weaken_pre
-
-lemma validNF_cong:
-   "\<lbrakk> \<And>s. P s = P' s; \<And>s. P s \<Longrightarrow> m s = m' s;
-           \<And>r' s' s. \<lbrakk> P s; (r', s') \<in> mres (m s) \<rbrakk> \<Longrightarrow> Q r' s' = Q' r' s' \<rbrakk> \<Longrightarrow>
-     (\<lbrace> P \<rbrace> m \<lbrace> Q \<rbrace>!) = (\<lbrace> P' \<rbrace> m' \<lbrace> Q' \<rbrace>!)"
-  by (fastforce simp: validNF_alt_def)
-
-lemma validE_NF_liftE [wp]:
-  "\<lbrace>P\<rbrace> f \<lbrace>Q\<rbrace>! \<Longrightarrow> \<lbrace>P\<rbrace> liftE f \<lbrace>Q\<rbrace>,\<lbrace>E\<rbrace>!"
-  by (wpsimp simp: validE_NF_alt_def liftE_def)
-
-lemma validE_NF_handleE' [wp]:
-  "\<lbrakk> \<And>x. \<lbrace>F x\<rbrace> handler x \<lbrace>Q\<rbrace>,\<lbrace>E\<rbrace>!; \<lbrace>P\<rbrace> f \<lbrace>Q\<rbrace>,\<lbrace>F\<rbrace>! \<rbrakk> \<Longrightarrow>
-   \<lbrace>P\<rbrace> f <handle2> (\<lambda>x. handler x) \<lbrace>Q\<rbrace>,\<lbrace>E\<rbrace>!"
-  apply (unfold validE_NF_alt_def handleE'_def)
-  apply (rule validNF_bind [rotated])
-   apply assumption
-  apply (clarsimp split: sum.splits)
-  apply wpsimp
-  done
-
-lemma validE_NF_handleE [wp]:
-  "\<lbrakk> \<And>x. \<lbrace>F x\<rbrace> handler x \<lbrace>Q\<rbrace>,\<lbrace>E\<rbrace>!; \<lbrace>P\<rbrace> f \<lbrace>Q\<rbrace>,\<lbrace>F\<rbrace>! \<rbrakk> \<Longrightarrow>
-   \<lbrace>P\<rbrace> f <handle> handler \<lbrace>Q\<rbrace>,\<lbrace>E\<rbrace>!"
-  apply (unfold handleE_def)
-  apply (metis validE_NF_handleE')
-  done
-
-lemma validE_NF_condition [wp]:
-  "\<lbrakk> \<lbrace> Q \<rbrace> A \<lbrace>P\<rbrace>,\<lbrace> E \<rbrace>!; \<lbrace> R \<rbrace> B \<lbrace>P\<rbrace>,\<lbrace> E \<rbrace>!\<rbrakk>
-      \<Longrightarrow> \<lbrace>\<lambda>s. if C s then Q s else R s\<rbrace> condition C A B \<lbrace>P\<rbrace>,\<lbrace> E \<rbrace>!"
-  apply rule
-   apply (drule validE_NF_valid)+
-   apply wp
-  apply (drule validE_NF_no_fail)+
-  apply (clarsimp simp: no_fail_def condition_def)
-  done
 
 lemma validI_name_pre:
   "prefix_closed f \<Longrightarrow>
@@ -2549,37 +1606,5 @@ lemma validI_well_behaved':
   done
 
 lemmas validI_well_behaved = validI_well_behaved'[unfolded le_fun_def, simplified]
-
-text \<open>Strengthen setup.\<close>
-
-context strengthen_implementation begin
-
-lemma strengthen_hoare [strg]:
-  "(\<And>r s. st F (\<longrightarrow>) (Q r s) (R r s))
-    \<Longrightarrow> st F (\<longrightarrow>) (\<lbrace>P\<rbrace> f \<lbrace>Q\<rbrace>) (\<lbrace>P\<rbrace> f \<lbrace>R\<rbrace>)"
-  by (cases F, auto elim: hoare_strengthen_post)
-
-lemma strengthen_validE_R_cong[strg]:
-  "(\<And>r s. st F (\<longrightarrow>) (Q r s) (R r s))
-    \<Longrightarrow> st F (\<longrightarrow>) (\<lbrace>P\<rbrace> f \<lbrace>Q\<rbrace>, -) (\<lbrace>P\<rbrace> f \<lbrace>R\<rbrace>, -)"
-  by (cases F, auto intro: hoare_post_imp_R)
-
-lemma strengthen_validE_cong[strg]:
-  "(\<And>r s. st F (\<longrightarrow>) (Q r s) (R r s))
-    \<Longrightarrow> (\<And>r s. st F (\<longrightarrow>) (S r s) (T r s))
-    \<Longrightarrow> st F (\<longrightarrow>) (\<lbrace>P\<rbrace> f \<lbrace>Q\<rbrace>, \<lbrace>S\<rbrace>) (\<lbrace>P\<rbrace> f \<lbrace>R\<rbrace>, \<lbrace>T\<rbrace>)"
-  by (cases F, auto elim: hoare_post_impErr)
-
-lemma strengthen_validE_E_cong[strg]:
-  "(\<And>r s. st F (\<longrightarrow>) (S r s) (T r s))
-    \<Longrightarrow> st F (\<longrightarrow>) (\<lbrace>P\<rbrace> f -, \<lbrace>S\<rbrace>) (\<lbrace>P\<rbrace> f -, \<lbrace>T\<rbrace>)"
-  by (cases F, auto elim: hoare_post_impErr simp: validE_E_def)
-
-lemma strengthen_validI[strg]:
-  "(\<And>r s0 s. st F (\<longrightarrow>) (Q r s0 s) (Q' r s0 s))
-    \<Longrightarrow> st F (\<longrightarrow>) (\<lbrace>P\<rbrace>,\<lbrace>G\<rbrace> f \<lbrace>R\<rbrace>,\<lbrace>Q\<rbrace>) (\<lbrace>P\<rbrace>,\<lbrace>G\<rbrace> f \<lbrace>R\<rbrace>,\<lbrace>Q'\<rbrace>)"
-  by (cases F, auto elim: validI_strengthen_post)
-
-end
 
 end
