lib/Monads/trace/Trace_More_VCG.thy
@@ -1,0 +1,20 @@
+(*
+ * Copyright 2023, Proofcraft Pty Ltd
+ * Copyright 2020, Data61, CSIRO (ABN 41 687 119 230)
+ *
+ * SPDX-License-Identifier: BSD-2-Clause
+ *)
+
+(* Partial correctness Hoare logic lemmas over the trace monad. Hoare triples, lifting lemmas, etc.
+   If it doesn't contain a Hoare triple it likely doesn't belong in here. *)
+
+theory Trace_More_VCG
+  imports
+    Trace_VCG
+begin
+
+lemma hoare_pre_tautI:
+  "\<lbrakk> \<lbrace>A and P\<rbrace> a \<lbrace>B\<rbrace>; \<lbrace>A and not P\<rbrace> a \<lbrace>B\<rbrace> \<rbrakk> \<Longrightarrow> \<lbrace>A\<rbrace> a \<lbrace>B\<rbrace>"
+  by (fastforce simp: valid_def split_def pred_conj_def pred_neg_def)
+
+end
