lib/Monads/trace/Trace_No_Fail.thy
@@ -1,0 +1,142 @@
+(*
+ * Copyright 2023, Proofcraft Pty Ltd
+ * Copyright 2020, Data61, CSIRO (ABN 41 687 119 230)
+ *
+ * SPDX-License-Identifier: BSD-2-Clause
+ *)
+
+(* Lemmas about the no_fail predicate. *)
+
+theory Trace_No_Fail
+  imports
+    Trace_In_Monad
+    Trace_VCG
+    WPSimp
+begin
+
+subsection "Non-Failure"
+
+text \<open>
+  With the failure flag, we can formulate non-failure separately from validity.
+  A monad @{text m} does not fail under precondition @{text P}, if for no start
+  state that satisfies the precondition it sets the failure flag.
+\<close>
+definition no_fail :: "('s \<Rightarrow> bool) \<Rightarrow> ('s,'a) tmonad \<Rightarrow> bool" where
+  "no_fail P m \<equiv> \<forall>s. P s \<longrightarrow> Failed \<notin> snd ` (m s)"
+
+
+subsection \<open>@{method wpc} setup\<close>
+
+lemma no_fail_pre[wp_pre]:
+  "\<lbrakk> no_fail P f; \<And>s. Q s \<Longrightarrow> P s\<rbrakk> \<Longrightarrow> no_fail Q f"
+  by (simp add: no_fail_def)
+
+lemma wpc_helper_no_fail_final:
+  "no_fail Q f \<Longrightarrow> wpc_helper (P, P', P'') (Q, Q', Q'') (no_fail P f)"
+  by (clarsimp simp: wpc_helper_def elim!: no_fail_pre)
+
+wpc_setup "\<lambda>m. no_fail P m" wpc_helper_no_fail_final
+
+
+subsection \<open>Bundles\<close>
+
+bundle no_pre = hoare_pre [wp_pre del] no_fail_pre [wp_pre del]
+
+
+subsection \<open>Lemmas\<close>
+
+lemma no_failD:
+  "\<lbrakk> no_fail P m; P s \<rbrakk> \<Longrightarrow> Failed \<notin> snd ` m s"
+  by (simp add: no_fail_def)
+
+lemma no_fail_modify[wp,simp]:
+  "no_fail \<top> (modify f)"
+  by (simp add: no_fail_def modify_def get_def put_def bind_def)
+
+lemma no_fail_gets_simp[simp]:
+  "no_fail P (gets f)"
+  unfolding no_fail_def gets_def get_def return_def bind_def
+  by simp
+
+lemma no_fail_gets[wp]:
+  "no_fail \<top> (gets f)"
+  by simp
+
+lemma no_fail_select[simp]:
+  "no_fail \<top> (select S)"
+  by (simp add: no_fail_def select_def image_def)
+
+lemma no_fail_alt[wp]:
+  "\<lbrakk> no_fail P f; no_fail Q g \<rbrakk> \<Longrightarrow> no_fail (P and Q) (f \<sqinter> g)"
+  by (auto simp: no_fail_def alternative_def)
+
+lemma no_fail_return[simp, wp]:
+  "no_fail \<top> (return x)"
+  by (simp add: return_def no_fail_def)
+
+lemma no_fail_get[simp, wp]:
+  "no_fail \<top> get"
+  by (simp add: get_def no_fail_def)
+
+lemma no_fail_put[simp, wp]:
+  "no_fail \<top> (put s)"
+  by (simp add: put_def no_fail_def)
+
+lemma no_fail_when[wp]:
+  "(P \<Longrightarrow> no_fail Q f) \<Longrightarrow> no_fail (if P then Q else \<top>) (when P f)"
+  by (simp add: when_def)
+
+lemma no_fail_unless[wp]:
+  "(\<not>P \<Longrightarrow> no_fail Q f) \<Longrightarrow> no_fail (if P then \<top> else Q) (unless P f)"
+  by (simp add: unless_def when_def)
+
+lemma no_fail_fail[simp, wp]:
+  "no_fail \<bottom> fail"
+  by (simp add: fail_def no_fail_def)
+
+lemma no_fail_assert[simp, wp]:
+  "no_fail (\<lambda>_. P) (assert P)"
+  by (simp add: assert_def)
+
+lemma no_fail_assert_opt[simp, wp]:
+  "no_fail (\<lambda>_. P \<noteq> None) (assert_opt P)"
+  by (simp add: assert_opt_def split: option.splits)
+
+lemma no_fail_case_option[wp]:
+  assumes f: "no_fail P f"
+  assumes g: "\<And>x. no_fail (Q x) (g x)"
+  shows "no_fail (if x = None then P else Q (the x)) (case_option f g x)"
+  by (clarsimp simp add: f g)
+
+lemma no_fail_if[wp]:
+  "\<lbrakk> P \<Longrightarrow> no_fail Q f; \<not>P \<Longrightarrow> no_fail R g \<rbrakk> \<Longrightarrow> no_fail (if P then Q else R) (if P then f else g)"
+  by simp
+
+lemma no_fail_apply[wp]:
+  "no_fail P (f (g x)) \<Longrightarrow> no_fail P (f $ g x)"
+  by simp
+
+lemma no_fail_undefined[simp, wp]:
+  "no_fail \<bottom> undefined"
+  by (simp add: no_fail_def)
+
+lemma no_fail_returnOK[simp, wp]:
+  "no_fail \<top> (returnOk x)"
+  by (simp add: returnOk_def)
+
+lemma no_fail_bind[wp]:
+  "\<lbrakk> no_fail P f; \<And>x. no_fail (R x) (g x); \<lbrace>Q\<rbrace> f \<lbrace>R\<rbrace> \<rbrakk> \<Longrightarrow> no_fail (P and Q) (f >>= (\<lambda>rv. g rv))"
+  apply (simp add: no_fail_def bind_def2 image_Un image_image
+                   in_image_constant)
+  apply (intro allI conjI impI)
+   apply (fastforce simp: image_def)
+  apply clarsimp
+  apply (drule(1) post_by_hoare, erule in_mres)
+  apply (fastforce simp: image_def)
+  done
+
+lemma no_fail_or:
+  "\<lbrakk>no_fail P a; no_fail Q a\<rbrakk> \<Longrightarrow> no_fail (P or Q) a"
+  by (clarsimp simp: no_fail_def)
+
+end
